# baseURI: http://anzsoil.org/def/au/asls/landform
# imports: http://purl.org/dc/elements/1.1/
# imports: http://www.w3.org/ns/sosa/

@prefix asls: <http://anzsoil.org/def/au/asls/> .
@prefix dc: <http://purl.org/dc/elements/1.1/> .
@prefix dcterms: <http://purl.org/dc/terms/> .
@prefix foaf: <http://xmlns.com/foaf/0.1/> .
@prefix lf: <http://anzsoil.org/def/au/asls/landform/> .
@prefix owl: <http://www.w3.org/2002/07/owl#> .
@prefix rdf: <http://www.w3.org/1999/02/22-rdf-syntax-ns#> .
@prefix rdfs: <http://www.w3.org/2000/01/rdf-schema#> .
@prefix reg: <http://purl.org/linked-data/registry#> .
@prefix skos: <http://www.w3.org/2004/02/skos/core#> .
@prefix skos-ext: <http://linked.data.gov.au/def/skos-ext#> .
@prefix sosa: <http://www.w3.org/ns/sosa/> .
@prefix ui: <http://purl.org/linked-data/registry-ui#> .
@prefix xsd: <http://www.w3.org/2001/XMLSchema#> .

asls:landform
  a owl:Ontology ;
  a skos:ConceptScheme ;
  dcterms:contributor <https://orcid.org/0000-0002-0693-1899> ;
  dcterms:contributor <https://orcid.org/0000-0002-3884-3420> ;
  dcterms:created "2018-01-16"^^xsd:date ;
  dcterms:creator [
      a dcterms:Agent ;
      foaf:name "J.G. Speight" ;
    ] ;
  dcterms:description """This vocabulary is a machine-readable representation of the classifiers described in chapter 5 Landform, by J.G. Speight in Australian Soil and Land Survey Field Handbook (3rd edn). 
In this technique for describing landforms, the whole land surface is viewed as a mosaic of tiles of odd shapes and sizes. The scheme is intended to produce a record of observations rather than inferences.""" ;
  dcterms:identifier "http://anzsoil.org/def/au/asls/landform"^^xsd:anyURI ;
  dcterms:identifier "http://anzsoil.org/def/au/asls/vegetation"^^xsd:anyURI ;
  dcterms:isFormatOf <https://catalogue.nla.gov.au/Record/4273240> ;
  dcterms:license <http://creativecommons.org/licences/by/4.0> ;
  dcterms:modified "2022-07-26"^^xsd:date ;
  dcterms:publisher <http://www.publish.csiro.au/> ;
  dcterms:rights "copyright CSIRO 2009, 2021. All rights reserved."@en ;
  dcterms:source "National Committee on Soil and Terrain (2009), 'Australian soil and land survey field handbook (3rd edn).' (CSIRO Publishing: Melbourne)"@en ;
  dcterms:title "ASLS Landform classifiers" ;
  rdfs:seeAlso <http://www.publish.csiro.au/nid/22/pid/5230.htm> ;
  rdfs:seeAlso <https://www.publish.csiro.au/book/5230> ;
  owl:imports dc: ;
  owl:imports sosa: ;
  skos:changeNote "2020-09-16 - made asls:landform a skos:ConceptScheme and added skos:inScheme link from all concepts" ;
  skos:changeNote "2022-07-26 - removed dcterms:description and rdfs:label - duplicates skos:definition andskos:prefLabel" ;
  skos:editorialNote "<p>The data was converted from the print representation to this linked-data form by <a href='https://orcid.org/0000-0002-0693-1899'>Linda Gregory</a> and <a href='https://orcid.org/0000-0002-3884-3420'>Simon J D Cox</a></p>"^^rdf:HTML ;
  skos:hasTopConcept lf:element-dimension-height ;
  skos:hasTopConcept lf:element-dimension-length ;
  skos:hasTopConcept lf:element-dimension-width ;
  skos:hasTopConcept lf:geomorphological-agent-BI ;
  skos:hasTopConcept lf:geomorphological-agent-CH ;
  skos:hasTopConcept lf:geomorphological-agent-DI ;
  skos:hasTopConcept lf:geomorphological-agent-EU ;
  skos:hasTopConcept lf:geomorphological-agent-FR ;
  skos:hasTopConcept lf:geomorphological-agent-GL ;
  skos:hasTopConcept lf:geomorphological-agent-GR ;
  skos:hasTopConcept lf:geomorphological-agent-HU ;
  skos:hasTopConcept lf:geomorphological-agent-IM ;
  skos:hasTopConcept lf:geomorphological-agent-OV ;
  skos:hasTopConcept lf:geomorphological-agent-SH ;
  skos:hasTopConcept lf:geomorphological-agent-SM ;
  skos:hasTopConcept lf:geomorphological-agent-SO ;
  skos:hasTopConcept lf:geomorphological-agent-TI ;
  skos:hasTopConcept lf:geomorphological-agent-VO ;
  skos:hasTopConcept lf:geomorphological-agent-WA ;
  skos:hasTopConcept lf:geomorphological-agent-WI ;
  skos:hasTopConcept lf:geomorphological-agent-WM ;
  skos:hasTopConcept lf:landform-element-ALC ;
  skos:hasTopConcept lf:landform-element-BAN ;
  skos:hasTopConcept lf:landform-element-BAR ;
  skos:hasTopConcept lf:landform-element-BEA ;
  skos:hasTopConcept lf:landform-element-BEN ;
  skos:hasTopConcept lf:landform-element-BER ;
  skos:hasTopConcept lf:landform-element-BKP ;
  skos:hasTopConcept lf:landform-element-BOU ;
  skos:hasTopConcept lf:landform-element-BRI ;
  skos:hasTopConcept lf:landform-element-BRK ;
  skos:hasTopConcept lf:landform-element-CBE ;
  skos:hasTopConcept lf:landform-element-CFS ;
  skos:hasTopConcept lf:landform-element-CIR ;
  skos:hasTopConcept lf:landform-element-CLI ;
  skos:hasTopConcept lf:landform-element-CON ;
  skos:hasTopConcept lf:landform-element-COS ;
  skos:hasTopConcept lf:landform-element-CRA ;
  skos:hasTopConcept lf:landform-element-CUT ;
  skos:hasTopConcept lf:landform-element-DAM ;
  skos:hasTopConcept lf:landform-element-DBA ;
  skos:hasTopConcept lf:landform-element-DDE ;
  skos:hasTopConcept lf:landform-element-DOC ;
  skos:hasTopConcept lf:landform-element-DOL ;
  skos:hasTopConcept lf:landform-element-DUB ;
  skos:hasTopConcept lf:landform-element-DUC ;
  skos:hasTopConcept lf:landform-element-DUF ;
  skos:hasTopConcept lf:landform-element-DUH ;
  skos:hasTopConcept lf:landform-element-DUN ;
  skos:hasTopConcept lf:landform-element-DUP ;
  skos:hasTopConcept lf:landform-element-DUS ;
  skos:hasTopConcept lf:landform-element-EMB ;
  skos:hasTopConcept lf:landform-element-EST ;
  skos:hasTopConcept lf:landform-element-FAN ;
  skos:hasTopConcept lf:landform-element-FIL ;
  skos:hasTopConcept lf:landform-element-FLD ;
  skos:hasTopConcept lf:landform-element-FOO ;
  skos:hasTopConcept lf:landform-element-FOR ;
  skos:hasTopConcept lf:landform-element-GUL ;
  skos:hasTopConcept lf:landform-element-HCR ;
  skos:hasTopConcept lf:landform-element-HSL ;
  skos:hasTopConcept lf:landform-element-ITF ;
  skos:hasTopConcept lf:landform-element-LAG ;
  skos:hasTopConcept lf:landform-element-LAK ;
  skos:hasTopConcept lf:landform-element-LDS ;
  skos:hasTopConcept lf:landform-element-LEV ;
  skos:hasTopConcept lf:landform-element-LUN ;
  skos:hasTopConcept lf:landform-element-MAA ;
  skos:hasTopConcept lf:landform-element-MOU ;
  skos:hasTopConcept lf:landform-element-OXB ;
  skos:hasTopConcept lf:landform-element-PED ;
  skos:hasTopConcept lf:landform-element-PIT ;
  skos:hasTopConcept lf:landform-element-PLA ;
  skos:hasTopConcept lf:landform-element-PLY ;
  skos:hasTopConcept lf:landform-element-PST ;
  skos:hasTopConcept lf:landform-element-REC ;
  skos:hasTopConcept lf:landform-element-REF ;
  skos:hasTopConcept lf:landform-element-RER ;
  skos:hasTopConcept lf:landform-element-RES ;
  skos:hasTopConcept lf:landform-element-RFL ;
  skos:hasTopConcept lf:landform-element-RPL ;
  skos:hasTopConcept lf:landform-element-SCA ;
  skos:hasTopConcept lf:landform-element-SCD ;
  skos:hasTopConcept lf:landform-element-SCR ;
  skos:hasTopConcept lf:landform-element-SFS ;
  skos:hasTopConcept lf:landform-element-SRP ;
  skos:hasTopConcept lf:landform-element-STB ;
  skos:hasTopConcept lf:landform-element-STC ;
  skos:hasTopConcept lf:landform-element-STF ;
  skos:hasTopConcept lf:landform-element-SUS ;
  skos:hasTopConcept lf:landform-element-SWL ;
  skos:hasTopConcept lf:landform-element-SWP ;
  skos:hasTopConcept lf:landform-element-TAL ;
  skos:hasTopConcept lf:landform-element-TDC ;
  skos:hasTopConcept lf:landform-element-TDF ;
  skos:hasTopConcept lf:landform-element-TEF ;
  skos:hasTopConcept lf:landform-element-TEP ;
  skos:hasTopConcept lf:landform-element-TOR ;
  skos:hasTopConcept lf:landform-element-TRE ;
  skos:hasTopConcept lf:landform-element-TUM ;
  skos:hasTopConcept lf:landform-element-VLF ;
  skos:hasTopConcept lf:landform-pattern-ALF ;
  skos:hasTopConcept lf:landform-pattern-ALP ;
  skos:hasTopConcept lf:landform-pattern-ANA ;
  skos:hasTopConcept lf:landform-pattern-BAD ;
  skos:hasTopConcept lf:landform-pattern-BAR ;
  skos:hasTopConcept lf:landform-pattern-BEA ;
  skos:hasTopConcept lf:landform-pattern-CAL ;
  skos:hasTopConcept lf:landform-pattern-CHE ;
  skos:hasTopConcept lf:landform-pattern-COR ;
  skos:hasTopConcept lf:landform-pattern-COV ;
  skos:hasTopConcept lf:landform-pattern-DEL ;
  skos:hasTopConcept lf:landform-pattern-DUN ;
  skos:hasTopConcept lf:landform-pattern-ESC ;
  skos:hasTopConcept lf:landform-pattern-FLO ;
  skos:hasTopConcept lf:landform-pattern-HIL ;
  skos:hasTopConcept lf:landform-pattern-KAR ;
  skos:hasTopConcept lf:landform-pattern-LAC ;
  skos:hasTopConcept lf:landform-pattern-LAV ;
  skos:hasTopConcept lf:landform-pattern-LON ;
  skos:hasTopConcept lf:landform-pattern-LOW ;
  skos:hasTopConcept lf:landform-pattern-MAD ;
  skos:hasTopConcept lf:landform-pattern-MAR ;
  skos:hasTopConcept lf:landform-pattern-MEA ;
  skos:hasTopConcept lf:landform-pattern-MET ;
  skos:hasTopConcept lf:landform-pattern-MOU ;
  skos:hasTopConcept lf:landform-pattern-PAR ;
  skos:hasTopConcept lf:landform-pattern-PED ;
  skos:hasTopConcept lf:landform-pattern-PEP ;
  skos:hasTopConcept lf:landform-pattern-PLA ;
  skos:hasTopConcept lf:landform-pattern-PLT ;
  skos:hasTopConcept lf:landform-pattern-PLY ;
  skos:hasTopConcept lf:landform-pattern-PNP ;
  skos:hasTopConcept lf:landform-pattern-RIS ;
  skos:hasTopConcept lf:landform-pattern-SAN ;
  skos:hasTopConcept lf:landform-pattern-SHF ;
  skos:hasTopConcept lf:landform-pattern-STA ;
  skos:hasTopConcept lf:landform-pattern-TEL ;
  skos:hasTopConcept lf:landform-pattern-TER ;
  skos:hasTopConcept lf:landform-pattern-TID ;
  skos:hasTopConcept lf:landform-pattern-VOL ;
  skos:hasTopConcept lf:location-within-the-landform-element-B ;
  skos:hasTopConcept lf:location-within-the-landform-element-M ;
  skos:hasTopConcept lf:location-within-the-landform-element-T ;
  skos:hasTopConcept lf:location-within-toposequence ;
  skos:hasTopConcept lf:mode-of-geomorphological-activity-AG ;
  skos:hasTopConcept lf:mode-of-geomorphological-activity-BU ;
  skos:hasTopConcept lf:mode-of-geomorphological-activity-EA ;
  skos:hasTopConcept lf:mode-of-geomorphological-activity-ER ;
  skos:hasTopConcept lf:mode-of-geomorphological-activity-EX ;
  skos:hasTopConcept lf:mode-of-geomorphological-activity-HU ;
  skos:hasTopConcept lf:mode-of-geomorphological-activity-SU ;
  skos:hasTopConcept lf:morphological-type-C ;
  skos:hasTopConcept lf:morphological-type-D ;
  skos:hasTopConcept lf:morphological-type-F ;
  skos:hasTopConcept lf:morphological-type-H ;
  skos:hasTopConcept lf:morphological-type-L ;
  skos:hasTopConcept lf:morphological-type-LA ;
  skos:hasTopConcept lf:morphological-type-LI ;
  skos:hasTopConcept lf:morphological-type-LN ;
  skos:hasTopConcept lf:morphological-type-LX ;
  skos:hasTopConcept lf:morphological-type-M ;
  skos:hasTopConcept lf:morphological-type-MA ;
  skos:hasTopConcept lf:morphological-type-MI ;
  skos:hasTopConcept lf:morphological-type-MN ;
  skos:hasTopConcept lf:morphological-type-MX ;
  skos:hasTopConcept lf:morphological-type-R ;
  skos:hasTopConcept lf:morphological-type-S ;
  skos:hasTopConcept lf:morphological-type-U ;
  skos:hasTopConcept lf:morphological-type-UA ;
  skos:hasTopConcept lf:morphological-type-UI ;
  skos:hasTopConcept lf:morphological-type-UN ;
  skos:hasTopConcept lf:morphological-type-UX ;
  skos:hasTopConcept lf:morphological-type-V ;
  skos:hasTopConcept lf:relative-inclination-of-slope-elements-A ;
  skos:hasTopConcept lf:relative-inclination-of-slope-elements-I ;
  skos:hasTopConcept lf:relative-inclination-of-slope-elements-N ;
  skos:hasTopConcept lf:relative-inclination-of-slope-elements-X ;
  skos:hasTopConcept lf:relief-class-H ;
  skos:hasTopConcept lf:relief-class-L ;
  skos:hasTopConcept lf:relief-class-M ;
  skos:hasTopConcept lf:relief-class-P ;
  skos:hasTopConcept lf:relief-class-R ;
  skos:hasTopConcept lf:simple-erosional-landform-pattern-B ;
  skos:hasTopConcept lf:simple-erosional-landform-pattern-GP ;
  skos:hasTopConcept lf:simple-erosional-landform-pattern-GR ;
  skos:hasTopConcept lf:simple-erosional-landform-pattern-LP ;
  skos:hasTopConcept lf:simple-erosional-landform-pattern-PH ;
  skos:hasTopConcept lf:simple-erosional-landform-pattern-PM ;
  skos:hasTopConcept lf:simple-erosional-landform-pattern-RH ;
  skos:hasTopConcept lf:simple-erosional-landform-pattern-RL ;
  skos:hasTopConcept lf:simple-erosional-landform-pattern-RM ;
  skos:hasTopConcept lf:simple-erosional-landform-pattern-RP ;
  skos:hasTopConcept lf:simple-erosional-landform-pattern-RR ;
  skos:hasTopConcept lf:simple-erosional-landform-pattern-SH ;
  skos:hasTopConcept lf:simple-erosional-landform-pattern-SL ;
  skos:hasTopConcept lf:simple-erosional-landform-pattern-SM ;
  skos:hasTopConcept lf:simple-erosional-landform-pattern-SR ;
  skos:hasTopConcept lf:simple-erosional-landform-pattern-UH ;
  skos:hasTopConcept lf:simple-erosional-landform-pattern-UL ;
  skos:hasTopConcept lf:simple-erosional-landform-pattern-UP ;
  skos:hasTopConcept lf:simple-erosional-landform-pattern-UR ;
  skos:hasTopConcept lf:simple-erosional-landform-pattern-VH ;
  skos:hasTopConcept lf:simple-erosional-landform-pattern-VL ;
  skos:hasTopConcept lf:simple-erosional-landform-pattern-VM ;
  skos:hasTopConcept lf:slope-class-CL ;
  skos:hasTopConcept lf:slope-class-GE ;
  skos:hasTopConcept lf:slope-class-LE ;
  skos:hasTopConcept lf:slope-class-MO ;
  skos:hasTopConcept lf:slope-class-PR ;
  skos:hasTopConcept lf:slope-class-ST ;
  skos:hasTopConcept lf:slope-class-VG ;
  skos:hasTopConcept lf:slope-class-VS ;
  skos:hasTopConcept lf:slope-evaluation-A ;
  skos:hasTopConcept lf:slope-evaluation-E ;
  skos:hasTopConcept lf:slope-evaluation-P ;
  skos:hasTopConcept lf:slope-evaluation-T ;
  skos:hasTopConcept lf:slope-value ;
  skos:hasTopConcept lf:stream-channel-development-A ;
  skos:hasTopConcept lf:stream-channel-development-E ;
  skos:hasTopConcept lf:stream-channel-development-I ;
  skos:hasTopConcept lf:stream-channel-development-O ;
  skos:hasTopConcept lf:stream-channel-migration-F ;
  skos:hasTopConcept lf:stream-channel-migration-R ;
  skos:hasTopConcept lf:stream-channel-migration-S ;
  skos:hasTopConcept lf:stream-channel-network-directionality-B ;
  skos:hasTopConcept lf:stream-channel-network-directionality-C ;
  skos:hasTopConcept lf:stream-channel-network-directionality-D ;
  skos:hasTopConcept lf:stream-channel-network-directionality-F ;
  skos:hasTopConcept lf:stream-channel-network-directionality-N ;
  skos:hasTopConcept lf:stream-channel-network-directionality-P ;
  skos:hasTopConcept lf:stream-channel-network-directionality-U ;
  skos:hasTopConcept lf:stream-channel-network-integration-D ;
  skos:hasTopConcept lf:stream-channel-network-integration-I ;
  skos:hasTopConcept lf:stream-channel-network-integration-P ;
  skos:hasTopConcept lf:stream-channel-relative-depth-width-D ;
  skos:hasTopConcept lf:stream-channel-relative-depth-width-M ;
  skos:hasTopConcept lf:stream-channel-relative-depth-width-S ;
  skos:hasTopConcept lf:stream-channel-relative-depth-width-V ;
  skos:hasTopConcept lf:stream-channel-spacing-AB ;
  skos:hasTopConcept lf:stream-channel-spacing-CS ;
  skos:hasTopConcept lf:stream-channel-spacing-MS ;
  skos:hasTopConcept lf:stream-channel-spacing-NU ;
  skos:hasTopConcept lf:stream-channel-spacing-SP ;
  skos:hasTopConcept lf:stream-channel-spacing-VC ;
  skos:hasTopConcept lf:stream-channel-spacing-VW ;
  skos:hasTopConcept lf:stream-channel-spacing-WS ;
  skos:hasTopConcept lf:streamwise-channel-pattern-D ;
  skos:hasTopConcept lf:streamwise-channel-pattern-N ;
  skos:hasTopConcept lf:streamwise-channel-pattern-R ;
  skos:hasTopConcept lf:streamwise-channel-pattern-T ;
  skos:prefLabel "ASLS Landform classifiers"@en ;
.
lf:compound-morphological-types
  a skos:Collection ;
  dcterms:identifier "http://anzsoil.org/def/au/asls/landform/compound-morphological-types"^^xsd:anyURI ;
  skos:definition "Several types of landform feature have crests and adjoining slopes that are so small that a 20 m radius site would usually include both. Two compound morphological types are distinguished by the relative length of the crest: Hillock and Ridge"@en ;
  skos:member lf:morphological-type-H ;
  skos:member lf:morphological-type-R ;
  skos:prefLabel "Compound morphological types"@en ;
.
lf:element-dimension-height
  a skos:Concept ;
  a sosa:ObservableProperty ;
  skos-ext:isMemberOf lf:element-dimensions ;
  dcterms:identifier "http://anzsoil.org/def/au/asls/landform/element-dimension-height"^^xsd:anyURI ;
  skos:altLabel "Depth of landform element"@en ;
  skos:definition "difference in elevation between the upper and lower margins of the element, measured along any slope line. Height can mean quite different things and must be carefully defined. For crests, ridges and hillocks, define the upper margin as the point where the selected slope line coalesces with others to form the ridge line. For depressions, define the lower margin as the point where the selected slope line coalesces with others to form the course line."@en ;
  skos:inScheme asls:landform ;
  skos:prefLabel "Height of landform element"@en ;
  skos:topConceptOf asls:landform ;
.
lf:element-dimension-length
  a skos:Concept ;
  a sosa:ObservableProperty ;
  skos-ext:isMemberOf lf:element-dimensions ;
  dcterms:identifier "http://anzsoil.org/def/au/asls/landform/element-dimension-length"^^xsd:anyURI ;
  skos:definition "horizontal distance between the upper and lower margins of the element, measured down a slope line. For crests, the slope line to be used is the ridge line; for depressions, the course line (see Figure 2a). By this definition, many crests and open depressions become very long."@en ;
  skos:inScheme asls:landform ;
  skos:prefLabel "Length of landform element"@en ;
  skos:topConceptOf asls:landform ;
.
lf:element-dimension-width
  a skos:Concept ;
  a sosa:ObservableProperty ;
  skos-ext:isMemberOf lf:element-dimensions ;
  dcterms:identifier "http://anzsoil.org/def/au/asls/landform/element-dimension-width"^^xsd:anyURI ;
  skos:definition "horizontal distance between the lateral margins of the element, measured perpendicularly to the length."@en ;
  skos:inScheme asls:landform ;
  skos:prefLabel "Width of landform element"@en ;
  skos:topConceptOf asls:landform ;
.
lf:element-dimensions
  a skos:Collection ;
  dcterms:identifier "http://anzsoil.org/def/au/asls/landform/element-dimensions"^^xsd:anyURI ;
  skos:definition "An occurrence of a landform element extends as far as its attributes remain constant. Its dimensions, which may be much greater than the specified sample area diameter of 40 m, can be significant to land use. Terms referring to dimension appear often in the definitions of landform element types. Three dimensions are distinguished, each to be expressed in metres: Length, Width, Height (or depth)."@en ;
  skos:member lf:element-dimension-height ;
  skos:member lf:element-dimension-length ;
  skos:member lf:element-dimension-width ;
  skos:prefLabel "Dimensions of landform element"@en ;
.
lf:geomorphological-agent-BI
  a skos:Concept ;
  skos-ext:isMemberOf lf:geomorphological-agents ;
  dcterms:identifier "http://anzsoil.org/def/au/asls/landform/geomorphological-agent-BI"^^xsd:anyURI ;
  rdfs:comment "Biological agent"@en ;
  skos:definition "Non-human biological agents; coral (Biological agents)."@en ;
  skos:inScheme asls:landform ;
  skos:notation "BI" ;
  skos:prefLabel "Non-human biological agents"@en ;
  skos:topConceptOf asls:landform ;
.
lf:geomorphological-agent-CH
  a skos:Concept ;
  skos-ext:isMemberOf lf:geomorphological-agents ;
  dcterms:identifier "http://anzsoil.org/def/au/asls/landform/geomorphological-agent-CH"^^xsd:anyURI ;
  rdfs:comment "Stream flow"@en ;
  skos:definition "Channelled stream flow (Stream flow)."@en ;
  skos:inScheme asls:landform ;
  skos:notation "CH" ;
  skos:prefLabel "Channelled stream flow"@en ;
  skos:topConceptOf asls:landform ;
.
lf:geomorphological-agent-DI
  a skos:Concept ;
  skos-ext:isMemberOf lf:geomorphological-agents ;
  dcterms:identifier "http://anzsoil.org/def/au/asls/landform/geomorphological-agent-DI"^^xsd:anyURI ;
  rdfs:comment "Internal forces"@en ;
  skos:definition "Diastrophism; earth movements (Internal forces)."@en ;
  skos:inScheme asls:landform ;
  skos:notation "DI" ;
  skos:prefLabel "Diastrophism"@en ;
  skos:topConceptOf asls:landform ;
.
lf:geomorphological-agent-EU
  a skos:Concept ;
  skos-ext:isMemberOf lf:geomorphological-agents ;
  dcterms:identifier "http://anzsoil.org/def/au/asls/landform/geomorphological-agent-EU"^^xsd:anyURI ;
  rdfs:comment "Standing water"@en ;
  skos:definition "Eustasy; changes in sea level (Standing water)."@en ;
  skos:inScheme asls:landform ;
  skos:notation "EU" ;
  skos:prefLabel "Eustasy"@en ;
  skos:topConceptOf asls:landform ;
.
lf:geomorphological-agent-FR
  a skos:Concept ;
  skos-ext:isMemberOf lf:geomorphological-agents ;
  dcterms:identifier "http://anzsoil.org/def/au/asls/landform/geomorphological-agent-FR"^^xsd:anyURI ;
  rdfs:comment "Ice"@en ;
  skos:definition "Frost (Ice)."@en ;
  skos:inScheme asls:landform ;
  skos:notation "FR" ;
  skos:prefLabel "Frost"@en ;
  skos:topConceptOf asls:landform ;
.
lf:geomorphological-agent-GL
  a skos:Concept ;
  skos-ext:isMemberOf lf:geomorphological-agents ;
  dcterms:identifier "http://anzsoil.org/def/au/asls/landform/geomorphological-agent-GL"^^xsd:anyURI ;
  rdfs:comment "Ice"@en ;
  skos:definition "Glacier flow (Ice)."@en ;
  skos:inScheme asls:landform ;
  skos:notation "GL" ;
  skos:prefLabel "Glacier flow"@en ;
  skos:topConceptOf asls:landform ;
.
lf:geomorphological-agent-GR
  a skos:Concept ;
  skos-ext:isMemberOf lf:geomorphological-agents ;
  dcterms:identifier "http://anzsoil.org/def/au/asls/landform/geomorphological-agent-GR"^^xsd:anyURI ;
  rdfs:comment "Gravity"@en ;
  skos:definition "Collapse, or particle fall."@en ;
  skos:inScheme asls:landform ;
  skos:notation "GR" ;
  skos:prefLabel "Gravity"@en ;
  skos:topConceptOf asls:landform ;
.
lf:geomorphological-agent-HU
  a skos:Concept ;
  skos-ext:isMemberOf lf:geomorphological-agents ;
  dcterms:identifier "http://anzsoil.org/def/au/asls/landform/geomorphological-agent-HU"^^xsd:anyURI ;
  rdfs:comment "Biological agents"@en ;
  skos:definition "Human agents (Biological agents)."@en ;
  skos:inScheme asls:landform ;
  skos:notation "HU" ;
  skos:prefLabel "Human agents"@en ;
  skos:topConceptOf asls:landform ;
.
lf:geomorphological-agent-IM
  a skos:Concept ;
  skos-ext:isMemberOf lf:geomorphological-agents ;
  dcterms:identifier "http://anzsoil.org/def/au/asls/landform/geomorphological-agent-IM"^^xsd:anyURI ;
  rdfs:comment "Extraterrestrial agents"@en ;
  skos:definition "Impact by meteors (Extraterrestrial agents)."@en ;
  skos:inScheme asls:landform ;
  skos:notation "IM" ;
  skos:prefLabel "Impact by meteors"@en ;
  skos:topConceptOf asls:landform ;
.
lf:geomorphological-agent-OV
  a skos:Concept ;
  skos-ext:isMemberOf lf:geomorphological-agents ;
  dcterms:identifier "http://anzsoil.org/def/au/asls/landform/geomorphological-agent-OV"^^xsd:anyURI ;
  rdfs:comment "Stream flow"@en ;
  skos:definition "Overbank stream flow, unchannelled (Stream flow)."@en ;
  skos:inScheme asls:landform ;
  skos:notation "OV" ;
  skos:prefLabel "Overbank stream flow, unchannelled"@en ;
  skos:topConceptOf asls:landform ;
.
lf:geomorphological-agent-SH
  a skos:Concept ;
  skos-ext:isMemberOf lf:geomorphological-agents ;
  dcterms:identifier "http://anzsoil.org/def/au/asls/landform/geomorphological-agent-SH"^^xsd:anyURI ;
  rdfs:comment "Precipitation"@en ;
  skos:definition "Sheet flow, sheet wash, surface wash (Precipitation)."@en ;
  skos:inScheme asls:landform ;
  skos:notation "SH" ;
  skos:prefLabel "Sheet flow, sheet wash, surface wash"@en ;
  skos:topConceptOf asls:landform ;
.
lf:geomorphological-agent-SM
  a skos:Concept ;
  skos-ext:isMemberOf lf:geomorphological-agents ;
  dcterms:identifier "http://anzsoil.org/def/au/asls/landform/geomorphological-agent-SM"^^xsd:anyURI ;
  rdfs:comment "Precipitation"@en ;
  skos:definition "Soil moisture status changes; creep (Precipitation)."@en ;
  skos:inScheme asls:landform ;
  skos:notation "SM" ;
  skos:prefLabel "Soil moisture status changes"@en ;
  skos:topConceptOf asls:landform ;
.
lf:geomorphological-agent-SO
  a skos:Concept ;
  skos-ext:isMemberOf lf:geomorphological-agents ;
  dcterms:identifier "http://anzsoil.org/def/au/asls/landform/geomorphological-agent-SO"^^xsd:anyURI ;
  rdfs:comment "Precipitation"@en ;
  skos:definition "Solution (Precipitation)."@en ;
  skos:inScheme asls:landform ;
  skos:notation "SO" ;
  skos:prefLabel "Solution"@en ;
  skos:topConceptOf asls:landform ;
.
lf:geomorphological-agent-TI
  a skos:Concept ;
  skos-ext:isMemberOf lf:geomorphological-agents ;
  dcterms:identifier "http://anzsoil.org/def/au/asls/landform/geomorphological-agent-TI"^^xsd:anyURI ;
  rdfs:comment "Standing water"@en ;
  skos:definition "Tides (Standing water)."@en ;
  skos:inScheme asls:landform ;
  skos:notation "TI" ;
  skos:prefLabel "Tides"@en ;
  skos:topConceptOf asls:landform ;
.
lf:geomorphological-agent-VO
  a skos:Concept ;
  skos-ext:isMemberOf lf:geomorphological-agents ;
  dcterms:identifier "http://anzsoil.org/def/au/asls/landform/geomorphological-agent-VO"^^xsd:anyURI ;
  rdfs:comment "Internal forces"@en ;
  skos:definition "Volcanism (Internal forces)."@en ;
  skos:inScheme asls:landform ;
  skos:notation "VO" ;
  skos:prefLabel "Volcanism"@en ;
  skos:topConceptOf asls:landform ;
.
lf:geomorphological-agent-WA
  a skos:Concept ;
  skos-ext:isMemberOf lf:geomorphological-agents ;
  dcterms:identifier "http://anzsoil.org/def/au/asls/landform/geomorphological-agent-WA"^^xsd:anyURI ;
  rdfs:comment "Standing water"@en ;
  skos:definition "Waves (Standing water)."@en ;
  skos:inScheme asls:landform ;
  skos:notation "WA" ;
  skos:prefLabel "Waves"@en ;
  skos:topConceptOf asls:landform ;
.
lf:geomorphological-agent-WI
  a skos:Concept ;
  skos-ext:isMemberOf lf:geomorphological-agents ;
  dcterms:identifier "http://anzsoil.org/def/au/asls/landform/geomorphological-agent-WI"^^xsd:anyURI ;
  rdfs:comment "Wind"@en ;
  skos:definition "Wind (Wind)."@en ;
  skos:inScheme asls:landform ;
  skos:notation "WI" ;
  skos:prefLabel "Wind"@en ;
  skos:topConceptOf asls:landform ;
.
lf:geomorphological-agent-WM
  a skos:Concept ;
  skos-ext:isMemberOf lf:geomorphological-agents ;
  dcterms:identifier "http://anzsoil.org/def/au/asls/landform/geomorphological-agent-WM"^^xsd:anyURI ;
  rdfs:comment "Precipitation"@en ;
  skos:definition "Water-aided mass movements; landslides (Precipitation)."@en ;
  skos:inScheme asls:landform ;
  skos:notation "WM" ;
  skos:prefLabel "Water-aided mass movements"@en ;
  skos:topConceptOf asls:landform ;
.
lf:geomorphological-agents
  a skos:Collection ;
  a sosa:ObservableProperty ;
  dcterms:identifier "http://anzsoil.org/def/au/asls/landform/geomorphological-agents"^^xsd:anyURI ;
  skos:definition "Geomorphological agents that play a role in producing distinctive landform elements."@en ;
  skos:member lf:geomorphological-agent-BI ;
  skos:member lf:geomorphological-agent-CH ;
  skos:member lf:geomorphological-agent-DI ;
  skos:member lf:geomorphological-agent-EU ;
  skos:member lf:geomorphological-agent-FR ;
  skos:member lf:geomorphological-agent-GL ;
  skos:member lf:geomorphological-agent-GR ;
  skos:member lf:geomorphological-agent-HU ;
  skos:member lf:geomorphological-agent-IM ;
  skos:member lf:geomorphological-agent-OV ;
  skos:member lf:geomorphological-agent-SH ;
  skos:member lf:geomorphological-agent-SM ;
  skos:member lf:geomorphological-agent-SO ;
  skos:member lf:geomorphological-agent-TI ;
  skos:member lf:geomorphological-agent-VO ;
  skos:member lf:geomorphological-agent-WA ;
  skos:member lf:geomorphological-agent-WI ;
  skos:member lf:geomorphological-agent-WM ;
  skos:prefLabel "Geomorphological agent values"@en ;
.
lf:landform-element-ALC
  a skos:Concept ;
  skos-ext:isMemberOf lf:landform-element-glossary ;
  dcterms:identifier "http://anzsoil.org/def/au/asls/landform/landform-element-ALC"^^xsd:anyURI ;
  skos:definition "moderately inclined to very steep, short open depression with concave cross-section, eroded by collapse, landslides, creep or surface wash."@en ;
  skos:inScheme asls:landform ;
  skos:notation "ALC" ;
  skos:prefLabel "Alcove"@en ;
  skos:topConceptOf asls:landform ;
.
lf:landform-element-BAN
  a skos:Concept ;
  skos-ext:isMemberOf lf:landform-element-glossary ;
  dcterms:identifier "http://anzsoil.org/def/au/asls/landform/landform-element-BAN"^^xsd:anyURI ;
  skos:definition "very short, very wide slope, moderately inclined to precipitous, forming the marginal upper parts of a stream channel and resulting from erosion or aggradation by channelled stream flow."@en ;
  skos:inScheme asls:landform ;
  skos:notation "BAN" ;
  skos:prefLabel "Bank (stream bank)"@en ;
  skos:topConceptOf asls:landform ;
.
lf:landform-element-BAR
  a skos:Concept ;
  skos-ext:isMemberOf lf:landform-element-glossary ;
  dcterms:identifier "http://anzsoil.org/def/au/asls/landform/landform-element-BAR"^^xsd:anyURI ;
  skos:definition "elongated, gently to moderately inclined, low ridge built up by channelled stream flow; part of a stream bed."@en ;
  skos:inScheme asls:landform ;
  skos:notation "BAR" ;
  skos:prefLabel "Bar (stream bar)"@en ;
  skos:topConceptOf asls:landform ;
.
lf:landform-element-BEA
  a skos:Concept ;
  skos-ext:isMemberOf lf:landform-element-glossary ;
  dcterms:identifier "http://anzsoil.org/def/au/asls/landform/landform-element-BEA"^^xsd:anyURI ;
  skos:definition "short, low, very wide slope, gently or moderately inclined, built up or eroded by waves, forming the shore of a lake or sea."@en ;
  skos:inScheme asls:landform ;
  skos:notation "BEA" ;
  skos:prefLabel "Beach"@en ;
  skos:topConceptOf asls:landform ;
.
lf:landform-element-BEN
  a skos:Concept ;
  skos-ext:isMemberOf lf:landform-element-glossary ;
  dcterms:identifier "http://anzsoil.org/def/au/asls/landform/landform-element-BEN"^^xsd:anyURI ;
  skos:definition "short, low, very wide slope, gently or moderately inclined, built up or eroded by waves, forming the shore of a lake or sea."@en ;
  skos:inScheme asls:landform ;
  skos:notation "BEN" ;
  skos:prefLabel "Bench"@en ;
  skos:topConceptOf asls:landform ;
.
lf:landform-element-BER
  a skos:Concept ;
  skos-ext:isMemberOf lf:landform-element-glossary ;
  dcterms:identifier "http://anzsoil.org/def/au/asls/landform/landform-element-BER"^^xsd:anyURI ;
  skos:definition "(i) short, very gently inclined to level minimal mid-slope in an embankment or cut face, eroded or aggraded by human activity. (ii) flat built up by waves above a beach."@en ;
  skos:inScheme asls:landform ;
  skos:notation "BER" ;
  skos:prefLabel "Berm"@en ;
  skos:topConceptOf asls:landform ;
.
lf:landform-element-BKP
  a skos:Concept ;
  skos-ext:isMemberOf lf:landform-element-glossary ;
  dcterms:identifier "http://anzsoil.org/def/au/asls/landform/landform-element-BKP"^^xsd:anyURI ;
  skos:definition "very long, low, narrow, nearly level, sinuous ridge immediately adjacent to a stream channel, built up by overbank flow. Levees are built, usually in pairs bounding the two sides of a stream channel, at the level reached by frequent floods. This element is part of a covered plain landform pattern. For an artificial levee, use Embankment. See also Prior stream."@en ;
  skos:inScheme asls:landform ;
  skos:notation "BKP" ;
  skos:prefLabel "Backplain"@en ;
  skos:topConceptOf asls:landform ;
.
lf:landform-element-BOU
  a skos:Concept ;
  skos-ext:isMemberOf lf:landform-element-glossary ;
  dcterms:identifier "http://anzsoil.org/def/au/asls/landform/landform-element-BOU"^^xsd:anyURI ;
  skos:definition "usually small, open or closed depression excavated by the wind."@en ;
  skos:inScheme asls:landform ;
  skos:notation "BOU" ;
  skos:prefLabel "Blow-out"@en ;
  skos:topConceptOf asls:landform ;
.
lf:landform-element-BRI
  a skos:Concept ;
  skos-ext:isMemberOf lf:landform-element-glossary ;
  dcterms:identifier "http://anzsoil.org/def/au/asls/landform/landform-element-BRI"^^xsd:anyURI ;
  skos:definition "very long, nearly straight, low ridge, built up by waves and usually modified by wind. A beach ridge is often a relict feature remote from the beach."@en ;
  skos:inScheme asls:landform ;
  skos:notation "BRI" ;
  skos:prefLabel "Beach ridge"@en ;
  skos:topConceptOf asls:landform ;
.
lf:landform-element-BRK
  a skos:Concept ;
  skos-ext:isMemberOf lf:landform-element-glossary ;
  dcterms:identifier "http://anzsoil.org/def/au/asls/landform/landform-element-BRK"^^xsd:anyURI ;
  skos:definition "steep maximal mid-slope or upper slope, generally comprising both a very short scarp (free face) that is often bare rockland, and a stony scarp-footslope (debris slope); often standing above a pediment."@en ;
  skos:inScheme asls:landform ;
  skos:notation "BRK" ;
  skos:prefLabel "Breakaway"@en ;
  skos:topConceptOf asls:landform ;
.
lf:landform-element-CBE
  a skos:Concept ;
  skos-ext:isMemberOf lf:landform-element-glossary ;
  dcterms:identifier "http://anzsoil.org/def/au/asls/landform/landform-element-CBE"^^xsd:anyURI ;
  skos:definition "flat at the margin of a stream channel aggraded and in part eroded by over-bank and channelled stream flow; an incipient flood plain. Channel benches have been referred to as 'low terraces', but the term terrace should be restricted to landform patterns above the influence of active stream flow."@en ;
  skos:inScheme asls:landform ;
  skos:notation "CBE" ;
  skos:prefLabel "Channel bench"@en ;
  skos:topConceptOf asls:landform ;
.
lf:landform-element-CFS
  a skos:Concept ;
  skos-ext:isMemberOf lf:landform-element-glossary ;
  dcterms:identifier "http://anzsoil.org/def/au/asls/landform/landform-element-CFS"^^xsd:anyURI ;
  skos:definition "slope situated below a cliff, with its contours generally parallel to the line of the cliff, eroded by sheet wash or water-aided mass movement, and aggraded locally by collapsed material from above."@en ;
  skos:inScheme asls:landform ;
  skos:notation "CFS" ;
  skos:prefLabel "Cliff-footslope"@en ;
  skos:topConceptOf asls:landform ;
.
lf:landform-element-CIR
  a skos:Concept ;
  skos-ext:isMemberOf lf:landform-element-glossary ;
  dcterms:identifier "http://anzsoil.org/def/au/asls/landform/landform-element-CIR"^^xsd:anyURI ;
  skos:definition "precipitous to gently inclined, typically closed depression of concave contour and profile excavated by ice. The closed part of the depression may be shallow, the larger part being an open depression like an alcove."@en ;
  skos:inScheme asls:landform ;
  skos:notation "CIR" ;
  skos:prefLabel "Cirque"@en ;
  skos:topConceptOf asls:landform ;
.
lf:landform-element-CLI
  a skos:Concept ;
  skos-ext:isMemberOf lf:landform-element-glossary ;
  dcterms:identifier "http://anzsoil.org/def/au/asls/landform/landform-element-CLI"^^xsd:anyURI ;
  skos:definition "very wide, cliffed (greater than 72º) maximal slope usually eroded by gravitational fall as a result of erosion of the base by various agencies; sometimes built up by marine organisms (cf. scarp)."@en ;
  skos:inScheme asls:landform ;
  skos:notation "CLI" ;
  skos:prefLabel "Cliff"@en ;
  skos:topConceptOf asls:landform ;
.
lf:landform-element-CON
  a skos:Concept ;
  skos-ext:isMemberOf lf:landform-element-glossary ;
  dcterms:identifier "http://anzsoil.org/def/au/asls/landform/landform-element-CON"^^xsd:anyURI ;
  skos:definition "hillock with a circular symmetry built up by volcanism. The crest may form a ring around a crater."@en ;
  skos:inScheme asls:landform ;
  skos:notation "CON" ;
  skos:prefLabel "Cone (volcanic)"@en ;
  skos:topConceptOf asls:landform ;
.
lf:landform-element-COS
  a skos:Concept ;
  skos-ext:isMemberOf lf:landform-element-glossary ;
  dcterms:identifier "http://anzsoil.org/def/au/asls/landform/landform-element-COS"^^xsd:anyURI ;
  skos:definition "flat eroded by human activity."@en ;
  skos:inScheme asls:landform ;
  skos:notation "COS" ;
  skos:prefLabel "Cut-over surface"@en ;
  skos:topConceptOf asls:landform ;
.
lf:landform-element-CRA
  a skos:Concept ;
  skos-ext:isMemberOf lf:landform-element-glossary ;
  dcterms:identifier "http://anzsoil.org/def/au/asls/landform/landform-element-CRA"^^xsd:anyURI ;
  skos:definition "steep to precipitous closed depression excavated by explosions due to vulcanism, human action, or impact of an extraterrestrial object."@en ;
  skos:inScheme asls:landform ;
  skos:notation "CRA" ;
  skos:prefLabel "Crater"@en ;
  skos:topConceptOf asls:landform ;
.
lf:landform-element-CUT
  a skos:Concept ;
  skos-ext:isMemberOf lf:landform-element-glossary ;
  dcterms:identifier "http://anzsoil.org/def/au/asls/landform/landform-element-CUT"^^xsd:anyURI ;
  skos:definition "slope eroded by human activity."@en ;
  skos:inScheme asls:landform ;
  skos:notation "CUT" ;
  skos:prefLabel "Cut face"@en ;
  skos:topConceptOf asls:landform ;
.
lf:landform-element-DAM
  a skos:Concept ;
  skos-ext:isMemberOf lf:landform-element-glossary ;
  dcterms:identifier "http://anzsoil.org/def/au/asls/landform/landform-element-DAM"^^xsd:anyURI ;
  skos:definition "ridge built up by human activity so as to close a depression."@en ;
  skos:inScheme asls:landform ;
  skos:notation "DAM" ;
  skos:prefLabel "Dam"@en ;
  skos:topConceptOf asls:landform ;
.
lf:landform-element-DBA
  a skos:Concept ;
  skos-ext:isMemberOf lf:landform-element-glossary ;
  dcterms:identifier "http://anzsoil.org/def/au/asls/landform/landform-element-DBA"^^xsd:anyURI ;
  skos:definition "basin excavated by wind erosion which removes loose material, commonly above a resistant or wet layer."@en ;
  skos:inScheme asls:landform ;
  skos:notation "DBA" ;
  skos:prefLabel "Deflation basin"@en ;
  skos:topConceptOf asls:landform ;
.
lf:landform-element-DDE
  a skos:Concept ;
  skos-ext:isMemberOf lf:landform-element-glossary ;
  dcterms:identifier "http://anzsoil.org/def/au/asls/landform/landform-element-DDE"^^xsd:anyURI ;
  skos:definition "level to gently inclined, long, narrow, shallow open depression with smoothly concave cross-section, rising to moderately inclined side slopes, eroded or aggraded by sheet wash."@en ;
  skos:inScheme asls:landform ;
  skos:notation "DDE" ;
  skos:prefLabel "Drainage depression"@en ;
  skos:topConceptOf asls:landform ;
.
lf:landform-element-DOC
  a skos:Concept ;
  skos-ext:isMemberOf lf:landform-element-glossary ;
  dcterms:identifier "http://anzsoil.org/def/au/asls/landform/landform-element-DOC"^^xsd:anyURI ;
  skos:definition "steep-sided, circular or elliptical closed depression, commonly funnel-shaped, characterised by subsurface drainage and formed by collapse of underlying caves within bedrock."@en ;
  skos:inScheme asls:landform ;
  skos:notation "DOC" ;
  skos:prefLabel "Collapse doline"@en ;
  skos:topConceptOf asls:landform ;
.
lf:landform-element-DOL
  a skos:Concept ;
  skos-ext:isMemberOf lf:landform-element-glossary ;
  dcterms:identifier "http://anzsoil.org/def/au/asls/landform/landform-element-DOL"^^xsd:anyURI ;
  skos:definition "steep-sided, circular or elliptical closed depression, commonly funnel-shaped, characterised by subsurface drainage and formed by dissolution of the surface or underlying bedrock."@en ;
  skos:inScheme asls:landform ;
  skos:notation "DOL" ;
  skos:prefLabel "Solution doline"@en ;
  skos:topConceptOf asls:landform ;
.
lf:landform-element-DUB
  a skos:Concept ;
  skos-ext:isMemberOf lf:landform-element-glossary ;
  dcterms:identifier "http://anzsoil.org/def/au/asls/landform/landform-element-DUB"^^xsd:anyURI ;
  skos:definition "crescent-shaped dune with tips extending leeward (downwind), making this side concave and the windward (upwind) side convex. Barchan dunes tend to be arranged in chains extending in the dominant wind direction."@en ;
  skos:inScheme asls:landform ;
  skos:notation "DUB" ;
  skos:prefLabel "Barchan dune"@en ;
  skos:topConceptOf asls:landform ;
.
lf:landform-element-DUC
  a skos:Concept ;
  skos-ext:isMemberOf lf:landform-element-glossary ;
  dcterms:identifier "http://anzsoil.org/def/au/asls/landform/landform-element-DUC"^^xsd:anyURI ;
  skos:definition "crest built up or eroded by the wind (see dune)."@en ;
  skos:inScheme asls:landform ;
  skos:notation "DUC" ;
  skos:prefLabel "Dunecrest"@en ;
  skos:topConceptOf asls:landform ;
.
lf:landform-element-DUF
  a skos:Concept ;
  skos-ext:isMemberOf lf:landform-element-glossary ;
  dcterms:identifier "http://anzsoil.org/def/au/asls/landform/landform-element-DUF"^^xsd:anyURI ;
  skos:definition "large, sharp-crested, elongated, longitudinal (linear) dune or chain of sand dunes, oriented parallel, rather than transverse (perpendicular), to the prevailing wind. (Not to be confused with the trailing arms of parabolic dunes.)"@en ;
  skos:inScheme asls:landform ;
  skos:notation "DUF" ;
  skos:prefLabel "Linear or longitudinal (seif) dune"@en ;
  skos:topConceptOf asls:landform ;
.
lf:landform-element-DUH
  a skos:Concept ;
  skos-ext:isMemberOf lf:landform-element-glossary ;
  dcterms:identifier "http://anzsoil.org/def/au/asls/landform/landform-element-DUH"^^xsd:anyURI ;
  skos:definition "very gently to moderately inclined rises or hillocks built up or eroded by wind and lacking distinct orientation or regular pattern."@en ;
  skos:inScheme asls:landform ;
  skos:notation "DUH" ;
  skos:prefLabel "Hummocky (weakly oriented) dune"@en ;
  skos:topConceptOf asls:landform ;
.
lf:landform-element-DUN
  a skos:Concept ;
  skos-ext:isMemberOf lf:landform-element-glossary ;
  dcterms:identifier "http://anzsoil.org/def/au/asls/landform/landform-element-DUN"^^xsd:anyURI ;
  skos:definition "moderately inclined to very steep ridge or hillock built up by the wind. This element may comprise dunecrest and duneslope."@en ;
  skos:inScheme asls:landform ;
  skos:notation "DUN" ;
  skos:prefLabel "Dune"@en ;
  skos:topConceptOf asls:landform ;
.
lf:landform-element-DUP
  a skos:Concept ;
  skos-ext:isMemberOf lf:landform-element-glossary ;
  dcterms:identifier "http://anzsoil.org/def/au/asls/landform/landform-element-DUP"^^xsd:anyURI ;
  skos:definition "sand dune with a long, scoop-shaped form, convex in the downwind direction so that its horns point upwind, whose ground plan approximates the form of a parabola. The dunes left behind can be referred to as trailing arms. Where many such dunes have traversed an area, these can give the appearance of linear dunes."@en ;
  skos:inScheme asls:landform ;
  skos:notation "DUP" ;
  skos:prefLabel "Parabolic dune"@en ;
  skos:topConceptOf asls:landform ;
.
lf:landform-element-DUS
  a skos:Concept ;
  skos-ext:isMemberOf lf:landform-element-glossary ;
  dcterms:identifier "http://anzsoil.org/def/au/asls/landform/landform-element-DUS"^^xsd:anyURI ;
  skos:definition "slope built up or eroded by the wind (see dune)."@en ;
  skos:inScheme asls:landform ;
  skos:notation "DUS" ;
  skos:prefLabel "Duneslope"@en ;
  skos:topConceptOf asls:landform ;
.
lf:landform-element-EMB
  a skos:Concept ;
  skos-ext:isMemberOf lf:landform-element-glossary ;
  dcterms:identifier "http://anzsoil.org/def/au/asls/landform/landform-element-EMB"^^xsd:anyURI ;
  skos:definition "ridge or slope built up by human activity."@en ;
  skos:inScheme asls:landform ;
  skos:notation "EMB" ;
  skos:prefLabel "Embankment"@en ;
  skos:topConceptOf asls:landform ;
.
lf:landform-element-EST
  a skos:Concept ;
  skos-ext:isMemberOf lf:landform-element-glossary ;
  dcterms:identifier "http://anzsoil.org/def/au/asls/landform/landform-element-EST"^^xsd:anyURI ;
  skos:definition "stream channel close to its junction with a sea or lake, where the action of channelled stream flow is modified by tide and waves. The width typically increases downstream."@en ;
  skos:inScheme asls:landform ;
  skos:notation "EST" ;
  skos:prefLabel "Estuary"@en ;
  skos:topConceptOf asls:landform ;
.
lf:landform-element-FAN
  a skos:Concept ;
  skos-ext:isMemberOf lf:landform-element-glossary ;
  dcterms:identifier "http://anzsoil.org/def/au/asls/landform/landform-element-FAN"^^xsd:anyURI ;
  skos:definition "large, gently inclined to level element with radial slope lines inclined away from a point, resulting from aggradation, or occasionally from erosion, by channelled, often braided, stream flow, or possibly by sheet flow."@en ;
  skos:inScheme asls:landform ;
  skos:notation "FAN" ;
  skos:prefLabel "Fan"@en ;
  skos:topConceptOf asls:landform ;
.
lf:landform-element-FIL
  a skos:Concept ;
  skos-ext:isMemberOf lf:landform-element-glossary ;
  dcterms:identifier "http://anzsoil.org/def/au/asls/landform/landform-element-FIL"^^xsd:anyURI ;
  skos:definition "flat aggraded by human activity."@en ;
  skos:inScheme asls:landform ;
  skos:notation "FIL" ;
  skos:prefLabel "Fill-top"@en ;
  skos:topConceptOf asls:landform ;
.
lf:landform-element-FLD
  a skos:Concept ;
  skos-ext:isMemberOf lf:landform-element-glossary ;
  dcterms:identifier "http://anzsoil.org/def/au/asls/landform/landform-element-FLD"^^xsd:anyURI ;
  skos:definition "flat inclined radially away from a point on the margin or at the end of a stream channel, aggraded by over-bank stream flow, or by channelled stream flow associated with channels developed within the over-bank flow; part of a covered plain landform pattern."@en ;
  skos:inScheme asls:landform ;
  skos:notation "FLD" ;
  skos:prefLabel "Flood-out"@en ;
  skos:topConceptOf asls:landform ;
.
lf:landform-element-FOO
  a skos:Concept ;
  skos-ext:isMemberOf lf:landform-element-glossary ;
  dcterms:identifier "http://anzsoil.org/def/au/asls/landform/landform-element-FOO"^^xsd:anyURI ;
  skos:definition "moderately to very gently inclined waning lower slope resulting from aggradation or erosion by sheet flow, earth flow or creep (cf. pediment)."@en ;
  skos:inScheme asls:landform ;
  skos:notation "FOO" ;
  skos:prefLabel "Footslope"@en ;
  skos:topConceptOf asls:landform ;
.
lf:landform-element-FOR
  a skos:Concept ;
  skos-ext:isMemberOf lf:landform-element-glossary ;
  dcterms:identifier "http://anzsoil.org/def/au/asls/landform/landform-element-FOR"^^xsd:anyURI ;
  skos:definition "very long, nearly straight, moderately inclined to very steep ridge built up by the wind from material from an adjacent beach."@en ;
  skos:inScheme asls:landform ;
  skos:notation "FOR" ;
  skos:prefLabel "Foredune"@en ;
  skos:topConceptOf asls:landform ;
.
lf:landform-element-GUL
  a skos:Concept ;
  skos-ext:isMemberOf lf:landform-element-glossary ;
  dcterms:identifier "http://anzsoil.org/def/au/asls/landform/landform-element-GUL"^^xsd:anyURI ;
  skos:definition "open depression with short, precipitous walls and moderately inclined to very gently inclined floor or small stream channel, eroded by channelled stream flow and consequent collapse and water-aided mass movement."@en ;
  skos:inScheme asls:landform ;
  skos:notation "GUL" ;
  skos:prefLabel "Gully"@en ;
  skos:topConceptOf asls:landform ;
.
lf:landform-element-HCR
  a skos:Concept ;
  skos-ext:isMemberOf lf:landform-element-glossary ;
  dcterms:identifier "http://anzsoil.org/def/au/asls/landform/landform-element-HCR"^^xsd:anyURI ;
  skos:definition "very gently inclined to steep crest, smoothly convex, eroded mainly by creep and sheet wash. A typical element of mountains, hills, low hills and rises."@en ;
  skos:inScheme asls:landform ;
  skos:notation "HCR" ;
  skos:prefLabel "Hillcrest"@en ;
  skos:topConceptOf asls:landform ;
.
lf:landform-element-HSL
  a skos:Concept ;
  skos-ext:isMemberOf lf:landform-element-glossary ;
  dcterms:identifier "http://anzsoil.org/def/au/asls/landform/landform-element-HSL"^^xsd:anyURI ;
  skos:definition "gently inclined to precipitous slope, commonly simple and maximal, eroded by sheet wash, creep or water-aided mass movement. A typical element of mountains, hills, low hills and rises."@en ;
  skos:inScheme asls:landform ;
  skos:notation "HSL" ;
  skos:prefLabel "Hillslope"@en ;
  skos:topConceptOf asls:landform ;
.
lf:landform-element-ITF
  a skos:Concept ;
  skos-ext:isMemberOf lf:landform-element-glossary ;
  dcterms:identifier "http://anzsoil.org/def/au/asls/landform/landform-element-ITF"^^xsd:anyURI ;
  skos:definition "large flat subject to inundation by water that is usually salt or brackish, aggraded by tides. An intertidal flat (ITF) is frequently inundated."@en ;
  skos:inScheme asls:landform ;
  skos:notation "ITF" ;
  skos:prefLabel "Intertidal flat"@en ;
  skos:related lf:landform-element-TDF ;
  skos:topConceptOf asls:landform ;
.
lf:landform-element-LAG
  a skos:Concept ;
  skos-ext:isMemberOf lf:landform-element-glossary ;
  dcterms:identifier "http://anzsoil.org/def/au/asls/landform/landform-element-LAG"^^xsd:anyURI ;
  skos:definition "closed depression filled with water that is typically salt or brackish, bounded at least in part by forms aggraded or built up by waves or reef-building organisms."@en ;
  skos:inScheme asls:landform ;
  skos:notation "LAG" ;
  skos:prefLabel "Lagoon"@en ;
  skos:topConceptOf asls:landform ;
.
lf:landform-element-LAK
  a skos:Concept ;
  skos-ext:isMemberOf lf:landform-element-glossary ;
  dcterms:identifier "http://anzsoil.org/def/au/asls/landform/landform-element-LAK"^^xsd:anyURI ;
  skos:definition "large, water-filled closed depression."@en ;
  skos:inScheme asls:landform ;
  skos:notation "LAK" ;
  skos:prefLabel "Lake"@en ;
  skos:topConceptOf asls:landform ;
.
lf:landform-element-LDS
  a skos:Concept ;
  skos-ext:isMemberOf lf:landform-element-glossary ;
  dcterms:identifier "http://anzsoil.org/def/au/asls/landform/landform-element-LDS"^^xsd:anyURI ;
  skos:definition "moderately inclined to very steep slope, eroded in the upper part and aggraded in the lower part by water-aided mass movement, characterised by irregular hummocks."@en ;
  skos:inScheme asls:landform ;
  skos:notation "LDS" ;
  skos:prefLabel "Landslide"@en ;
  skos:topConceptOf asls:landform ;
.
lf:landform-element-LEV
  a skos:Concept ;
  skos-ext:isMemberOf lf:landform-element-glossary ;
  dcterms:identifier "http://anzsoil.org/def/au/asls/landform/landform-element-LEV"^^xsd:anyURI ;
  skos:definition "very long, low, narrow, nearly level, sinuous ridge immediately adjacent to a stream channel, built up by over-bank flow. Levees are built, usually in pairs bounding the two sides of a stream channel, at the level reached by frequent floods. This element is part of a covered plain landform pattern. For an artificial levee, use embankment. See also prior stream."@en ;
  skos:inScheme asls:landform ;
  skos:notation "LEV" ;
  skos:prefLabel "Levee"@en ;
  skos:topConceptOf asls:landform ;
.
lf:landform-element-LUN
  a skos:Concept ;
  skos-ext:isMemberOf lf:landform-element-glossary ;
  dcterms:identifier "http://anzsoil.org/def/au/asls/landform/landform-element-LUN"^^xsd:anyURI ;
  skos:definition "elongated, gently curved, low ridge built up by wind on the margin of a playa, typically with a moderate, wave-modified slope towards the playa and a gentle outer slope."@en ;
  skos:inScheme asls:landform ;
  skos:notation "LUN" ;
  skos:prefLabel "Lunette"@en ;
  skos:topConceptOf asls:landform ;
.
lf:landform-element-MAA
  a skos:Concept ;
  skos-ext:isMemberOf lf:landform-element-glossary ;
  dcterms:identifier "http://anzsoil.org/def/au/asls/landform/landform-element-MAA"^^xsd:anyURI ;
  skos:definition "elongated, gently curved, low ridge built up by wind on the margin of a playa, typically with a moderate, wave-modified slope towards the playa and a gentle outer slope."@en ;
  skos:inScheme asls:landform ;
  skos:notation "MAA" ;
  skos:prefLabel "Maar"@en ;
  skos:topConceptOf asls:landform ;
.
lf:landform-element-MOU
  a skos:Concept ;
  skos-ext:isMemberOf lf:landform-element-glossary ;
  dcterms:identifier "http://anzsoil.org/def/au/asls/landform/landform-element-MOU"^^xsd:anyURI ;
  skos:definition "hillock built up by human activity."@en ;
  skos:inScheme asls:landform ;
  skos:notation "MOU" ;
  skos:prefLabel "Mound"@en ;
  skos:topConceptOf asls:landform ;
.
lf:landform-element-OXB
  a skos:Concept ;
  skos-ext:isMemberOf lf:landform-element-glossary ;
  dcterms:identifier "http://anzsoil.org/def/au/asls/landform/landform-element-OXB"^^xsd:anyURI ;
  skos:definition "long, curved, commonly water-filled closed depression eroded by channelled stream flow but closed as a result of aggradation by channelled or over-bank stream flow during the formation of a meander plain landform pattern. The floor of an ox-bow may be more or less aggraded by over-bank stream flow, wind, and biological (peat) accumulation."@en ;
  skos:inScheme asls:landform ;
  skos:notation "OXB" ;
  skos:prefLabel "Ox-bow"@en ;
  skos:topConceptOf asls:landform ;
.
lf:landform-element-PED
  a skos:Concept ;
  skos-ext:isMemberOf lf:landform-element-glossary ;
  dcterms:identifier "http://anzsoil.org/def/au/asls/landform/landform-element-PED"^^xsd:anyURI ;
  skos:definition "large, gently inclined to level (<1%) waning lower slope, with slope lines inclined in a single direction, or somewhat convergent or divergent, eroded or sometimes slightly aggraded by sheet flow (cf. footslope). It is underlain by bedrock."@en ;
  skos:inScheme asls:landform ;
  skos:notation "PED" ;
  skos:prefLabel "Pediment"@en ;
  skos:topConceptOf asls:landform ;
.
lf:landform-element-PIT
  a skos:Concept ;
  skos-ext:isMemberOf lf:landform-element-glossary ;
  dcterms:identifier "http://anzsoil.org/def/au/asls/landform/landform-element-PIT"^^xsd:anyURI ;
  skos:definition "closed depression excavated by human activity."@en ;
  skos:inScheme asls:landform ;
  skos:notation "PIT" ;
  skos:prefLabel "Pit"@en ;
  skos:topConceptOf asls:landform ;
.
lf:landform-element-PLA
  a skos:Concept ;
  skos-ext:isMemberOf lf:landform-element-glossary ;
  dcterms:identifier "http://anzsoil.org/def/au/asls/landform/landform-element-PLA"^^xsd:anyURI ;
  skos:definition "large, very gently inclined or level element, of unspecified geomorphological agent or mode of activity."@en ;
  skos:inScheme asls:landform ;
  skos:notation "PLA" ;
  skos:prefLabel "Plain"@en ;
  skos:topConceptOf asls:landform ;
.
lf:landform-element-PLY
  a skos:Concept ;
  skos-ext:isMemberOf lf:landform-element-glossary ;
  dcterms:identifier "http://anzsoil.org/def/au/asls/landform/landform-element-PLY"^^xsd:anyURI ;
  skos:altLabel "Pan"@en ;
  skos:definition "large, shallow, level-floored closed depression, intermittently water-filled, but mainly dry due to evaporation, bounded as a rule by flats aggraded by sheet flow and channelled stream flow."@en ;
  skos:inScheme asls:landform ;
  skos:notation "PLY" ;
  skos:prefLabel "Playa"@en ;
  skos:topConceptOf asls:landform ;
.
lf:landform-element-PST
  a skos:Concept ;
  skos-ext:isMemberOf lf:landform-element-glossary ;
  dcterms:identifier "http://anzsoil.org/def/au/asls/landform/landform-element-PST"^^xsd:anyURI ;
  skos:definition "long, generally sinuous, low ridge built up from materials originally deposited by stream flow along the line of a former stream channel. The landform element may include a depression marking the old stream bed, and relict levees."@en ;
  skos:inScheme asls:landform ;
  skos:notation "PST" ;
  skos:prefLabel "Prior stream"@en ;
  skos:topConceptOf asls:landform ;
.
lf:landform-element-REC
  a skos:Concept ;
  skos-ext:isMemberOf lf:landform-element-glossary ;
  dcterms:identifier "http://anzsoil.org/def/au/asls/landform/landform-element-REC"^^xsd:anyURI ;
  skos:definition "crest of hillock of very low to extremely low relief (<30 m) (see residual rise)."@en ;
  skos:inScheme asls:landform ;
  skos:notation "REC" ;
  skos:prefLabel "Risecrest"@en ;
  skos:topConceptOf asls:landform ;
.
lf:landform-element-REF
  a skos:Concept ;
  skos-ext:isMemberOf lf:landform-element-glossary ;
  dcterms:identifier "http://anzsoil.org/def/au/asls/landform/landform-element-REF"^^xsd:anyURI ;
  skos:definition "flat built up to sea level by marine organisms."@en ;
  skos:inScheme asls:landform ;
  skos:notation "REF" ;
  skos:prefLabel "Reef flat"@en ;
  skos:topConceptOf asls:landform ;
.
lf:landform-element-RER
  a skos:Concept ;
  skos-ext:isMemberOf lf:landform-element-glossary ;
  dcterms:identifier "http://anzsoil.org/def/au/asls/landform/landform-element-RER"^^xsd:anyURI ;
  skos:definition "hillock of very low to extremely low relief (<30 m) and very gentle to steep slopes. This term is used to refer to an isolated rise surrounded by other landforms."@en ;
  skos:inScheme asls:landform ;
  skos:notation "RER" ;
  skos:prefLabel "Residual rise"@en ;
  skos:topConceptOf asls:landform ;
.
lf:landform-element-RES
  a skos:Concept ;
  skos-ext:isMemberOf lf:landform-element-glossary ;
  dcterms:identifier "http://anzsoil.org/def/au/asls/landform/landform-element-RES"^^xsd:anyURI ;
  skos:definition "slope of hillock of very low to extremely low relief (<30 m) (see residual rise)."@en ;
  skos:inScheme asls:landform ;
  skos:notation "RES" ;
  skos:prefLabel "Riseslope"@en ;
  skos:topConceptOf asls:landform ;
.
lf:landform-element-RFL
  a skos:Concept ;
  skos-ext:isMemberOf lf:landform-element-glossary ;
  dcterms:identifier "http://anzsoil.org/def/au/asls/landform/landform-element-RFL"^^xsd:anyURI ;
  skos:definition "flat of bare consolidated rock, usually eroded by sheet wash."@en ;
  skos:inScheme asls:landform ;
  skos:notation "RFL" ;
  skos:prefLabel "Rock flat"@en ;
  skos:topConceptOf asls:landform ;
.
lf:landform-element-RPL
  a skos:Concept ;
  skos-ext:isMemberOf lf:landform-element-glossary ;
  dcterms:identifier "http://anzsoil.org/def/au/asls/landform/landform-element-RPL"^^xsd:anyURI ;
  skos:definition "flat of consolidated rock eroded by waves."@en ;
  skos:inScheme asls:landform ;
  skos:notation "RPL" ;
  skos:prefLabel "Rock platform"@en ;
  skos:topConceptOf asls:landform ;
.
lf:landform-element-SCA
  a skos:Concept ;
  skos-ext:isMemberOf lf:landform-element-glossary ;
  dcterms:identifier "http://anzsoil.org/def/au/asls/landform/landform-element-SCA"^^xsd:anyURI ;
  skos:definition "very wide, steep to precipitous maximal slope eroded by gravity, water-aided mass movement or sheet flow (cf. cliff)."@en ;
  skos:inScheme asls:landform ;
  skos:notation "SCA" ;
  skos:prefLabel "Scarp"@en ;
  skos:topConceptOf asls:landform ;
.
lf:landform-element-SCD
  a skos:Concept ;
  skos-ext:isMemberOf lf:landform-element-glossary ;
  dcterms:identifier "http://anzsoil.org/def/au/asls/landform/landform-element-SCD"^^xsd:anyURI ;
  skos:definition "flat, bare of vegetation, from which soil has been eroded or excavated by surface wash or wind."@en ;
  skos:inScheme asls:landform ;
  skos:notation "SCD" ;
  skos:prefLabel "Scald"@en ;
  skos:topConceptOf asls:landform ;
.
lf:landform-element-SCR
  a skos:Concept ;
  skos-ext:isMemberOf lf:landform-element-glossary ;
  dcterms:identifier "http://anzsoil.org/def/au/asls/landform/landform-element-SCR"^^xsd:anyURI ;
  skos:definition "long, curved, very low ridge built up by channelled stream flow and left relict by channel migration. Part of a meander plain landform pattern."@en ;
  skos:inScheme asls:landform ;
  skos:notation "SCR" ;
  skos:prefLabel "Scroll"@en ;
  skos:topConceptOf asls:landform ;
.
lf:landform-element-SFS
  a skos:Concept ;
  skos-ext:isMemberOf lf:landform-element-glossary ;
  dcterms:identifier "http://anzsoil.org/def/au/asls/landform/landform-element-SFS"^^xsd:anyURI ;
  skos:definition "waning or minimal slope situated below a scarp, with its contours generally parallel to the line of the scarp."@en ;
  skos:inScheme asls:landform ;
  skos:notation "SFS" ;
  skos:prefLabel "Scarp-footslope"@en ;
  skos:topConceptOf asls:landform ;
.
lf:landform-element-SRP
  a skos:Concept ;
  skos-ext:isMemberOf lf:landform-element-glossary ;
  dcterms:identifier "http://anzsoil.org/def/au/asls/landform/landform-element-SRP"^^xsd:anyURI ;
  skos:definition "large flat resulting from aggradation by channelled stream flow as a stream migrates from side to side; the dominant element of a meander plain landform pattern. This landform element may include occurrences of scroll, swale and ox-bow."@en ;
  skos:inScheme asls:landform ;
  skos:notation "SRP" ;
  skos:prefLabel "Scroll plain"@en ;
  skos:topConceptOf asls:landform ;
.
lf:landform-element-STB
  a skos:Concept ;
  skos-ext:isMemberOf lf:landform-element-glossary ;
  dcterms:identifier "http://anzsoil.org/def/au/asls/landform/landform-element-STB"^^xsd:anyURI ;
  skos:definition "linear, generally sinuous open depression forming the bottom of a stream channel, eroded and locally excavated, aggraded or built up by channelled stream flow. Parts that are built up include bars."@en ;
  skos:inScheme asls:landform ;
  skos:notation "STB" ;
  skos:prefLabel "Stream bed"@en ;
  skos:topConceptOf asls:landform ;
.
lf:landform-element-STC
  a skos:Concept ;
  skos-ext:isMemberOf lf:landform-element-glossary ;
  dcterms:identifier "http://anzsoil.org/def/au/asls/landform/landform-element-STC"^^xsd:anyURI ;
  skos:altLabel "Channel"@en ;
  skos:definition "linear, generally sinuous open depression, in parts eroded, excavated, built up and aggraded by channelled stream flow. This element comprises stream bed and banks."@en ;
  skos:inScheme asls:landform ;
  skos:notation "STC" ;
  skos:prefLabel "Stream channel"@en ;
  skos:topConceptOf asls:landform ;
.
lf:landform-element-STF
  a skos:Concept ;
  skos-ext:isMemberOf lf:landform-element-glossary ;
  dcterms:identifier "http://anzsoil.org/def/au/asls/landform/landform-element-STF"^^xsd:anyURI ;
  skos:definition "large flat subject to inundation by water that is usually salt or brackish, aggraded by tides. a supratidal flat (STF) is seldom inundated."@en ;
  skos:inScheme asls:landform ;
  skos:notation "STF" ;
  skos:prefLabel "Supratidal flat"@en ;
  skos:related lf:landform-element-TDF ;
  skos:topConceptOf asls:landform ;
.
lf:landform-element-SUS
  a skos:Concept ;
  skos-ext:isMemberOf lf:landform-element-glossary ;
  dcterms:identifier "http://anzsoil.org/def/au/asls/landform/landform-element-SUS"^^xsd:anyURI ;
  skos:definition "very wide, level to gently inclined crest with abrupt margins, commonly eroded by water-aided mass movement or sheet wash."@en ;
  skos:inScheme asls:landform ;
  skos:notation "SUS" ;
  skos:prefLabel "Summit surface"@en ;
  skos:topConceptOf asls:landform ;
.
lf:landform-element-SWL
  a skos:Concept ;
  skos-ext:isMemberOf lf:landform-element-glossary ;
  dcterms:identifier "http://anzsoil.org/def/au/asls/landform/landform-element-SWL"^^xsd:anyURI ;
  skos:definition "(i) linear, level-floored open depression excavated by wind, or left relict between ridges built up by wind or waves, or built up to a lesser height than them. (ii) long, curved open or closed depression left relict between scrolls built up by channelled stream flow."@en ;
  skos:inScheme asls:landform ;
  skos:notation "SWL" ;
  skos:prefLabel "Swale"@en ;
  skos:topConceptOf asls:landform ;
.
lf:landform-element-SWP
  a skos:Concept ;
  skos-ext:isMemberOf lf:landform-element-glossary ;
  dcterms:identifier "http://anzsoil.org/def/au/asls/landform/landform-element-SWP"^^xsd:anyURI ;
  skos:definition "almost level, closed or almost closed depression with a seasonal or permanent watertable at or above the surface, commonly aggraded by overbank stream flow and sometimes biological (peat) accumulation."@en ;
  skos:inScheme asls:landform ;
  skos:notation "SWP" ;
  skos:prefLabel "Swamp"@en ;
  skos:topConceptOf asls:landform ;
.
lf:landform-element-TAL
  a skos:Concept ;
  skos-ext:isMemberOf lf:landform-element-glossary ;
  dcterms:identifier "http://anzsoil.org/def/au/asls/landform/landform-element-TAL"^^xsd:anyURI ;
  skos:definition "moderately inclined or steep waning lower slope, consisting of rock fragments aggraded by gravity."@en ;
  skos:inScheme asls:landform ;
  skos:notation "TAL" ;
  skos:prefLabel "Talus"@en ;
  skos:topConceptOf asls:landform ;
.
lf:landform-element-TDC
  a skos:Concept ;
  skos-ext:isMemberOf lf:landform-element-glossary ;
  dcterms:identifier "http://anzsoil.org/def/au/asls/landform/landform-element-TDC"^^xsd:anyURI ;
  skos:definition "intermittently water-filled open depression in parts eroded, excavated, built up and aggraded by channelled tide-water flow; type of stream channel characterised by a rapid increase in width downstream."@en ;
  skos:inScheme asls:landform ;
  skos:notation "TDC" ;
  skos:prefLabel "Tidal creek"@en ;
  skos:topConceptOf asls:landform ;
.
lf:landform-element-TDF
  a skos:Concept ;
  skos-ext:isMemberOf lf:landform-element-glossary ;
  dcterms:identifier "http://anzsoil.org/def/au/asls/landform/landform-element-TDF"^^xsd:anyURI ;
  skos:definition "large flat subject to inundation by water that is usually salt or brackish, aggraded by tides. An intertidal flat (ITF) is frequently inundated; a supratidal flat (STF) is seldom inundated."@en ;
  skos:inScheme asls:landform ;
  skos:notation "TDF" ;
  skos:prefLabel "Tidal flat"@en ;
  skos:related lf:landform-element-ITF ;
  skos:related lf:landform-element-STF ;
  skos:topConceptOf asls:landform ;
.
lf:landform-element-TEF
  a skos:Concept ;
  skos-ext:isMemberOf lf:landform-element-glossary ;
  dcterms:identifier "http://anzsoil.org/def/au/asls/landform/landform-element-TEF"^^xsd:anyURI ;
  skos:definition "small flat aggraded or eroded by channelled or over-bank stream flow, standing above a scarp and no longer frequently inundated; a former valley flat or part of a former flood plain."@en ;
  skos:inScheme asls:landform ;
  skos:notation "TEF" ;
  skos:prefLabel "Terrace flat"@en ;
  skos:topConceptOf asls:landform ;
.
lf:landform-element-TEP
  a skos:Concept ;
  skos-ext:isMemberOf lf:landform-element-glossary ;
  dcterms:identifier "http://anzsoil.org/def/au/asls/landform/landform-element-TEP"^^xsd:anyURI ;
  skos:definition "large or very large flat aggraded by channelled or over-bank stream flow, standing above a scarp and no longer frequently inundated; part of a former flood plain."@en ;
  skos:inScheme asls:landform ;
  skos:notation "TEP" ;
  skos:prefLabel "Terrace plain"@en ;
  skos:topConceptOf asls:landform ;
.
lf:landform-element-TOR
  a skos:Concept ;
  skos-ext:isMemberOf lf:landform-element-glossary ;
  dcterms:identifier "http://anzsoil.org/def/au/asls/landform/landform-element-TOR"^^xsd:anyURI ;
  skos:definition "steep to precipitous hillock, typically convex, with a surface mainly of bare rock, either coherent or comprising subangular to rounded, large boulders (exhumed core-stones, also themselves called tors) separated by open fissures; eroded by sheet wash or water-aided mass movement."@en ;
  skos:inScheme asls:landform ;
  skos:notation "TOR" ;
  skos:prefLabel "Tor"@en ;
  skos:topConceptOf asls:landform ;
.
lf:landform-element-TRE
  a skos:Concept ;
  skos-ext:isMemberOf lf:landform-element-glossary ;
  dcterms:identifier "http://anzsoil.org/def/au/asls/landform/landform-element-TRE"^^xsd:anyURI ;
  skos:definition "open depression excavated by human activity."@en ;
  skos:inScheme asls:landform ;
  skos:notation "TRE" ;
  skos:prefLabel "Trench"@en ;
  skos:topConceptOf asls:landform ;
.
lf:landform-element-TUM
  a skos:Concept ;
  skos-ext:isMemberOf lf:landform-element-glossary ;
  dcterms:identifier "http://anzsoil.org/def/au/asls/landform/landform-element-TUM"^^xsd:anyURI ;
  skos:definition "hillock heaved up by volcanism (or, elsewhere, built up by human activity at a burial site)."@en ;
  skos:inScheme asls:landform ;
  skos:notation "TUM" ;
  skos:prefLabel "Tumulus"@en ;
  skos:topConceptOf asls:landform ;
.
lf:landform-element-VLF
  a skos:Concept ;
  skos-ext:isMemberOf lf:landform-element-glossary ;
  dcterms:identifier "http://anzsoil.org/def/au/asls/landform/landform-element-VLF"^^xsd:anyURI ;
  skos:definition "small, gently inclined to level flat, aggraded or sometimes eroded by channelled or over-bank stream flow, typically enclosed by hillslopes; a miniature alluvial plain landform pattern."@en ;
  skos:inScheme asls:landform ;
  skos:notation "VLF" ;
  skos:prefLabel "Valley flat"@en ;
  skos:topConceptOf asls:landform ;
.
lf:landform-element-descriptions
  a skos:Collection ;
  skos-ext:topMemberOf asls:landform ;
  dcterms:identifier "http://anzsoil.org/def/au/asls/landform/landform-element-descriptions"^^xsd:anyURI ;
  skos:definition "A landform element may be described by the following attributes, assessed within a circle of about 20 m radius:"@en ;
  skos:member lf:element-dimensions ;
  skos:member lf:landform-genesis ;
  skos:member lf:location-within-the-landform-element ;
  skos:member lf:location-within-toposequence ;
  skos:member lf:morphological-type ;
  skos:member lf:slope ;
  skos:prefLabel "Description of landform element"@en ;
.
lf:landform-element-glossary
  a skos:Collection ;
  skos-ext:topMemberOf asls:landform ;
  dcterms:identifier "http://anzsoil.org/def/au/asls/landform/landform-element-glossary"^^xsd:anyURI ;
  skos:definition "The landform element glossary aims to provide an adequate, concise set of names for types of landform element."@en ;
  skos:member lf:landform-element-ALC ;
  skos:member lf:landform-element-BAN ;
  skos:member lf:landform-element-BAR ;
  skos:member lf:landform-element-BEA ;
  skos:member lf:landform-element-BEN ;
  skos:member lf:landform-element-BER ;
  skos:member lf:landform-element-BKP ;
  skos:member lf:landform-element-BOU ;
  skos:member lf:landform-element-BRI ;
  skos:member lf:landform-element-BRK ;
  skos:member lf:landform-element-CBE ;
  skos:member lf:landform-element-CFS ;
  skos:member lf:landform-element-CIR ;
  skos:member lf:landform-element-CLI ;
  skos:member lf:landform-element-CON ;
  skos:member lf:landform-element-COS ;
  skos:member lf:landform-element-CRA ;
  skos:member lf:landform-element-CUT ;
  skos:member lf:landform-element-DAM ;
  skos:member lf:landform-element-DBA ;
  skos:member lf:landform-element-DDE ;
  skos:member lf:landform-element-DOC ;
  skos:member lf:landform-element-DOL ;
  skos:member lf:landform-element-DUB ;
  skos:member lf:landform-element-DUC ;
  skos:member lf:landform-element-DUF ;
  skos:member lf:landform-element-DUH ;
  skos:member lf:landform-element-DUN ;
  skos:member lf:landform-element-DUP ;
  skos:member lf:landform-element-DUS ;
  skos:member lf:landform-element-EMB ;
  skos:member lf:landform-element-EST ;
  skos:member lf:landform-element-FAN ;
  skos:member lf:landform-element-FIL ;
  skos:member lf:landform-element-FLD ;
  skos:member lf:landform-element-FOO ;
  skos:member lf:landform-element-FOR ;
  skos:member lf:landform-element-GUL ;
  skos:member lf:landform-element-HCR ;
  skos:member lf:landform-element-HSL ;
  skos:member lf:landform-element-ITF ;
  skos:member lf:landform-element-LAG ;
  skos:member lf:landform-element-LAK ;
  skos:member lf:landform-element-LDS ;
  skos:member lf:landform-element-LEV ;
  skos:member lf:landform-element-LUN ;
  skos:member lf:landform-element-MAA ;
  skos:member lf:landform-element-MOU ;
  skos:member lf:landform-element-OXB ;
  skos:member lf:landform-element-PED ;
  skos:member lf:landform-element-PIT ;
  skos:member lf:landform-element-PLA ;
  skos:member lf:landform-element-PLY ;
  skos:member lf:landform-element-PST ;
  skos:member lf:landform-element-REC ;
  skos:member lf:landform-element-REF ;
  skos:member lf:landform-element-RER ;
  skos:member lf:landform-element-RES ;
  skos:member lf:landform-element-RFL ;
  skos:member lf:landform-element-RPL ;
  skos:member lf:landform-element-SCA ;
  skos:member lf:landform-element-SCD ;
  skos:member lf:landform-element-SCR ;
  skos:member lf:landform-element-SFS ;
  skos:member lf:landform-element-SRP ;
  skos:member lf:landform-element-STB ;
  skos:member lf:landform-element-STC ;
  skos:member lf:landform-element-STF ;
  skos:member lf:landform-element-SUS ;
  skos:member lf:landform-element-SWL ;
  skos:member lf:landform-element-SWP ;
  skos:member lf:landform-element-TAL ;
  skos:member lf:landform-element-TDC ;
  skos:member lf:landform-element-TDF ;
  skos:member lf:landform-element-TEF ;
  skos:member lf:landform-element-TEP ;
  skos:member lf:landform-element-TOR ;
  skos:member lf:landform-element-TRE ;
  skos:member lf:landform-element-TUM ;
  skos:member lf:landform-element-VLF ;
  skos:prefLabel "Glossary of landform elements"@en ;
.
lf:landform-genesis
  a skos:Collection ;
  dcterms:identifier "http://anzsoil.org/def/au/asls/landform/landform-genesis"^^xsd:anyURI ;
  skos:definition """The two following sections on geomorphological modes and agents refer to the inferred genesis of a landform element. This genesis may have spanned thousands of years. Changes, such as erosion and aggradation, that are produced by current land use are separately assessed as attributes of the land surface (pages 92–96).
To think clearly about the origin of a landform, one should ask two questions: ‘What agent formed it?’ and ‘What was the mode of activity of that agent?’
Landforms created by different agents, such as wind, creep, and stream flow, may result from the same mode of geomorphological activity: erosion, for example. Those created by the same agent may differ according to whether the mode of activity builds them up or erodes them down.
"""@en ;
  skos:member lf:geomorphological-agents ;
  skos:member lf:mode-of-geomorphological-activity ;
  skos:prefLabel "Landform genesis"@en ;
.
lf:landform-pattern-ALF
  a skos:Concept ;
  skos-ext:isMemberOf lf:landform-pattern-glossary ;
  skos-ext:relatedCollection lf:landform-pattern-ALF-common-elements ;
  skos-ext:relatedCollection lf:landform-pattern-ALF-comparewith-patterns ;
  skos-ext:relatedCollection lf:landform-pattern-ALF-typical-elements ;
  dcterms:identifier "http://anzsoil.org/def/au/asls/landform/landform-pattern-ALF"^^xsd:anyURI ;
  dcterms:references lf:relief-class-P ;
  dcterms:references lf:slope-class-LE ;
  dcterms:references lf:slope-class-VG ;
  skos:definition """<p>level (less than 1% slope) to very gently inclined, complex landform pattern of extremely low relief. The rapidly migrating alluvial stream channels are shallow to moderately deep, locally numerous, but elsewhere widely spaced. The channels form a centrifugal to divergent, integrated, reticulated to distributary pattern. The landform pattern includes areas that are bar plains, being aggraded or eroded by frequently active channelled stream flow, and other areas comprising terraces or stagnant alluvial plains with slopes that are greater than usual, formed by channelled stream flow but now relict. Incision in the upslope area may give rise to an erosional stream bed between scarps. </p>
<p>Typical elements: stream bed, bar, plain.</p>
<p>Common element: scarp.</p>
<p>Compare with sheet-flood fan and pediment. </p>"""^^rdf:HTML ;
  skos:inScheme asls:landform ;
  skos:notation "ALF" ;
  skos:prefLabel "Alluvial fan"@en ;
  skos:related lf:relief-class-P ;
  skos:related lf:slope-class-LE ;
  skos:related lf:slope-class-VG ;
  skos:topConceptOf asls:landform ;
.
lf:landform-pattern-ALF-common-elements
  a skos:Collection ;
  dcterms:identifier "http://anzsoil.org/def/au/asls/landform/landform-pattern-ALF-common-elements"^^xsd:anyURI ;
  skos:member lf:landform-element-SCA ;
  skos:prefLabel "Common elements of an Alluvial fan"@en ;
  skos:related lf:landform-pattern-ALF ;
.
lf:landform-pattern-ALF-comparewith-patterns
  a skos:Collection ;
  dcterms:identifier "http://anzsoil.org/def/au/asls/landform/landform-pattern-ALF-comparewith-patterns"^^xsd:anyURI ;
  skos:member lf:landform-pattern-PED ;
  skos:member lf:landform-pattern-SHF ;
  skos:prefLabel "Compare Alluvial fans with these patterns"@en ;
  skos:related lf:landform-pattern-ALF ;
.
lf:landform-pattern-ALF-typical-elements
  a skos:Collection ;
  dcterms:identifier "http://anzsoil.org/def/au/asls/landform/landform-pattern-ALF-typical-elements"^^xsd:anyURI ;
  skos:member lf:landform-element-BAR ;
  skos:member lf:landform-element-PLA ;
  skos:member lf:landform-element-STB ;
  skos:prefLabel "Typical elements of an Alluvial fan"@en ;
  skos:related lf:landform-pattern-ALF ;
.
lf:landform-pattern-ALP
  a skos:Concept ;
  skos-ext:isMemberOf lf:landform-pattern-glossary ;
  skos-ext:relatedCollection lf:landform-pattern-ALP-common-elements ;
  skos-ext:relatedCollection lf:landform-pattern-ALP-included-patterns ;
  skos-ext:relatedCollection lf:landform-pattern-ALP-occasional-elements ;
  skos-ext:relatedCollection lf:landform-pattern-ALP-typical-elements ;
  dcterms:identifier "http://anzsoil.org/def/au/asls/landform/landform-pattern-ALP"^^xsd:anyURI ;
  skos:definition """<p>level landform pattern with extremely low relief. The shallow to deep alluvial stream channels are sparse to widely spaced, forming a unidirectional, integrated network. There may be frequently active erosion and aggradation by channelled and overbank stream flow, or the landforms may be relict from these proceses. </p>
<p>Typical elements: stream channel (stream bed and bank), plain (dominant).</p>
<p>Common elements: bar, scroll, levee, backplain, swamp.</p>
<p>Occasional elements: ox-bow, flood-out, lake.</p>
<p>Included types of landform pattern are: flood plain, bar plain, meander plain, covered plain, anastomotic plain, delta, stagnant alluvial plain, terrace, terraced land. </p>""" ;
  skos:inScheme asls:landform ;
  skos:notation "ALP" ;
  skos:prefLabel "Alluvial plain"@en ;
  skos:related lf:relief-class-P ;
  skos:related lf:slope-class-LE ;
  skos:topConceptOf asls:landform ;
.
lf:landform-pattern-ALP-common-elements
  a skos:Collection ;
  dcterms:identifier "http://anzsoil.org/def/au/asls/landform/landform-pattern-ALP-common-elements"^^xsd:anyURI ;
  skos:member lf:landform-element-BAR ;
  skos:member lf:landform-element-BKP ;
  skos:member lf:landform-element-LEV ;
  skos:member lf:landform-element-SCR ;
  skos:member lf:landform-element-SWP ;
  skos:prefLabel "Common elements of an Alluvial plain"@en ;
  skos:related lf:landform-pattern-ALP ;
.
lf:landform-pattern-ALP-included-patterns
  a skos:Collection ;
  dcterms:identifier "http://anzsoil.org/def/au/asls/landform/landform-pattern-ALP-included-patterns"^^xsd:anyURI ;
  skos:member lf:landform-pattern-ANA ;
  skos:member lf:landform-pattern-BAR ;
  skos:member lf:landform-pattern-COV ;
  skos:member lf:landform-pattern-DEL ;
  skos:member lf:landform-pattern-FLO ;
  skos:member lf:landform-pattern-MEA ;
  skos:member lf:landform-pattern-STA ;
  skos:member lf:landform-pattern-TEL ;
  skos:member lf:landform-pattern-TER ;
  skos:prefLabel "Included types of landform pattern for Alluvial plain"@en ;
  skos:related lf:landform-pattern-ALP ;
.
lf:landform-pattern-ALP-occasional-elements
  a skos:Collection ;
  dcterms:identifier "http://anzsoil.org/def/au/asls/landform/landform-pattern-ALP-occasional-elements"^^xsd:anyURI ;
  skos:member lf:landform-element-FLD ;
  skos:member lf:landform-element-LAK ;
  skos:member lf:landform-element-OXB ;
  skos:prefLabel "Occasional elements of an Alluvial plain"@en ;
  skos:related lf:landform-pattern-ALP ;
.
lf:landform-pattern-ALP-typical-elements
  a skos:Collection ;
  dcterms:identifier "http://anzsoil.org/def/au/asls/landform/landform-pattern-ALP-typical-elements"^^xsd:anyURI ;
  skos:member lf:landform-element-BAN ;
  skos:member lf:landform-element-PLA ;
  skos:member lf:landform-element-STB ;
  skos:member lf:landform-element-STC ;
  skos:prefLabel "Typical elements of an Alluvial plain"@en ;
  skos:related lf:landform-pattern-ALP ;
.
lf:landform-pattern-ANA
  a skos:Concept ;
  skos-ext:isMemberOf lf:landform-pattern-glossary ;
  skos-ext:relatedCollection lf:landform-pattern-ANA-common-elements ;
  skos-ext:relatedCollection lf:landform-pattern-ANA-comparewith-patterns ;
  skos-ext:relatedCollection lf:landform-pattern-ANA-typical-elements ;
  dcterms:identifier "http://anzsoil.org/def/au/asls/landform/landform-pattern-ANA"^^xsd:anyURI ;
  skos:definition """<p>flood plain with slowly migrating, deep alluvial channels, usually moderately spaced, forming a divergent to unidirectional, integrated reticulated network. There is frequently active aggradation by over-bank and channelled stream flow. </p>
<p>Typical elements: stream channel (stream bed and bank), levee, backplain (dominant).</p>
<p>Common element: swamp.</p>
<p>Compare with other types under alluvial plain and flood plain. </p>"""^^rdf:HTML ;
  skos:inScheme asls:landform ;
  skos:notation "ANA" ;
  skos:prefLabel "Anastomotic plain"@en ;
  skos:related lf:relief-class-P ;
  skos:related lf:slope-class-LE ;
  skos:topConceptOf asls:landform ;
.
lf:landform-pattern-ANA-common-elements
  a skos:Collection ;
  dcterms:identifier "http://anzsoil.org/def/au/asls/landform/landform-pattern-ANA-common-elements"^^xsd:anyURI ;
  skos:member lf:landform-element-SWP ;
  skos:prefLabel "Common elements of an Anastomotic plain"@en ;
  skos:related lf:landform-pattern-ANA ;
.
lf:landform-pattern-ANA-comparewith-patterns
  a skos:Collection ;
  dcterms:identifier "http://anzsoil.org/def/au/asls/landform/landform-pattern-ANA-comparewith-patterns"^^xsd:anyURI ;
  skos:member lf:landform-pattern-ALP ;
  skos:member lf:landform-pattern-FLO ;
  skos:prefLabel "Compare Anastomotic plain with these patterns"@en ;
  skos:related lf:landform-pattern-ANA ;
.
lf:landform-pattern-ANA-typical-elements
  a skos:Collection ;
  dcterms:identifier "http://anzsoil.org/def/au/asls/landform/landform-pattern-ANA-typical-elements"^^xsd:anyURI ;
  skos:member lf:landform-element-BAN ;
  skos:member lf:landform-element-BKP ;
  skos:member lf:landform-element-LEV ;
  skos:member lf:landform-element-STB ;
  skos:member lf:landform-element-STC ;
  skos:prefLabel "Typical elements of an Anastomotic plain"@en ;
  skos:related lf:landform-pattern-ANA ;
.
lf:landform-pattern-BAD
  a skos:Concept ;
  skos-ext:isMemberOf lf:landform-pattern-glossary ;
  skos-ext:relatedCollection lf:landform-pattern-BAD-comparewith-patterns ;
  skos-ext:relatedCollection lf:landform-pattern-BAD-occasional-elements ;
  skos-ext:relatedCollection lf:landform-pattern-BAD-typical-elements ;
  dcterms:identifier "http://anzsoil.org/def/au/asls/landform/landform-pattern-BAD"^^xsd:anyURI ;
  skos:definition """landform pattern of low to extremely low relief (less than 90 m) and steep to precipitous slopes, typically with numerous fixed, erosional stream channels which form a non-directional, integrated tributary network. There is continuously active erosion by collapse, landslide, sheet flow, creep and channelled stream flow. 
Typical elements: ridge (dominant), stream bed or gully.
Occasional elements: summit surface, hillcrest, hillslope, talus.
Compare with mountains, hills, low hills, rises and plain."""@en ;
  skos:inScheme asls:landform ;
  skos:notation "BAD" ;
  skos:prefLabel "Badlands"@en ;
  skos:related lf:relief-class-L ;
  skos:related lf:relief-class-P ;
  skos:related lf:relief-class-R ;
  skos:related lf:slope-class-PR ;
  skos:related lf:slope-class-ST ;
  skos:related lf:slope-class-VS ;
  skos:topConceptOf asls:landform ;
.
lf:landform-pattern-BAD-comparewith-patterns
  a skos:Collection ;
  dcterms:identifier "http://anzsoil.org/def/au/asls/landform/landform-pattern-BAD-comparewith-patterns"^^xsd:anyURI ;
  skos:member lf:landform-pattern-HIL ;
  skos:member lf:landform-pattern-LOW ;
  skos:member lf:landform-pattern-PLA ;
  skos:member lf:landform-pattern-RIS ;
  skos:prefLabel "Compare Badlands with these patterns"@en ;
  skos:related lf:landform-pattern-BAD ;
.
lf:landform-pattern-BAD-occasional-elements
  a skos:Collection ;
  dcterms:identifier "http://anzsoil.org/def/au/asls/landform/landform-pattern-ANA-occasional-elements"^^xsd:anyURI ;
  skos:member lf:landform-element-HCR ;
  skos:member lf:landform-element-HSL ;
  skos:member lf:landform-element-SUS ;
  skos:member lf:landform-element-TAL ;
  skos:prefLabel "Occasional elements of Badlands"@en ;
  skos:related lf:landform-pattern-BAD ;
.
lf:landform-pattern-BAD-typical-elements
  a skos:Collection ;
  dcterms:identifier "http://anzsoil.org/def/au/asls/landform/landform-pattern-BAD-typical-elements"^^xsd:anyURI ;
  skos:member lf:landform-element-GUL ;
  skos:member lf:landform-element-STB ;
  skos:member lf:morphological-type-R ;
  skos:prefLabel "Typical elements of Badlands"@en ;
  skos:related lf:landform-pattern-BAD ;
.
lf:landform-pattern-BAR
  a skos:Concept ;
  skos-ext:isMemberOf lf:landform-pattern-glossary ;
  skos-ext:relatedCollection lf:landform-pattern-BAR-comparewith-patterns ;
  skos-ext:relatedCollection lf:landform-pattern-BAR-typical-elements ;
  dcterms:identifier "http://anzsoil.org/def/au/asls/landform/landform-pattern-BAR"^^xsd:anyURI ;
  skos:definition """flood plain with numerous rapidly migrating, shallow alluvial channels forming a unidirectional, integrated reticulated network. There is frequently active aggradation and erosion by channelled stream flow. (Described by Melton 1936.) 
Typical elements: stream bed, bar (dominant).
Compare with other types under alluvial plain and flood plain."""@en ;
  skos:inScheme asls:landform ;
  skos:notation "BAR" ;
  skos:prefLabel "Bar plain"@en ;
  skos:topConceptOf asls:landform ;
.
lf:landform-pattern-BAR-comparewith-patterns
  a skos:Collection ;
  dcterms:identifier "http://anzsoil.org/def/au/asls/landform/landform-pattern-BAR-comparewith-patterns"^^xsd:anyURI ;
  skos:member lf:landform-pattern-ALP ;
  skos:member lf:landform-pattern-FLO ;
  skos:prefLabel "Compare Bar plain with these patterns"@en ;
  skos:related lf:landform-pattern-BAR ;
.
lf:landform-pattern-BAR-typical-elements
  a skos:Collection ;
  dcterms:identifier "http://anzsoil.org/def/au/asls/landform/landform-pattern-BAR-typical-elements"^^xsd:anyURI ;
  skos:member lf:landform-element-BAR ;
  skos:member lf:landform-element-STB ;
  skos:prefLabel "Typical elements of Bar plain"@en ;
  skos:related lf:landform-pattern-BAR ;
.
lf:landform-pattern-BEA
  a skos:Concept ;
  skos-ext:isMemberOf lf:landform-pattern-glossary ;
  skos-ext:relatedCollection lf:landform-pattern-BEA-common-elements ;
  skos-ext:relatedCollection lf:landform-pattern-BEA-comparewith-patterns ;
  skos-ext:relatedCollection lf:landform-pattern-BEA-typical-elements ;
  dcterms:identifier "http://anzsoil.org/def/au/asls/landform/landform-pattern-BEA"^^xsd:anyURI ;
  skos:definition """level to gently undulating landform pattern of extremely low relief on which stream channels are absent or very rare; it consists of relict, parallel beach ridges. 
Typical elements: beach ridge (co-dominant), swale (co-dominant).
Common elements: beach, foredune, tidal creek.
Compare with chenier plain."""@en ;
  skos:inScheme asls:landform ;
  skos:notation "BEA" ;
  skos:prefLabel "Beach ridge plain"@en ;
  skos:related lf:relief-class-P ;
  skos:related lf:slope-class-LE ;
  skos:related lf:slope-class-VG ;
  skos:topConceptOf asls:landform ;
.
lf:landform-pattern-BEA-common-elements
  a skos:Collection ;
  dcterms:identifier "http://anzsoil.org/def/au/asls/landform/landform-pattern-BEA-common-elements"^^xsd:anyURI ;
  skos:member lf:landform-element-BEA ;
  skos:member lf:landform-element-FOR ;
  skos:member lf:landform-element-TDC ;
  skos:prefLabel "Common elements of Beach ridge plain"@en ;
  skos:related lf:landform-pattern-BEA ;
.
lf:landform-pattern-BEA-comparewith-patterns
  a skos:Collection ;
  dcterms:identifier "http://anzsoil.org/def/au/asls/landform/landform-pattern-BEA-comparewith-patterns"^^xsd:anyURI ;
  skos:member lf:landform-pattern-CHE ;
  skos:prefLabel "Compare Beach ridge plain with these patterns"@en ;
  skos:related lf:landform-pattern-BEA ;
.
lf:landform-pattern-BEA-typical-elements
  a skos:Collection ;
  dcterms:identifier "http://anzsoil.org/def/au/asls/landform/landform-pattern-BEA-typical-elements"^^xsd:anyURI ;
  skos:member lf:landform-element-BRI ;
  skos:member lf:landform-element-SWL ;
  skos:prefLabel "Typical elements of Beach ridge plain"@en ;
  skos:related lf:landform-pattern-BEA ;
.
lf:landform-pattern-CAL
  a skos:Concept ;
  skos-ext:isMemberOf lf:landform-pattern-glossary ;
  skos-ext:relatedCollection lf:landform-pattern-CAL-occasional-elements ;
  skos-ext:relatedCollection lf:landform-pattern-CAL-typical-elements ;
  dcterms:identifier "http://anzsoil.org/def/au/asls/landform/landform-pattern-CAL"^^xsd:anyURI ;
  skos:definition """rare landform pattern typically of very high relief and steep to precipitous slope. It is without stream channels or has fixed, erosional channels forming a centripetal, integrated tributary pattern. The landform has subsided or was excavated as a result of volcanism. 
rare landform pattern typically of very high relief and steep to precipitous slope. It is without stream channels or has fixed, erosional channels forming a centripetal, integrated tributary pattern. The landform has subsided or was excavated as a result of volcanism.
Typical elements: scarp, hillslope, lake.
Occasional elements: cone, hillcrest, stream channel."""@en ;
  skos:inScheme asls:landform ;
  skos:notation "CAL" ;
  skos:prefLabel "Caldera"@en ;
  skos:related lf:relief-class-M ;
  skos:related lf:slope-class-PR ;
  skos:related lf:slope-class-ST ;
  skos:related lf:slope-class-VS ;
  skos:topConceptOf asls:landform ;
.
lf:landform-pattern-CAL-occasional-elements
  a skos:Collection ;
  dcterms:identifier "http://anzsoil.org/def/au/asls/landform/landform-pattern-CAL-occasional-elements"^^xsd:anyURI ;
  skos:member lf:landform-element-CON ;
  skos:member lf:landform-element-HCR ;
  skos:member lf:landform-element-STC ;
  skos:prefLabel "Occasional elements of Caldera"@en ;
  skos:related lf:landform-pattern-CAL ;
.
lf:landform-pattern-CAL-typical-elements
  a skos:Collection ;
  dcterms:identifier "http://anzsoil.org/def/au/asls/landform/landform-pattern-CAL-typical-elements"^^xsd:anyURI ;
  skos:member lf:landform-element-HSL ;
  skos:member lf:landform-element-LAK ;
  skos:member lf:landform-element-SCA ;
  skos:prefLabel "Typical elements of Caldera"@en ;
  skos:related lf:landform-pattern-CAL ;
.
lf:landform-pattern-CHE
  a skos:Concept ;
  skos-ext:isMemberOf lf:landform-pattern-glossary ;
  skos-ext:relatedCollection lf:landform-pattern-CHE-common-elements ;
  skos-ext:relatedCollection lf:landform-pattern-CHE-comparewith-patterns ;
  skos-ext:relatedCollection lf:landform-pattern-CHE-typical-elements ;
  dcterms:identifier "http://anzsoil.org/def/au/asls/landform/landform-pattern-CHE"^^xsd:anyURI ;
  skos:definition """level to gently undulating landform pattern of extremely low relief on which stream channels are very rare. The pattern consists of relict, parallel, linear ridges built up by waves, separated by, and built over, flats (mud flats) aggraded by tides or over-bank stream flow. 
Typical elements: beach ridge (co-dominant), flat (co-dominant).
Common elements: tidal flat, swamp, beach, foredune, tidal creek.
Compare with beach ridge plain."""@en ;
  skos:inScheme asls:landform ;
  skos:notation "CHE" ;
  skos:prefLabel "Chenier plain"@en ;
  skos:related lf:relief-class-P ;
  skos:related lf:slope-class-GE ;
  skos:related lf:slope-class-LE ;
  skos:related lf:slope-class-VG ;
  skos:topConceptOf asls:landform ;
.
lf:landform-pattern-CHE-common-elements
  a skos:Collection ;
  dcterms:identifier "http://anzsoil.org/def/au/asls/landform/landform-pattern-CHE-common-elements"^^xsd:anyURI ;
  skos:member lf:landform-element-BEA ;
  skos:member lf:landform-element-FOR ;
  skos:member lf:landform-element-SWP ;
  skos:member lf:landform-element-TDC ;
  skos:prefLabel "Common elements of Chenier plain"@en ;
  skos:related lf:landform-pattern-CHE ;
.
lf:landform-pattern-CHE-comparewith-patterns
  a skos:Collection ;
  dcterms:identifier "http://anzsoil.org/def/au/asls/landform/landform-pattern-CHE-comparewith-patterns"^^xsd:anyURI ;
  skos:member lf:landform-pattern-BEA ;
  skos:prefLabel "Compare Chenier plain with these patterns"@en ;
  skos:related lf:landform-pattern-CHE ;
.
lf:landform-pattern-CHE-typical-elements
  a skos:Collection ;
  dcterms:identifier "http://anzsoil.org/def/au/asls/landform/landform-pattern-CHE-typical-elements"^^xsd:anyURI ;
  skos:member lf:landform-element-BRI ;
  skos:member lf:landform-element-TDF ;
  skos:member lf:morphological-type-F ;
  skos:prefLabel "Typical elements of Chenier plain"@en ;
  skos:related lf:landform-pattern-CHE ;
.
lf:landform-pattern-COR
  a skos:Concept ;
  skos-ext:isMemberOf lf:landform-pattern-glossary ;
  skos-ext:relatedCollection lf:landform-pattern-COR-common-elements ;
  skos-ext:relatedCollection lf:landform-pattern-COR-typical-elements ;
  dcterms:identifier "http://anzsoil.org/def/au/asls/landform/landform-pattern-COR"^^xsd:anyURI ;
  skos:definition """continuously active or relict landform pattern built up to the sea level of the present day or of a former time by corals and other organisms. It is mainly level, with moderately inclined to precipitous slopes below the sea level. Stream channels are generally absent, but there may occasionally be fixed, deep, erosional tidal stream channels forming a disintegrated non-tributary pattern. 
Typical elements: reef flat, lagoon, cliff (submarine).
Common elements: beach, beach ridge."""@en ;
  skos:inScheme asls:landform ;
  skos:notation "COR" ;
  skos:prefLabel "Coral reef"@en ;
  skos:related lf:slope-class-LE ;
  skos:related lf:slope-class-MO ;
  skos:related lf:slope-class-PR ;
  skos:related lf:slope-class-ST ;
  skos:related lf:slope-class-VS ;
  skos:topConceptOf asls:landform ;
.
lf:landform-pattern-COR-common-elements
  a skos:Collection ;
  dcterms:identifier "http://anzsoil.org/def/au/asls/landform/landform-pattern-COR-common-elements"^^xsd:anyURI ;
  skos:member lf:landform-element-BEA ;
  skos:member lf:landform-element-BRI ;
  skos:prefLabel "Common elements of Coral reef"@en ;
  skos:related lf:landform-pattern-COR ;
.
lf:landform-pattern-COR-typical-elements
  a skos:Collection ;
  dcterms:identifier "http://anzsoil.org/def/au/asls/landform/landform-pattern-COR-typical-elements"^^xsd:anyURI ;
  skos:member lf:landform-element-CLI ;
  skos:member lf:landform-element-LAG ;
  skos:member lf:landform-element-REF ;
  skos:prefLabel "Typical elements of Coral reef"@en ;
  skos:related lf:landform-pattern-COR ;
.
lf:landform-pattern-COV
  a skos:Concept ;
  skos-ext:isMemberOf lf:landform-pattern-glossary ;
  skos-ext:relatedCollection lf:landform-pattern-COV-common-elements ;
  skos-ext:relatedCollection lf:landform-pattern-COV-comparewith-patterns ;
  skos-ext:relatedCollection lf:landform-pattern-COV-typical-elements ;
  dcterms:identifier "http://anzsoil.org/def/au/asls/landform/landform-pattern-COV"^^xsd:anyURI ;
  skos:definition """flood plain with slowly migrating, deep alluvial channels, usually widely spaced and forming a unidirectional, integrated non-tributary network. There is frequently active aggradation by over-bank stream flow. (Described by Melton 1936.) 
Typical elements: stream channel (stream bed and bank), levee, backplain (dominant).
Common element: swamp.
Compare with other types under alluvial plain and flood plain."""@en ;
  skos:inScheme asls:landform ;
  skos:notation "COV" ;
  skos:prefLabel "Covered plain"@en ;
  skos:topConceptOf asls:landform ;
.
lf:landform-pattern-COV-common-elements
  a skos:Collection ;
  dcterms:identifier "http://anzsoil.org/def/au/asls/landform/landform-pattern-COV-common-elements"^^xsd:anyURI ;
  skos:member lf:landform-element-SWP ;
  skos:prefLabel "Common elements of Covered plain"@en ;
  skos:related lf:landform-pattern-COV ;
.
lf:landform-pattern-COV-comparewith-patterns
  a skos:Collection ;
  dcterms:identifier "http://anzsoil.org/def/au/asls/landform/landform-pattern-COV-comparewith-patterns"^^xsd:anyURI ;
  skos:member lf:landform-pattern-ALP ;
  skos:member lf:landform-pattern-FLO ;
  skos:prefLabel "Compare Covered plain with these patterns"@en ;
  skos:related lf:landform-pattern-COV ;
.
lf:landform-pattern-COV-typical-elements
  a skos:Collection ;
  dcterms:identifier "http://anzsoil.org/def/au/asls/landform/landform-pattern-COV-typical-elements"^^xsd:anyURI ;
  skos:member lf:landform-element-BAN ;
  skos:member lf:landform-element-BKP ;
  skos:member lf:landform-element-LEV ;
  skos:member lf:landform-element-STB ;
  skos:member lf:landform-element-STC ;
  skos:prefLabel "Typical elements of Covered plain"@en ;
  skos:related lf:landform-pattern-COV ;
.
lf:landform-pattern-DEL
  a skos:Concept ;
  skos-ext:isMemberOf lf:landform-pattern-glossary ;
  skos-ext:relatedCollection lf:landform-pattern-DEL-common-elements ;
  skos-ext:relatedCollection lf:landform-pattern-DEL-comparewith-patterns ;
  skos-ext:relatedCollection lf:landform-pattern-DEL-typical-elements ;
  dcterms:identifier "http://anzsoil.org/def/au/asls/landform/landform-pattern-DEL"^^xsd:anyURI ;
  skos:definition """flood plain projecting into a sea or lake, with slowly migrating, deep alluvial channels, usually moderately spaced, typically forming a divergent, integrated distributary network. This landform is aggraded by frequently active over-bank and channelled stream flow that is modified by tides. 
Typical elements: stream channel (stream bed and bank), levee, backplain (co-dominant), swamp (co-dominant), lagoon (co-dominant).
Common elements: beach ridge, swale, beach, estuary, tidal creek.
Compare with other types under alluvial plain, flood plain and chenier plain."""@en ;
  skos:inScheme asls:landform ;
  skos:notation "DEL" ;
  skos:prefLabel "Delta"@en ;
  skos:topConceptOf asls:landform ;
.
lf:landform-pattern-DEL-common-elements
  a skos:Collection ;
  dcterms:identifier "http://anzsoil.org/def/au/asls/landform/landform-pattern-DEL-common-elements"^^xsd:anyURI ;
  skos:member lf:landform-element-BEA ;
  skos:member lf:landform-element-BRI ;
  skos:member lf:landform-element-EST ;
  skos:member lf:landform-element-SWL ;
  skos:member lf:landform-element-TDC ;
  skos:prefLabel "Common elements of Delta"@en ;
  skos:related lf:landform-pattern-DEL ;
.
lf:landform-pattern-DEL-comparewith-patterns
  a skos:Collection ;
  dcterms:identifier "http://anzsoil.org/def/au/asls/landform/landform-pattern-DEL-comparewith-patterns"^^xsd:anyURI ;
  skos:member lf:landform-pattern-ALP ;
  skos:member lf:landform-pattern-CHE ;
  skos:member lf:landform-pattern-FLO ;
  skos:prefLabel "Compare Delta with these patterns"@en ;
  skos:related lf:landform-pattern-DEL ;
.
lf:landform-pattern-DEL-typical-elements
  a skos:Collection ;
  dcterms:identifier "http://anzsoil.org/def/au/asls/landform/landform-pattern-DEL-typical-elements"^^xsd:anyURI ;
  skos:member lf:landform-element-BAN ;
  skos:member lf:landform-element-BKP ;
  skos:member lf:landform-element-LAG ;
  skos:member lf:landform-element-LEV ;
  skos:member lf:landform-element-STB ;
  skos:member lf:landform-element-STC ;
  skos:member lf:landform-element-SWP ;
  skos:prefLabel "Typical elements of Delta"@en ;
  skos:related lf:landform-pattern-DEL ;
.
lf:landform-pattern-DUN
  a skos:Concept ;
  skos-ext:isMemberOf lf:landform-pattern-glossary ;
  skos-ext:relatedCollection lf:landform-pattern-DUN-common-elements ;
  skos-ext:relatedCollection lf:landform-pattern-DUN-included-patterns ;
  skos-ext:relatedCollection lf:landform-pattern-DUN-typical-elements ;
  dcterms:identifier "http://anzsoil.org/def/au/asls/landform/landform-pattern-DUN"^^xsd:anyURI ;
  skos:definition """level to rolling landform pattern of very low or extremely low relief without stream channels, built up or locally excavated, eroded or aggraded by wind. 
Typical elements: dune or dunecrest, duneslope, swale, blow-out, risecrest, residual rise, riseslope.
Common elements: hummocky dune, barchan dune, parabolic dune, linear dune.
Included types of landform pattern are: longitudinal dunefield, parabolic dunefield."""@en ;
  skos:inScheme asls:landform ;
  skos:notation "DUN" ;
  skos:prefLabel "Dunefield"@en ;
  skos:related lf:relief-class-P ;
  skos:related lf:relief-class-R ;
  skos:related lf:slope-class-GE ;
  skos:related lf:slope-class-LE ;
  skos:related lf:slope-class-MO ;
  skos:related lf:slope-class-VG ;
  skos:topConceptOf asls:landform ;
.
lf:landform-pattern-DUN-common-elements
  a skos:Collection ;
  dcterms:identifier "http://anzsoil.org/def/au/asls/landform/landform-pattern-DUN-common-elements"^^xsd:anyURI ;
  skos:member lf:landform-element-DUB ;
  skos:member lf:landform-element-DUF ;
  skos:member lf:landform-element-DUH ;
  skos:member lf:landform-element-DUP ;
  skos:prefLabel "Common elements of Dunefield"@en ;
  skos:related lf:landform-pattern-DUN ;
.
lf:landform-pattern-DUN-included-patterns
  a skos:Collection ;
  dcterms:identifier "http://anzsoil.org/def/au/asls/landform/landform-pattern-DUN-included-patterns"^^xsd:anyURI ;
  skos:member lf:landform-pattern-LON ;
  skos:member lf:landform-pattern-PAR ;
  skos:prefLabel "Included patterns of Dunefield"@en ;
  skos:related lf:landform-pattern-DUN ;
.
lf:landform-pattern-DUN-typical-elements
  a skos:Collection ;
  dcterms:identifier "http://anzsoil.org/def/au/asls/landform/landform-pattern-DUN-typical-elements"^^xsd:anyURI ;
  skos:member lf:landform-element-BOU ;
  skos:member lf:landform-element-DUC ;
  skos:member lf:landform-element-DUN ;
  skos:member lf:landform-element-DUS ;
  skos:member lf:landform-element-REC ;
  skos:member lf:landform-element-RER ;
  skos:member lf:landform-element-RES ;
  skos:member lf:landform-element-SWL ;
  skos:prefLabel "Typical elements of Dunefield"@en ;
  skos:related lf:landform-pattern-DUN ;
.
lf:landform-pattern-ESC
  a skos:Concept ;
  skos-ext:isMemberOf lf:landform-pattern-glossary ;
  skos-ext:relatedCollection lf:landform-pattern-ESC-common-elements ;
  skos-ext:relatedCollection lf:landform-pattern-ESC-occasional-elements ;
  skos-ext:relatedCollection lf:landform-pattern-ESC-typical-elements ;
  dcterms:identifier "http://anzsoil.org/def/au/asls/landform/landform-pattern-ESC"^^xsd:anyURI ;
  skos:definition """steep to precipitous landform pattern forming a linearly extensive, straight or sinuous, inclined surface, which separates terrains at different altitudes; a plateau is commonly above the escarpment. Relief within the landform pattern may be high (hilly) or low (planar). The upper margin is often marked by an included cliff or scarp. 
Typical elements: hillcrest, hillslope, cliff-footslope.
Common elements: cliff, scarp, scarp-footslope, talus, footslope, alcove.
Occasional element: stream bed."""@en ;
  skos:inScheme asls:landform ;
  skos:notation "ESC" ;
  skos:prefLabel "Escarpment"@en ;
  skos:related lf:relief-class-H ;
  skos:related lf:relief-class-L ;
  skos:related lf:slope-class-PR ;
  skos:related lf:slope-class-ST ;
  skos:related lf:slope-class-VS ;
  skos:topConceptOf asls:landform ;
.
lf:landform-pattern-ESC-common-elements
  a skos:Collection ;
  dcterms:identifier "http://anzsoil.org/def/au/asls/landform/landform-pattern-ESC-common-elements"^^xsd:anyURI ;
  skos:member lf:landform-element-ALC ;
  skos:member lf:landform-element-CLI ;
  skos:member lf:landform-element-FOO ;
  skos:member lf:landform-element-SCA ;
  skos:member lf:landform-element-SFS ;
  skos:member lf:landform-element-TAL ;
  skos:prefLabel "Common elements of Escarpment"@en ;
  skos:related lf:landform-pattern-ESC ;
.
lf:landform-pattern-ESC-occasional-elements
  a skos:Collection ;
  dcterms:identifier "http://anzsoil.org/def/au/asls/landform/landform-pattern-ESC-occasional-elements"^^xsd:anyURI ;
  skos:member lf:landform-element-STB ;
  skos:prefLabel "Occasional elements of Escarpment"@en ;
  skos:related lf:landform-pattern-ESC ;
.
lf:landform-pattern-ESC-typical-elements
  a skos:Collection ;
  dcterms:identifier "http://anzsoil.org/def/au/asls/landform/landform-pattern-ESC-typical-elements"^^xsd:anyURI ;
  skos:member lf:landform-element-CFS ;
  skos:member lf:landform-element-HCR ;
  skos:member lf:landform-element-HSL ;
  skos:prefLabel "Typical elements of Escarpment"@en ;
  skos:related lf:landform-pattern-ESC ;
.
lf:landform-pattern-FLO
  a skos:Concept ;
  skos-ext:isMemberOf lf:landform-pattern-glossary ;
  skos-ext:relatedCollection lf:landform-pattern-FLO-common-elements ;
  skos-ext:relatedCollection lf:landform-pattern-FLO-included-patterns ;
  skos-ext:relatedCollection lf:landform-pattern-FLO-occasional-elements ;
  skos-ext:relatedCollection lf:landform-pattern-FLO-related-patterns ;
  skos-ext:relatedCollection lf:landform-pattern-FLO-typical-elements ;
  dcterms:identifier "http://anzsoil.org/def/au/asls/landform/landform-pattern-FLO"^^xsd:anyURI ;
  skos:definition """alluvial plain characterised by frequently active erosion and aggradation by channelled or over-bank stream flow. Unless otherwise specified, ‘frequently active’ is to mean that flow has an Average Recurrence Interval of 50 years or less. 
Typical elements: stream channel (stream bed and bank), plain (dominant).
Common elements: bar, scroll, levee, backplain, swamp.
Occasional elements: ox-bow, flood-out, scroll.
Included types of landform pattern are: bar plain, meander plain, covered plain, anastomotic plain.
Related relict landform patterns are: stagnant alluvial plain, terrace, terraced land (partly relict)."""@en ;
  skos:inScheme asls:landform ;
  skos:notation "FLO" ;
  skos:prefLabel "Food plain"@en ;
  skos:topConceptOf asls:landform ;
.
lf:landform-pattern-FLO-common-elements
  a skos:Collection ;
  dcterms:identifier "http://anzsoil.org/def/au/asls/landform/landform-pattern-FLO-common-elements"^^xsd:anyURI ;
  skos:member lf:landform-element-BAR ;
  skos:member lf:landform-element-BKP ;
  skos:member lf:landform-element-LEV ;
  skos:member lf:landform-element-SCR ;
  skos:member lf:landform-element-SWP ;
  skos:prefLabel "Common elements of Flood plain"@en ;
  skos:related lf:landform-pattern-FLO ;
.
lf:landform-pattern-FLO-included-patterns
  a skos:Collection ;
  dcterms:identifier "http://anzsoil.org/def/au/asls/landform/landform-pattern-FLO-included-patterns"^^xsd:anyURI ;
  skos:member lf:landform-pattern-ANA ;
  skos:member lf:landform-pattern-BAR ;
  skos:member lf:landform-pattern-COV ;
  skos:member lf:landform-pattern-MEA ;
  skos:prefLabel "Included patterns of Flood plain"@en ;
  skos:related lf:landform-pattern-FLO ;
.
lf:landform-pattern-FLO-occasional-elements
  a skos:Collection ;
  dcterms:identifier "http://anzsoil.org/def/au/asls/landform/landform-pattern-FLO-occasional-elements"^^xsd:anyURI ;
  skos:member lf:landform-element-FLD ;
  skos:member lf:landform-element-OXB ;
  skos:prefLabel "Occasional elements of Flood plain"@en ;
  skos:related lf:landform-pattern-FLO ;
.
lf:landform-pattern-FLO-related-patterns
  a skos:Collection ;
  dcterms:identifier "http://anzsoil.org/def/au/asls/landform/landform-pattern-FLO-related-patterns"^^xsd:anyURI ;
  skos:member lf:landform-pattern-STA ;
  skos:member lf:landform-pattern-TEL ;
  skos:member lf:landform-pattern-TER ;
  skos:prefLabel "Related relic patterns of Flood plain"@en ;
  skos:related lf:landform-pattern-FLO ;
.
lf:landform-pattern-FLO-typical-elements
  a skos:Collection ;
  dcterms:identifier "http://anzsoil.org/def/au/asls/landform/landform-pattern-FLO-typical-elements"^^xsd:anyURI ;
  skos:member lf:landform-element-BAN ;
  skos:member lf:landform-element-PLA ;
  skos:member lf:landform-element-STB ;
  skos:member lf:landform-element-STC ;
  skos:prefLabel "Typical elements of Flood plain"@en ;
  skos:related lf:landform-pattern-FLO ;
.
lf:landform-pattern-HIL
  a skos:Concept ;
  skos-ext:isMemberOf lf:landform-pattern-glossary ;
  skos-ext:relatedCollection lf:landform-pattern-HIL-common-elements ;
  skos-ext:relatedCollection lf:landform-pattern-HIL-comparewith-patterns ;
  skos-ext:relatedCollection lf:landform-pattern-HIL-occasional-elements ;
  skos-ext:relatedCollection lf:landform-pattern-HIL-typical-elements ;
  dcterms:identifier "http://anzsoil.org/def/au/asls/landform/landform-pattern-HIL"^^xsd:anyURI ;
  skos:definition """landform pattern of high relief (90–300 m) with gently inclined to precipitous slopes. Fixed, shallow, erosional stream channels, closely to very widely spaced, form a non-directional or convergent, integrated tributary network. There is continuously active erosion by wash and creep and, in some cases, rarely active erosion by landslides. 
Typical elements: hillcrest, hillslope (dominant), drainage depression, stream bed.
Common elements: footslope, alcove, valley flat, gully.
Occasional elements: tor, summit surface, scarp, landslide, talus, bench, terrace, doline.
Compare with mountains, low hills, rises and plain."""@en ;
  skos:inScheme asls:landform ;
  skos:notation "HIL" ;
  skos:prefLabel "Hills"@en ;
  skos:related lf:relief-class-H ;
  skos:related lf:slope-class-GE ;
  skos:related lf:slope-class-MO ;
  skos:related lf:slope-class-PR ;
  skos:related lf:slope-class-ST ;
  skos:related lf:slope-class-VS ;
  skos:topConceptOf asls:landform ;
.
lf:landform-pattern-HIL-common-elements
  a skos:Collection ;
  dcterms:identifier "http://anzsoil.org/def/au/asls/landform/landform-pattern-HIL-common-elements"^^xsd:anyURI ;
  skos:member lf:landform-element-ALC ;
  skos:member lf:landform-element-FOO ;
  skos:member lf:landform-element-GUL ;
  skos:member lf:landform-element-VLF ;
  skos:prefLabel "Common elements of Hills"@en ;
  skos:related lf:landform-pattern-HIL ;
.
lf:landform-pattern-HIL-comparewith-patterns
  a skos:Collection ;
  dcterms:identifier "http://anzsoil.org/def/au/asls/landform/landform-pattern-HIL-included-patterns"^^xsd:anyURI ;
  skos:member lf:landform-pattern-LOW ;
  skos:member lf:landform-pattern-PLA ;
  skos:member lf:landform-pattern-RIS ;
  skos:prefLabel "Compare Hills with these patterns"@en ;
  skos:related lf:landform-pattern-HIL ;
.
lf:landform-pattern-HIL-occasional-elements
  a skos:Collection ;
  dcterms:identifier "http://anzsoil.org/def/au/asls/landform/landform-pattern-HIL-occasional-elements"^^xsd:anyURI ;
  skos:member lf:landform-element-BEN ;
  skos:member lf:landform-element-DOC ;
  skos:member lf:landform-element-LDS ;
  skos:member lf:landform-element-SCA ;
  skos:member lf:landform-element-SUS ;
  skos:member lf:landform-element-TAL ;
  skos:member lf:landform-element-TOR ;
  skos:prefLabel "Occasional elements of Hills"@en ;
  skos:related lf:landform-pattern-HIL ;
.
lf:landform-pattern-HIL-typical-elements
  a skos:Collection ;
  dcterms:identifier "http://anzsoil.org/def/au/asls/landform/landform-pattern-HIL-typical-elements"^^xsd:anyURI ;
  skos:member lf:landform-element-DDE ;
  skos:member lf:landform-element-HCR ;
  skos:member lf:landform-element-HSL ;
  skos:member lf:landform-element-STB ;
  skos:prefLabel "Typical elements of Hills"@en ;
  skos:related lf:landform-pattern-HIL ;
.
lf:landform-pattern-KAR
  a skos:Concept ;
  skos-ext:isMemberOf lf:landform-pattern-glossary ;
  skos-ext:relatedCollection lf:landform-pattern-KAR-common-elements ;
  skos-ext:relatedCollection lf:landform-pattern-KAR-occasional-elements ;
  skos-ext:relatedCollection lf:landform-pattern-KAR-typical-elements ;
  dcterms:identifier "http://anzsoil.org/def/au/asls/landform/landform-pattern-KAR"^^xsd:anyURI ;
  skos:definition """landform pattern of unspecified relief and slope (for specification use the terms in Table 4, for example ‘Karst rolling hills’) typically with fixed, deep, erosional stream channels forming a non-directional, disintegrated tributary pattern and many closed depressions without stream channels. It is eroded by continuously active solution and rarely active collapse, the products being removed through underground channels. 
Typical elements: hillcrest, hillslope (dominant), doline.
Common elements: summit surface, valley flat, plain, alcove, drainage depression, stream channel, scarp, footslope, landslide.
Occasional element: talus."""@en ;
  skos:inScheme asls:landform ;
  skos:notation "KAR" ;
  skos:prefLabel "Karst"@en ;
  skos:topConceptOf asls:landform ;
.
lf:landform-pattern-KAR-common-elements
  a skos:Collection ;
  dcterms:identifier "http://anzsoil.org/def/au/asls/landform/landform-pattern-KAR-common-elements"^^xsd:anyURI ;
  skos:member lf:landform-element-ALC ;
  skos:member lf:landform-element-DDE ;
  skos:member lf:landform-element-FOO ;
  skos:member lf:landform-element-LDS ;
  skos:member lf:landform-element-PLA ;
  skos:member lf:landform-element-SCA ;
  skos:member lf:landform-element-STC ;
  skos:member lf:landform-element-SUS ;
  skos:member lf:landform-element-VLF ;
  skos:prefLabel "Common elements of Karst"@en ;
  skos:related lf:landform-pattern-KAR ;
.
lf:landform-pattern-KAR-occasional-elements
  a skos:Collection ;
  dcterms:identifier "http://anzsoil.org/def/au/asls/landform/landform-pattern-KAR-occasional-elements"^^xsd:anyURI ;
  skos:member lf:landform-element-TAL ;
  skos:prefLabel "Occasional elements of Karst"@en ;
  skos:related lf:landform-pattern-KAR ;
.
lf:landform-pattern-KAR-typical-elements
  a skos:Collection ;
  dcterms:identifier "http://anzsoil.org/def/au/asls/landform/landform-pattern-KAR-typical-elements"^^xsd:anyURI ;
  skos:member lf:landform-element-DOC ;
  skos:member lf:landform-element-HCR ;
  skos:member lf:landform-element-HSL ;
  skos:prefLabel "Typical elements of Karst"@en ;
  skos:related lf:landform-pattern-KAR ;
.
lf:landform-pattern-LAC
  a skos:Concept ;
  skos-ext:isMemberOf lf:landform-pattern-glossary ;
  skos-ext:relatedCollection lf:landform-pattern-LAC-common-elements ;
  skos-ext:relatedCollection lf:landform-pattern-LAC-comparewith-patterns ;
  skos-ext:relatedCollection lf:landform-pattern-LAC-occasional-elements ;
  skos-ext:relatedCollection lf:landform-pattern-LAC-typical-elements ;
  dcterms:identifier "http://anzsoil.org/def/au/asls/landform/landform-pattern-LAC"^^xsd:anyURI ;
  skos:definition """level landform pattern with extremely low relief formerly occupied by a lake but now partly or completely dry. It is relict after aggradation by waves and by deposition of material from suspension and solution in standing water. The pattern is usually bounded by wave-formed features such as cliffs, rock platforms, beaches, berms and lunettes. These may be included or excluded. 
Typical element: plain.
Common elements: beach, cliff.
Occasional elements: rock platform, berm.
Compare with playa plain."""@en ;
  skos:inScheme asls:landform ;
  skos:notation "LAC" ;
  skos:prefLabel "Lacustrine plain"@en ;
  skos:related lf:relief-class-P ;
  skos:related lf:slope-class-LE ;
  skos:topConceptOf asls:landform ;
.
lf:landform-pattern-LAC-common-elements
  a skos:Collection ;
  dcterms:identifier "http://anzsoil.org/def/au/asls/landform/landform-pattern-LAC-common-elements"^^xsd:anyURI ;
  skos:member lf:landform-element-BEA ;
  skos:member lf:landform-element-CLI ;
  skos:prefLabel "Common elements of Lacustrine plain"@en ;
  skos:related lf:landform-pattern-LAC ;
.
lf:landform-pattern-LAC-comparewith-patterns
  a skos:Collection ;
  dcterms:identifier "http://anzsoil.org/def/au/asls/landform/landform-pattern-LAC-comparewith-patterns"^^xsd:anyURI ;
  skos:member lf:landform-pattern-PLY ;
  skos:prefLabel "Compare Lacustrine plain with these patterns"@en ;
  skos:related lf:landform-pattern-LAC ;
.
lf:landform-pattern-LAC-occasional-elements
  a skos:Collection ;
  dcterms:identifier "http://anzsoil.org/def/au/asls/landform/landform-pattern-LAC-occasional-elements"^^xsd:anyURI ;
  skos:member lf:landform-element-BER ;
  skos:member lf:landform-element-RPL ;
  skos:prefLabel "Occasional elements of Lacustrine plain"@en ;
  skos:related lf:landform-pattern-LAC ;
.
lf:landform-pattern-LAC-typical-elements
  a skos:Collection ;
  dcterms:identifier "http://anzsoil.org/def/au/asls/landform/landform-pattern-LAC-typical-elements"^^xsd:anyURI ;
  skos:member lf:landform-element-PLA ;
  skos:prefLabel "Typical elements of Lacustrine plain"@en ;
  skos:related lf:landform-pattern-LAC ;
.
lf:landform-pattern-LAV
  a skos:Concept ;
  skos-ext:isMemberOf lf:landform-pattern-glossary ;
  skos-ext:relatedCollection lf:landform-pattern-LAV-common-elements ;
  skos-ext:relatedCollection lf:landform-pattern-LAV-typical-elements ;
  dcterms:identifier "http://anzsoil.org/def/au/asls/landform/landform-pattern-LAV"^^xsd:anyURI ;
  skos:definition """level to undulating landform pattern of very low to extremely low relief typically with widely spaced, fixed, erosional stream channels that form a non-directional, integrated or interrupted tributary pattern. The landform pattern is aggraded by volcanism (lava flow) that is generally relict; it is subject to erosion by continuously active sheet flow, creep, and channelled stream flow. 
Typical elements: plain, hillslope, stream bed.
Occasional element: tumulus."""@en ;
  skos:inScheme asls:landform ;
  skos:notation "LAV" ;
  skos:prefLabel "Lava plain"@en ;
  skos:related lf:relief-class-L ;
  skos:related lf:relief-class-P ;
  skos:related lf:relief-class-R ;
  skos:related lf:slope-class-GE ;
  skos:related lf:slope-class-LE ;
  skos:related lf:slope-class-VG ;
  skos:topConceptOf asls:landform ;
.
lf:landform-pattern-LAV-common-elements
  a skos:Collection ;
  dcterms:identifier "http://anzsoil.org/def/au/asls/landform/landform-pattern-LAV-common-elements"^^xsd:anyURI ;
  skos:member lf:landform-element-TUM ;
  skos:prefLabel "Common elements of Lava plain"@en ;
  skos:related lf:landform-pattern-LAV ;
.
lf:landform-pattern-LAV-typical-elements
  a skos:Collection ;
  dcterms:identifier "http://anzsoil.org/def/au/asls/landform/landform-pattern-LAV-typical-elements"^^xsd:anyURI ;
  skos:member lf:landform-element-HSL ;
  skos:member lf:landform-element-PLA ;
  skos:member lf:landform-element-STB ;
  skos:prefLabel "Typical elements of Lava plain"@en ;
  skos:related lf:landform-pattern-LAV ;
.
lf:landform-pattern-LON
  a skos:Concept ;
  skos-ext:isMemberOf lf:landform-pattern-glossary ;
  skos-ext:relatedCollection lf:landform-pattern-LON-comparewith-patterns ;
  skos-ext:relatedCollection lf:landform-pattern-LON-typical-elements ;
  dcterms:identifier "http://anzsoil.org/def/au/asls/landform/landform-pattern-LON"^^xsd:anyURI ;
  skos:definition """dunefield characterised by long, narrow sand dunes and wide, flat swales. The dunes are oriented parallel with the direction of the prevailing wind, and in cross-section one slope is typically steeper than the other. 
Typical elements: dune or dunecrest, duneslope, swale, blow-out.
Compare with parabolic dunefield."""@en ;
  skos:inScheme asls:landform ;
  skos:notation "LON" ;
  skos:prefLabel "Longitudinal dunefield"@en ;
  skos:topConceptOf asls:landform ;
.
lf:landform-pattern-LON-comparewith-patterns
  a skos:Collection ;
  dcterms:identifier "http://anzsoil.org/def/au/asls/landform/landform-pattern-LON-comparewith-patterns"^^xsd:anyURI ;
  skos:member lf:landform-pattern-PAR ;
  skos:prefLabel "Compare Longitudinal dunefield with these patterns"@en ;
  skos:related lf:landform-pattern-LON ;
.
lf:landform-pattern-LON-typical-elements
  a skos:Collection ;
  dcterms:identifier "http://anzsoil.org/def/au/asls/landform/landform-pattern-LON-typical-elements"^^xsd:anyURI ;
  skos:member lf:landform-element-BOU ;
  skos:member lf:landform-element-DUC ;
  skos:member lf:landform-element-DUN ;
  skos:member lf:landform-element-DUS ;
  skos:member lf:landform-element-SWL ;
  skos:prefLabel "Typical elements of Longitudinal dunefield"@en ;
  skos:related lf:landform-pattern-LON ;
.
lf:landform-pattern-LOW
  a skos:Concept ;
  skos-ext:isMemberOf lf:landform-pattern-glossary ;
  skos-ext:relatedCollection lf:landform-pattern-LOW-common-elements ;
  skos-ext:relatedCollection lf:landform-pattern-LOW-comparewith-patterns ;
  skos-ext:relatedCollection lf:landform-pattern-LOW-occasional-elements ;
  skos-ext:relatedCollection lf:landform-pattern-LOW-typical-elements ;
  dcterms:identifier "http://anzsoil.org/def/au/asls/landform/landform-pattern-LOW"^^xsd:anyURI ;
  skos:definition """landform pattern of low relief (30–90 m) and gentle to very steep slopes, typically with fixed, erosional stream channels, closely to very widely spaced, which form a non-directional or convergent, integrated tributary pattern. There is continuously active sheet flow, creep, and channelled stream flow.  
Typical elements: hillcrest, hillslope (dominant), drainage depression, stream bed.
Common elements: footslope, alcove, valley flat, gully.
Occasional elements: tor, summit surface, landslide, doline.
Compare with mountains, hills, rises and plain."""@en ;
  skos:inScheme asls:landform ;
  skos:notation "LOW" ;
  skos:prefLabel "Low hills"@en ;
  skos:related lf:relief-class-L ;
  skos:related lf:slope-class-GE ;
  skos:related lf:slope-class-MO ;
  skos:related lf:slope-class-ST ;
  skos:related lf:slope-class-VS ;
  skos:topConceptOf asls:landform ;
.
lf:landform-pattern-LOW-common-elements
  a skos:Collection ;
  dcterms:identifier "http://anzsoil.org/def/au/asls/landform/landform-pattern-LOW-common-elements"^^xsd:anyURI ;
  skos:member lf:landform-element-ALC ;
  skos:member lf:landform-element-FOO ;
  skos:member lf:landform-element-GUL ;
  skos:member lf:landform-element-VLF ;
  skos:prefLabel "Common elements of Low hills"@en ;
  skos:related lf:landform-pattern-LOW ;
.
lf:landform-pattern-LOW-comparewith-patterns
  a skos:Collection ;
  dcterms:identifier "http://anzsoil.org/def/au/asls/landform/landform-pattern-LOW-comparewith-patterns"^^xsd:anyURI ;
  skos:member lf:landform-pattern-HIL ;
  skos:member lf:landform-pattern-PLA ;
  skos:member lf:landform-pattern-RIS ;
  skos:prefLabel "Compare Low hills with these patterns"@en ;
  skos:related lf:landform-pattern-LOW ;
.
lf:landform-pattern-LOW-occasional-elements
  a skos:Collection ;
  dcterms:identifier "http://anzsoil.org/def/au/asls/landform/landform-pattern-LOW-occasional-elements"^^xsd:anyURI ;
  skos:member lf:landform-element-DOC ;
  skos:member lf:landform-element-LDS ;
  skos:member lf:landform-element-SUS ;
  skos:member lf:landform-element-TOR ;
  skos:prefLabel "Occasional elements of Low hills"@en ;
  skos:related lf:landform-pattern-LOW ;
.
lf:landform-pattern-LOW-typical-elements
  a skos:Collection ;
  dcterms:identifier "http://anzsoil.org/def/au/asls/landform/landform-pattern-LOW-typical-elements"^^xsd:anyURI ;
  skos:member lf:landform-element-DDE ;
  skos:member lf:landform-element-HCR ;
  skos:member lf:landform-element-HSL ;
  skos:member lf:landform-element-STB ;
  skos:prefLabel "Typical elements of Low hills"@en ;
  skos:related lf:landform-pattern-LOW ;
.
lf:landform-pattern-MAD
  a skos:Concept ;
  skos-ext:isMemberOf lf:landform-pattern-glossary ;
  skos-ext:relatedCollection lf:landform-pattern-MAD-common-elements ;
  skos-ext:relatedCollection lf:landform-pattern-MAD-typical-elements ;
  dcterms:identifier "http://anzsoil.org/def/au/asls/landform/landform-pattern-MAD"^^xsd:anyURI ;
  skos:definition """landform pattern typically of very low or extremely low relief and with slopes either level or very steep. Sparse, fixed, deep, artificial stream channels form a non-directional, interrupted tributary pattern. The landform pattern is eroded and aggraded, and locally built up or excavated, by rarely active human agency. 
Typical elements: fill-top (dominant), cut-over surface, cut face, embankment, berm, trench.
Common elements: mound, pit, dam."""@en ;
  skos:inScheme asls:landform ;
  skos:notation "MAD" ;
  skos:prefLabel "Made land"@en ;
  skos:related lf:relief-class-P ;
  skos:related lf:relief-class-R ;
  skos:related lf:slope-class-LE ;
  skos:related lf:slope-class-VS ;
  skos:topConceptOf asls:landform ;
.
lf:landform-pattern-MAD-common-elements
  a skos:Collection ;
  dcterms:identifier "http://anzsoil.org/def/au/asls/landform/landform-pattern-MAD-common-elements"^^xsd:anyURI ;
  skos:member lf:landform-element-DAM ;
  skos:member lf:landform-element-MOU ;
  skos:member lf:landform-element-PIT ;
  skos:prefLabel "Common elements of Made land"@en ;
  skos:related lf:landform-pattern-MAD ;
.
lf:landform-pattern-MAD-typical-elements
  a skos:Collection ;
  dcterms:identifier "http://anzsoil.org/def/au/asls/landform/landform-pattern-MAD-typical-elements"^^xsd:anyURI ;
  skos:member lf:landform-element-BER ;
  skos:member lf:landform-element-COS ;
  skos:member lf:landform-element-CUT ;
  skos:member lf:landform-element-EMB ;
  skos:member lf:landform-element-FIL ;
  skos:member lf:landform-element-TRE ;
  skos:prefLabel "Typical elements of Made land"@en ;
  skos:related lf:landform-pattern-MAD ;
.
lf:landform-pattern-MAR
  a skos:Concept ;
  skos-ext:isMemberOf lf:landform-pattern-glossary ;
  skos-ext:relatedCollection lf:landform-pattern-MAR-occasional-elements ;
  skos-ext:relatedCollection lf:landform-pattern-MAR-typical-elements ;
  dcterms:identifier "http://anzsoil.org/def/au/asls/landform/landform-pattern-MAR"^^xsd:anyURI ;
  skos:definition """plain eroded or aggraded by waves, tides, or submarine currents, and aggraded by deposition of material from suspension and solution in sea water, elevated above sea level by earth movements or eustasy, and little modified by subaerial agents such as stream flow or wind. 
Typical element: plain.
Occasional elements: dune, stream channel."""@en ;
  skos:inScheme asls:landform ;
  skos:notation "MAR" ;
  skos:prefLabel "Marine plain"@en ;
  skos:topConceptOf asls:landform ;
.
lf:landform-pattern-MAR-occasional-elements
  a skos:Collection ;
  dcterms:identifier "http://anzsoil.org/def/au/asls/landform/landform-pattern-MAR-occasional-elements"^^xsd:anyURI ;
  skos:member lf:landform-element-DUN ;
  skos:member lf:landform-element-STC ;
  skos:prefLabel "Occasional elements of Marine plain"@en ;
  skos:related lf:landform-pattern-MAR ;
.
lf:landform-pattern-MAR-typical-elements
  a skos:Collection ;
  dcterms:identifier "http://anzsoil.org/def/au/asls/landform/landform-pattern-MAR-typical-elements"^^xsd:anyURI ;
  skos:member lf:landform-element-PLA ;
  skos:prefLabel "Typical elements of Marine plain"@en ;
  skos:related lf:landform-pattern-MAR ;
.
lf:landform-pattern-MEA
  a skos:Concept ;
  skos-ext:isMemberOf lf:landform-pattern-glossary ;
  skos-ext:relatedCollection lf:landform-pattern-MEA-common-elements ;
  skos-ext:relatedCollection lf:landform-pattern-MEA-comparewith-patterns ;
  skos-ext:relatedCollection lf:landform-pattern-MEA-typical-elements ;
  dcterms:identifier "http://anzsoil.org/def/au/asls/landform/landform-pattern-MEA"^^xsd:anyURI ;
  skos:definition """flood plain with widely spaced, rapidly migrating, moderately deep alluvial stream channels which form a unidirectional, integrated non-tributary network. There is frequently active aggradation and erosion by channelled stream flow with subordinate aggradation by over-bank stream flow. (Described by Melton 1936.) 
Typical elements: stream channel (stream bed, bank and bar), scroll, scroll plain (dominant).
Common element: ox-bow.
Compare with other types under alluvial plain and flood plain."""@en ;
  skos:inScheme asls:landform ;
  skos:notation "MEA" ;
  skos:prefLabel "Meander plain"@en ;
  skos:topConceptOf asls:landform ;
.
lf:landform-pattern-MEA-common-elements
  a skos:Collection ;
  dcterms:identifier "http://anzsoil.org/def/au/asls/landform/landform-pattern-MEA-common-elements"^^xsd:anyURI ;
  skos:member lf:landform-element-OXB ;
  skos:prefLabel "Common elements of Meander plain"@en ;
  skos:related lf:landform-pattern-MEA ;
.
lf:landform-pattern-MEA-comparewith-patterns
  a skos:Collection ;
  dcterms:identifier "http://anzsoil.org/def/au/asls/landform/landform-pattern-MEA-comparewith-patterns"^^xsd:anyURI ;
  skos:member lf:landform-pattern-ALP ;
  skos:member lf:landform-pattern-FLO ;
  skos:prefLabel "Compare Meander plain with these patterns"@en ;
  skos:related lf:landform-pattern-MEA ;
.
lf:landform-pattern-MEA-typical-elements
  a skos:Collection ;
  dcterms:identifier "http://anzsoil.org/def/au/asls/landform/landform-pattern-MEA-typical-elements"^^xsd:anyURI ;
  skos:member lf:landform-element-BAN ;
  skos:member lf:landform-element-BAR ;
  skos:member lf:landform-element-SCR ;
  skos:member lf:landform-element-SRP ;
  skos:member lf:landform-element-STB ;
  skos:member lf:landform-element-STC ;
  skos:prefLabel "Typical elements of Meander plain"@en ;
  skos:related lf:landform-pattern-MEA ;
.
lf:landform-pattern-MET
  a skos:Concept ;
  skos-ext:isMemberOf lf:landform-pattern-glossary ;
  skos-ext:relatedCollection lf:landform-pattern-MET-typical-elements ;
  dcterms:identifier "http://anzsoil.org/def/au/asls/landform/landform-pattern-MET"^^xsd:anyURI ;
  skos:definition """rare landform pattern comprising a circular closed depression (see crater landform element) with a raised margin; it is typically of low to high relief and has a large range of slope values, without stream channels, or with a peripheral integrated pattern of centrifugal tributary streams. The pattern is excavated, heaved up and built up by a meteor impact and is now relict. 
Typical elements: crater (scarp, talus, footslope and plain), hillcrest, hillslope."""@en ;
  skos:inScheme asls:landform ;
  skos:notation "MET" ;
  skos:prefLabel "Meteor crater"@en ;
  skos:related lf:relief-class-H ;
  skos:related lf:relief-class-L ;
  skos:topConceptOf asls:landform ;
.
lf:landform-pattern-MET-typical-elements
  a skos:Collection ;
  dcterms:identifier "http://anzsoil.org/def/au/asls/landform/landform-pattern-MET-typical-elements"^^xsd:anyURI ;
  skos:member lf:landform-element-CRA ;
  skos:member lf:landform-element-FOO ;
  skos:member lf:landform-element-HCR ;
  skos:member lf:landform-element-HSL ;
  skos:member lf:landform-element-PLA ;
  skos:member lf:landform-element-SCA ;
  skos:member lf:landform-element-TAL ;
  skos:prefLabel "Typical elements of Meteor crater"@en ;
  skos:related lf:landform-pattern-MET ;
.
lf:landform-pattern-MOU
  a skos:Concept ;
  skos-ext:isMemberOf lf:landform-pattern-glossary ;
  skos-ext:relatedCollection lf:landform-pattern-MOU-common-elements ;
  skos-ext:relatedCollection lf:landform-pattern-MOU-comparewith-patterns ;
  skos-ext:relatedCollection lf:landform-pattern-MOU-occasional-elements ;
  skos-ext:relatedCollection lf:landform-pattern-MOU-typical-elements ;
  dcterms:identifier "http://anzsoil.org/def/au/asls/landform/landform-pattern-MOU"^^xsd:anyURI ;
  skos:definition """landform pattern of very high relief (greater than 300 m) with moderate to precipitous slopes and fixed, erosional stream channels that are closely to very widely spaced and form a non-directional or diverging, integrated tributary network. There is continuously active erosion by collapse, landslide, sheet flow, creep, and channelled stream flow. 
Typical elements: hillcrest, hillslope (dominant), stream bed.
Common elements: talus, landslide, alcove, valley flat, scarp.
Occasional elements: cirque, footslope.
Compare with hills, low hills, rises and plain."""@en ;
  skos:inScheme asls:landform ;
  skos:notation "MOU" ;
  skos:prefLabel "Mountains"@en ;
  skos:related lf:relief-class-M ;
  skos:related lf:slope-class-MO ;
  skos:related lf:slope-class-PR ;
  skos:related lf:slope-class-ST ;
  skos:related lf:slope-class-VS ;
  skos:topConceptOf asls:landform ;
.
lf:landform-pattern-MOU-common-elements
  a skos:Collection ;
  dcterms:identifier "http://anzsoil.org/def/au/asls/landform/landform-pattern-MOU-common-elements"^^xsd:anyURI ;
  skos:member lf:landform-element-ALC ;
  skos:member lf:landform-element-LDS ;
  skos:member lf:landform-element-SCA ;
  skos:member lf:landform-element-TAL ;
  skos:member lf:landform-element-VLF ;
  skos:prefLabel "Common elements of Mountains"@en ;
  skos:related lf:landform-pattern-MOU ;
.
lf:landform-pattern-MOU-comparewith-patterns
  a skos:Collection ;
  dcterms:identifier "http://anzsoil.org/def/au/asls/landform/landform-pattern-MOU-comparewith-patterns"^^xsd:anyURI ;
  skos:member lf:landform-pattern-HIL ;
  skos:member lf:landform-pattern-LOW ;
  skos:member lf:landform-pattern-PLA ;
  skos:member lf:landform-pattern-RIS ;
  skos:prefLabel "Compare Mountains with these patterns"@en ;
  skos:related lf:landform-pattern-MOU ;
.
lf:landform-pattern-MOU-occasional-elements
  a skos:Collection ;
  dcterms:identifier "http://anzsoil.org/def/au/asls/landform/landform-pattern-MOU-occasional-elements"^^xsd:anyURI ;
  skos:member lf:landform-element-CIR ;
  skos:member lf:landform-element-FOO ;
  skos:prefLabel "Occasional elements of Mountains"@en ;
  skos:related lf:landform-pattern-MOU ;
.
lf:landform-pattern-MOU-typical-elements
  a skos:Collection ;
  dcterms:identifier "http://anzsoil.org/def/au/asls/landform/landform-pattern-MOU-typical-elements"^^xsd:anyURI ;
  skos:member lf:landform-element-HCR ;
  skos:member lf:landform-element-HSL ;
  skos:member lf:landform-element-STB ;
  skos:prefLabel "Typical elements of Mountains"@en ;
  skos:related lf:landform-pattern-MOU ;
.
lf:landform-pattern-PAR
  a skos:Concept ;
  skos-ext:isMemberOf lf:landform-pattern-glossary ;
  skos-ext:relatedCollection lf:landform-pattern-PAR-comparewith-patterns ;
  skos-ext:relatedCollection lf:landform-pattern-PAR-typical-elements ;
  dcterms:identifier "http://anzsoil.org/def/au/asls/landform/landform-pattern-PAR"^^xsd:anyURI ;
  skos:definition """dunefield characterised by sand dunes with a long, scoop-shaped form, convex in the downwind direction so that its trailing arms point upwind; the ground plan, when developed, approximates the form of a parabola. Where many parabolic dunes have been active, the trailing arms give the impression of a longitudinal dunefield. 
Typical elements: dune or dunecrest, duneslope, swale, blow-out.
Compare with longitudinal dunefield."""@en ;
  skos:inScheme asls:landform ;
  skos:notation "PAR" ;
  skos:prefLabel "Parabolic dunefield"@en ;
  skos:topConceptOf asls:landform ;
.
lf:landform-pattern-PAR-comparewith-patterns
  a skos:Collection ;
  dcterms:identifier "http://anzsoil.org/def/au/asls/landform/landform-pattern-PAR-comparewith-patterns"^^xsd:anyURI ;
  skos:member lf:landform-pattern-LON ;
  skos:prefLabel "Compare Parabolic dunefields with these patterns"@en ;
  skos:related lf:landform-pattern-PAR ;
.
lf:landform-pattern-PAR-typical-elements
  a skos:Collection ;
  dcterms:identifier "http://anzsoil.org/def/au/asls/landform/landform-pattern-PAR-typical-elements"^^xsd:anyURI ;
  skos:member lf:landform-element-BOU ;
  skos:member lf:landform-element-DUC ;
  skos:member lf:landform-element-DUN ;
  skos:member lf:landform-element-DUS ;
  skos:member lf:landform-element-SWL ;
  skos:prefLabel "Typical elements of Parabolic dunefields"@en ;
  skos:related lf:landform-pattern-PAR ;
.
lf:landform-pattern-PED
  a skos:Concept ;
  skos-ext:isMemberOf lf:landform-pattern-glossary ;
  skos-ext:relatedCollection lf:landform-pattern-PAR-comparewith-patterns ;
  skos-ext:relatedCollection lf:landform-pattern-PAR-typical-elements ;
  dcterms:identifier "http://anzsoil.org/def/au/asls/landform/landform-pattern-PED"^^xsd:anyURI ;
  skos:definition """gently inclined to level (less than 1%) landform pattern of extremely low relief, typically with numerous rapidly migrating, very shallow incipient stream channels, which form a centrifugal to diverging, integrated reticulated pattern. It is underlain by bedrock, eroded, and locally aggraded, by frequently active channelled stream flow or sheet flow, with subordinate wind erosion. Pediments characteristically lie downslope from adjacent hills with markedly steeper slopes. 
Typical elements: pediment, plain, stream bed(?).
Compare with sheet-flood fan and alluvial fan."""@en ;
  skos:inScheme asls:landform ;
  skos:notation "PED" ;
  skos:prefLabel "Pediment (pattern)"@en ;
  skos:related lf:relief-class-P ;
  skos:related lf:slope-class-GE ;
  skos:related lf:slope-class-LE ;
  skos:related lf:slope-class-VG ;
  skos:topConceptOf asls:landform ;
.
lf:landform-pattern-PED-comparewith-patterns
  a skos:Collection ;
  dcterms:identifier "http://anzsoil.org/def/au/asls/landform/landform-pattern-PED-comparewith-patterns"^^xsd:anyURI ;
  skos:member lf:landform-pattern-ALF ;
  skos:member lf:landform-pattern-SHF ;
  skos:prefLabel "Compare Pediment with these patterns"@en ;
  skos:related lf:landform-pattern-PED ;
.
lf:landform-pattern-PED-typical-elements
  a skos:Collection ;
  dcterms:identifier "http://anzsoil.org/def/au/asls/landform/landform-pattern-PED-typical-elements"^^xsd:anyURI ;
  skos:member lf:landform-element-PED ;
  skos:member lf:landform-element-PLA ;
  skos:member lf:landform-element-STB ;
  skos:prefLabel "Typical elements of Pediment"@en ;
  skos:related lf:landform-pattern-PED ;
.
lf:landform-pattern-PEP
  a skos:Concept ;
  skos-ext:isMemberOf lf:landform-pattern-glossary ;
  skos-ext:relatedCollection lf:landform-pattern-PEP-typical-elements ;
  dcterms:identifier "http://anzsoil.org/def/au/asls/landform/landform-pattern-PEP"^^xsd:anyURI ;
  skos:definition """level to very gently inclined landform pattern with extremely low relief and no stream channels, eroded by barely active sheet flow and wind. Largely relict from more effective erosion by stream flow in incipient stream channels as on a pediment. (Described by King 1953.) 
Typical element: plain."""@en ;
  skos:inScheme asls:landform ;
  skos:notation "PEP" ;
  skos:prefLabel "Pediplain"@en ;
  skos:related lf:relief-class-P ;
  skos:related lf:slope-class-LE ;
  skos:related lf:slope-class-VG ;
  skos:topConceptOf asls:landform ;
.
lf:landform-pattern-PEP-typical-elements
  a skos:Collection ;
  dcterms:identifier "http://anzsoil.org/def/au/asls/landform/landform-pattern-PEP-typical-elements"^^xsd:anyURI ;
  skos:member lf:landform-element-PLA ;
  skos:prefLabel "Typical elements of Pediplain"@en ;
  skos:related lf:landform-pattern-PEP ;
.
lf:landform-pattern-PLA
  a skos:Concept ;
  skos-ext:isMemberOf lf:landform-pattern-glossary ;
  skos-ext:relatedCollection lf:landform-pattern-PLA-comparewith-patterns ;
  dcterms:identifier "http://anzsoil.org/def/au/asls/landform/landform-pattern-PLA"^^xsd:anyURI ;
  skos:definition "level to undulating or, rarely, rolling landform pattern of extremely low relief (less than 9 m)."@en ;
  skos:inScheme asls:landform ;
  skos:notation "PLA" ;
  skos:prefLabel "Plain (pattern)"@en ;
  skos:related lf:relief-class-P ;
  skos:related lf:slope-class-GE ;
  skos:related lf:slope-class-LE ;
  skos:related lf:slope-class-MO ;
  skos:related lf:slope-class-VG ;
  skos:topConceptOf asls:landform ;
.
lf:landform-pattern-PLA-comparewith-patterns
  a skos:Collection ;
  dcterms:identifier "http://anzsoil.org/def/au/asls/landform/landform-pattern-PLA-comparewith-patterns"^^xsd:anyURI ;
  skos:member lf:landform-pattern-HIL ;
  skos:member lf:landform-pattern-LOW ;
  skos:member lf:landform-pattern-MOU ;
  skos:member lf:landform-pattern-RIS ;
  skos:prefLabel "Compare Plain with these patterns"@en ;
  skos:related lf:landform-pattern-PLA ;
.
lf:landform-pattern-PLT
  a skos:Concept ;
  skos-ext:isMemberOf lf:landform-pattern-glossary ;
  skos-ext:relatedCollection lf:landform-pattern-PLT-common-elements ;
  skos-ext:relatedCollection lf:landform-pattern-PLT-occasional-elements ;
  skos-ext:relatedCollection lf:landform-pattern-PLT-typical-elements ;
  dcterms:identifier "http://anzsoil.org/def/au/asls/landform/landform-pattern-PLT"^^xsd:anyURI ;
  skos:definition """level to rolling landform pattern of plains, rises or low hills standing above a cliff, scarp or escarpment that extends around a large part of its perimeter. A bounding scarp or cliff landform element may be included or excluded; a bounding escarpment would be an adjacent landform pattern. 
Typical elements: plain, summit surface, cliff.
Common elements: hillcrest, hillslope, drainage depression, rock flat, scarp.
Occasional element: stream channel."""@en ;
  skos:inScheme asls:landform ;
  skos:notation "PLT" ;
  skos:prefLabel "Plateau"@en ;
  skos:related lf:slope-class-GE ;
  skos:related lf:slope-class-LE ;
  skos:related lf:slope-class-MO ;
  skos:related lf:slope-class-VG ;
  skos:topConceptOf asls:landform ;
.
lf:landform-pattern-PLT-common-elements
  a skos:Collection ;
  dcterms:identifier "http://anzsoil.org/def/au/asls/landform/landform-pattern-PLT-common-elements"^^xsd:anyURI ;
  skos:member lf:landform-element-DDE ;
  skos:member lf:landform-element-HCR ;
  skos:member lf:landform-element-HSL ;
  skos:member lf:landform-element-RFL ;
  skos:member lf:landform-element-SCA ;
  skos:prefLabel "Common elements of Plateau"@en ;
  skos:related lf:landform-pattern-PLT ;
.
lf:landform-pattern-PLT-occasional-elements
  a skos:Collection ;
  dcterms:identifier "http://anzsoil.org/def/au/asls/landform/landform-pattern-PLT-occasional-elements"^^xsd:anyURI ;
  skos:member lf:landform-element-STC ;
  skos:prefLabel "Occasional elements of Plateau"@en ;
  skos:related lf:landform-pattern-PLT ;
.
lf:landform-pattern-PLT-typical-elements
  a skos:Collection ;
  dcterms:identifier "http://anzsoil.org/def/au/asls/landform/landform-pattern-PLT-typical-elements"^^xsd:anyURI ;
  skos:member lf:landform-element-CLI ;
  skos:member lf:landform-element-PLA ;
  skos:member lf:landform-element-SUS ;
  skos:prefLabel "Typical elements of Plateau"@en ;
  skos:related lf:landform-pattern-PLT ;
.
lf:landform-pattern-PLY
  a skos:Concept ;
  skos-ext:isMemberOf lf:landform-pattern-glossary ;
  skos-ext:relatedCollection lf:landform-pattern-PLY-comparewith-patterns ;
  skos-ext:relatedCollection lf:landform-pattern-PLY-typical-elements ;
  dcterms:identifier "http://anzsoil.org/def/au/asls/landform/landform-pattern-PLY"^^xsd:anyURI ;
  skos:definition """level landform pattern with extremely low relief, typically without stream channels, aggraded by rarely active sheet flow and modified by wind, waves, and soil phenomena. 
Typical elements: playa, lunette, plain.
Compare with lacustrine plain."""@en ;
  skos:inScheme asls:landform ;
  skos:notation "PLY" ;
  skos:prefLabel "Playa plain"@en ;
  skos:related lf:relief-class-P ;
  skos:related lf:slope-class-LE ;
  skos:topConceptOf asls:landform ;
.
lf:landform-pattern-PLY-comparewith-patterns
  a skos:Collection ;
  dcterms:identifier "http://anzsoil.org/def/au/asls/landform/landform-pattern-PLY-comparewith-patterns"^^xsd:anyURI ;
  skos:member lf:landform-pattern-LAC ;
  skos:prefLabel "Compare Playa plain with these patterns"@en ;
  skos:related lf:landform-pattern-PLY ;
.
lf:landform-pattern-PLY-typical-elements
  a skos:Collection ;
  dcterms:identifier "http://anzsoil.org/def/au/asls/landform/landform-pattern-PLY-typical-elements"^^xsd:anyURI ;
  skos:member lf:landform-element-LUN ;
  skos:member lf:landform-element-PLA ;
  skos:member lf:landform-element-PLY ;
  skos:prefLabel "Typical elements of Playa plain"@en ;
  skos:related lf:landform-pattern-PLY ;
.
lf:landform-pattern-PNP
  a skos:Concept ;
  skos-ext:isMemberOf lf:landform-pattern-glossary ;
  skos-ext:relatedCollection lf:landform-pattern-PNP-typical-elements ;
  dcterms:identifier "http://anzsoil.org/def/au/asls/landform/landform-pattern-PNP"^^xsd:anyURI ;
  skos:definition """level to gently undulating landform pattern with extremely low relief and sparse, slowly migrating alluvial stream channels which form a non-directional, integrated tributary pattern. It is eroded by barely active sheet flow, creep, and channelled and over-bank stream flow. (Described by Davis 1889.) 
Typical elements: plain (dominant), stream channel."""@en ;
  skos:inScheme asls:landform ;
  skos:notation "PNP" ;
  skos:prefLabel "Peneplain"@en ;
  skos:related lf:relief-class-P ;
  skos:related lf:slope-class-LE ;
  skos:related lf:slope-class-VG ;
  skos:topConceptOf asls:landform ;
.
lf:landform-pattern-PNP-typical-elements
  a skos:Collection ;
  dcterms:identifier "http://anzsoil.org/def/au/asls/landform/landform-pattern-PNP-typical-elements"^^xsd:anyURI ;
  skos:member lf:landform-element-PLA ;
  skos:member lf:landform-element-STC ;
  skos:prefLabel "Typical elements of Peneplain"@en ;
  skos:related lf:landform-pattern-PNP ;
.
lf:landform-pattern-RIS
  a skos:Concept ;
  skos-ext:isMemberOf lf:landform-pattern-glossary ;
  skos-ext:relatedCollection lf:landform-pattern-RIS-common-elements ;
  skos-ext:relatedCollection lf:landform-pattern-RIS-comparewith-patterns ;
  skos-ext:relatedCollection lf:landform-pattern-RIS-occasional-elements ;
  skos-ext:relatedCollection lf:landform-pattern-RIS-typical-elements ;
  dcterms:identifier "http://anzsoil.org/def/au/asls/landform/landform-pattern-RIS"^^xsd:anyURI ;
  skos:definition """landform pattern of very low relief (9–30 m) and very gentle to steep slopes. The fixed, erosional stream channels are closely to very widely spaced and form a non-directional to convergent, integrated or interrupted tributary pattern. The pattern is eroded by continuously active to barely active creep and sheet flow. 
Typical elements: hillcrest, hillslope (dominant), footslope, drainage depression, riseslope.
Common elements: valley flat, stream channel.
Occasional elements: gully, fan, tor.
Compare with mountains, hills, low hills and plain."""@en ;
  skos:inScheme asls:landform ;
  skos:notation "RIS" ;
  skos:prefLabel "Rises"@en ;
  skos:related lf:relief-class-R ;
  skos:related lf:slope-class-GE ;
  skos:related lf:slope-class-MO ;
  skos:related lf:slope-class-ST ;
  skos:related lf:slope-class-VG ;
  skos:topConceptOf asls:landform ;
.
lf:landform-pattern-RIS-common-elements
  a skos:Collection ;
  dcterms:identifier "http://anzsoil.org/def/au/asls/landform/landform-pattern-RIS-common-elements"^^xsd:anyURI ;
  skos:member lf:landform-element-STC ;
  skos:member lf:landform-element-VLF ;
  skos:prefLabel "Common elements of Rises"@en ;
  skos:related lf:landform-pattern-RIS ;
.
lf:landform-pattern-RIS-comparewith-patterns
  a skos:Collection ;
  dcterms:identifier "http://anzsoil.org/def/au/asls/landform/landform-pattern-RIS-comparewith-patterns"^^xsd:anyURI ;
  skos:member lf:landform-pattern-HIL ;
  skos:member lf:landform-pattern-LOW ;
  skos:member lf:landform-pattern-PLA ;
  skos:prefLabel "Compare Rises with these patterns"@en ;
  skos:related lf:landform-pattern-RIS ;
.
lf:landform-pattern-RIS-occasional-elements
  a skos:Collection ;
  dcterms:identifier "http://anzsoil.org/def/au/asls/landform/landform-pattern-RIS-occasional-elements"^^xsd:anyURI ;
  skos:member lf:landform-element-FAN ;
  skos:member lf:landform-element-GUL ;
  skos:member lf:landform-element-TOR ;
  skos:prefLabel "Occasional elements of Rises"@en ;
  skos:related lf:landform-pattern-RIS ;
.
lf:landform-pattern-RIS-typical-elements
  a skos:Collection ;
  dcterms:identifier "http://anzsoil.org/def/au/asls/landform/landform-pattern-RIS-typical-elements"^^xsd:anyURI ;
  skos:member lf:landform-element-DDE ;
  skos:member lf:landform-element-FOO ;
  skos:member lf:landform-element-HCR ;
  skos:member lf:landform-element-HSL ;
  skos:member lf:landform-element-RES ;
  skos:prefLabel "Typical elements of Rises"@en ;
  skos:related lf:landform-pattern-RIS ;
.
lf:landform-pattern-SAN
  a skos:Concept ;
  skos-ext:isMemberOf lf:landform-pattern-glossary ;
  skos-ext:relatedCollection lf:landform-pattern-SAN-occasional-elements ;
  skos-ext:relatedCollection lf:landform-pattern-SAN-typical-elements ;
  dcterms:identifier "http://anzsoil.org/def/au/asls/landform/landform-pattern-SAN"^^xsd:anyURI ;
  skos:definition """level to gently undulating landform pattern of extremely low relief and without channels; formed possibly by sheet flow or stream flow, but now relict and modified by wind action. 
Typical element: plain.
Occasional elements: dune, playa, lunette."""@en ;
  skos:inScheme asls:landform ;
  skos:notation "SAN" ;
  skos:prefLabel "Sand plain"@en ;
  skos:related lf:relief-class-P ;
  skos:related lf:slope-class-LE ;
  skos:related lf:slope-class-VG ;
  skos:topConceptOf asls:landform ;
.
lf:landform-pattern-SAN-occasional-elements
  a skos:Collection ;
  dcterms:identifier "http://anzsoil.org/def/au/asls/landform/landform-pattern-SAN-occasional-elements"^^xsd:anyURI ;
  skos:member lf:landform-element-DUN ;
  skos:member lf:landform-element-LUN ;
  skos:member lf:landform-element-PLY ;
  skos:prefLabel "Occasional elements of Sand plain"@en ;
  skos:related lf:landform-pattern-SAN ;
.
lf:landform-pattern-SAN-typical-elements
  a skos:Collection ;
  dcterms:identifier "http://anzsoil.org/def/au/asls/landform/landform-pattern-SAN-typical-elements"^^xsd:anyURI ;
  skos:member lf:landform-element-PLA ;
  skos:prefLabel "Typical elements of Sand plain"@en ;
  skos:related lf:landform-pattern-SAN ;
.
lf:landform-pattern-SHF
  a skos:Concept ;
  skos-ext:isMemberOf lf:landform-pattern-glossary ;
  skos-ext:relatedCollection lf:landform-pattern-SHF-comparewith-patterns ;
  skos-ext:relatedCollection lf:landform-pattern-SHF-typical-elements ;
  dcterms:identifier "http://anzsoil.org/def/au/asls/landform/landform-pattern-SHF"^^xsd:anyURI ;
  skos:definition """level (less than 1% slope) to very gently inclined landform pattern of extremely low relief with numerous rapidly migrating, very shallow incipient stream channels forming a divergent to unidirectional, integrated or interrupted reticulated pattern. The pattern is aggraded by frequently active sheet flow and channelled stream flow, with subordinate wind erosion. 
Typical elements: plain, stream bed.
Compare with alluvial fan and pediment."""@en ;
  skos:inScheme asls:landform ;
  skos:notation "SHF" ;
  skos:prefLabel "Sheet-flood fan"@en ;
  skos:related lf:relief-class-P ;
  skos:related lf:slope-class-LE ;
  skos:related lf:slope-class-VG ;
  skos:topConceptOf asls:landform ;
.
lf:landform-pattern-SHF-comparewith-patterns
  a skos:Collection ;
  dcterms:identifier "http://anzsoil.org/def/au/asls/landform/landform-pattern-SHF-comparewith-patterns"^^xsd:anyURI ;
  skos:member lf:landform-pattern-ALF ;
  skos:member lf:landform-pattern-PED ;
  skos:prefLabel "Compare Sheet-flood fan with these patterns"@en ;
  skos:related lf:landform-pattern-SHF ;
.
lf:landform-pattern-SHF-typical-elements
  a skos:Collection ;
  dcterms:identifier "http://anzsoil.org/def/au/asls/landform/landform-pattern-SHF-typical-elements"^^xsd:anyURI ;
  skos:member lf:landform-element-PLA ;
  skos:member lf:landform-element-STB ;
  skos:prefLabel "Typical elements of Sheet-flood fan"@en ;
  skos:related lf:landform-pattern-SHF ;
.
lf:landform-pattern-STA
  a skos:Concept ;
  skos-ext:isMemberOf lf:landform-pattern-glossary ;
  skos-ext:relatedCollection lf:landform-pattern-STA-common-elements ;
  skos-ext:relatedCollection lf:landform-pattern-STA-comparewith-patterns ;
  skos-ext:relatedCollection lf:landform-pattern-STA-occasional-elements ;
  skos-ext:relatedCollection lf:landform-pattern-STA-typical-elements ;
  dcterms:identifier "http://anzsoil.org/def/au/asls/landform/landform-pattern-STA"^^xsd:anyURI ;
  skos:definition """alluvial plain on which erosion and aggradation by channelled and over-bank stream flow is barely active or inactive because of reduced water supply, without apparent incision or channel enlargement that would lower the level of stream action. 
Typical elements: stream channel (stream bed and bank), plain (dominant).
Common elements: bar, scroll, levee, backplain, swamp.
Occasional elements: ox-bow, flood-out, lake.
Compare with flood plain and terrace."""@en ;
  skos:inScheme asls:landform ;
  skos:notation "STA" ;
  skos:prefLabel "Stagnant alluvial plain"@en ;
  skos:topConceptOf asls:landform ;
.
lf:landform-pattern-STA-common-elements
  a skos:Collection ;
  dcterms:identifier "http://anzsoil.org/def/au/asls/landform/landform-pattern-STA-common-elements"^^xsd:anyURI ;
  skos:member lf:landform-element-BAR ;
  skos:member lf:landform-element-BKP ;
  skos:member lf:landform-element-LEV ;
  skos:member lf:landform-element-SCR ;
  skos:member lf:landform-element-SWP ;
  skos:prefLabel "Common elements of Stagnant alluvial plain"@en ;
  skos:related lf:landform-pattern-STA ;
.
lf:landform-pattern-STA-comparewith-patterns
  a skos:Collection ;
  dcterms:identifier "http://anzsoil.org/def/au/asls/landform/landform-pattern-STA-comparewith-patterns"^^xsd:anyURI ;
  skos:member lf:landform-pattern-FLO ;
  skos:member lf:landform-pattern-TER ;
  skos:prefLabel "Compare Stagnant alluvial plain with these patterns"@en ;
  skos:related lf:landform-pattern-STA ;
.
lf:landform-pattern-STA-occasional-elements
  a skos:Collection ;
  dcterms:identifier "http://anzsoil.org/def/au/asls/landform/landform-pattern-STA-occasional-elements"^^xsd:anyURI ;
  skos:member lf:landform-element-FLD ;
  skos:member lf:landform-element-LAK ;
  skos:member lf:landform-element-OXB ;
  skos:prefLabel "Occasional elements of Stagnant alluvial plain"@en ;
  skos:related lf:landform-pattern-STA ;
.
lf:landform-pattern-STA-typical-elements
  a skos:Collection ;
  dcterms:identifier "http://anzsoil.org/def/au/asls/landform/landform-pattern-STA-typical-elements"^^xsd:anyURI ;
  skos:member lf:landform-element-BAN ;
  skos:member lf:landform-element-PLA ;
  skos:member lf:landform-element-STB ;
  skos:member lf:landform-element-STC ;
  skos:prefLabel "Typical elements of Stagnant alluvial plain"@en ;
  skos:related lf:landform-pattern-STA ;
.
lf:landform-pattern-TEL
  a skos:Concept ;
  skos-ext:isMemberOf lf:landform-pattern-glossary ;
  skos-ext:relatedCollection lf:landform-pattern-TEL-occasional-elements ;
  skos-ext:relatedCollection lf:landform-pattern-TEL-typical-elements ;
  dcterms:identifier "http://anzsoil.org/def/au/asls/landform/landform-pattern-TEL"^^xsd:anyURI ;
  skos:definition """landform pattern including one or more terraces and often a flood plain. Relief is low or very low (9–90 m). Terrace plains or terrace flats occur at stated heights above the top of the stream bank. 
Typical elements: terrace plains, terrace flats, scarps, scroll plain, stream channel.
Occasional elements: stream channel, scroll, levee."""@en ;
  skos:inScheme asls:landform ;
  skos:notation "TEL" ;
  skos:prefLabel "Terraced land (alluvial)"@en ;
  skos:topConceptOf asls:landform ;
.
lf:landform-pattern-TEL-occasional-elements
  a skos:Collection ;
  dcterms:identifier "http://anzsoil.org/def/au/asls/landform/landform-pattern-TEL-occasional-elements"^^xsd:anyURI ;
  skos:member lf:landform-element-LEV ;
  skos:member lf:landform-element-SCR ;
  skos:prefLabel "Occasional elements of Terraced land"@en ;
  skos:related lf:landform-pattern-TEL ;
.
lf:landform-pattern-TEL-typical-elements
  a skos:Collection ;
  dcterms:identifier "http://anzsoil.org/def/au/asls/landform/landform-pattern-TEL-typical-elements"^^xsd:anyURI ;
  skos:member lf:landform-element-SCA ;
  skos:member lf:landform-element-SRP ;
  skos:member lf:landform-element-STC ;
  skos:member lf:landform-element-TEF ;
  skos:member lf:landform-element-TEP ;
  skos:prefLabel "Typical elements of Terraced land"@en ;
  skos:related lf:landform-pattern-TEL ;
.
lf:landform-pattern-TER
  a skos:Concept ;
  skos-ext:isMemberOf lf:landform-pattern-glossary ;
  skos-ext:relatedCollection lf:landform-pattern-TER-occasional-elements ;
  skos-ext:relatedCollection lf:landform-pattern-TER-typical-elements ;
  dcterms:identifier "http://anzsoil.org/def/au/asls/landform/landform-pattern-TER"^^xsd:anyURI ;
  skos:definition """former flood plain on which erosion and aggradation by channelled and over-bank stream flow is barely active or inactive because deepening or enlargement of the stream channel has lowered the level of flooding. A pattern that has both a former flood plain and a significant, active flood plain, or that has former flood plains at more than one level, becomes terraced land. 
Typical elements: terrace plain (dominant), scarp, channel bench.
Occasional elements: stream channel, scroll, levee."""@en ;
  skos:inScheme asls:landform ;
  skos:notation "TER" ;
  skos:prefLabel "Terrace (alluvial)"@en ;
  skos:topConceptOf asls:landform ;
.
lf:landform-pattern-TER-occasional-elements
  a skos:Collection ;
  dcterms:identifier "http://anzsoil.org/def/au/asls/landform/landform-pattern-TER-occasional-elements"^^xsd:anyURI ;
  skos:member lf:landform-element-LEV ;
  skos:member lf:landform-element-SCR ;
  skos:member lf:landform-element-STC ;
  skos:prefLabel "Occasional elements of Terrace"@en ;
  skos:related lf:landform-pattern-TER ;
.
lf:landform-pattern-TER-typical-elements
  a skos:Collection ;
  dcterms:identifier "http://anzsoil.org/def/au/asls/landform/landform-pattern-TER-typical-elements"^^xsd:anyURI ;
  skos:member lf:landform-element-CBE ;
  skos:member lf:landform-element-SCA ;
  skos:member lf:landform-element-TEP ;
  skos:prefLabel "Typical elements of Terrace"@en ;
  skos:related lf:landform-pattern-TER ;
.
lf:landform-pattern-TID
  a skos:Concept ;
  skos-ext:isMemberOf lf:landform-pattern-glossary ;
  skos-ext:relatedCollection lf:landform-pattern-TID-occasional-elements ;
  skos-ext:relatedCollection lf:landform-pattern-TID-typical-elements ;
  dcterms:identifier "http://anzsoil.org/def/au/asls/landform/landform-pattern-TID"^^xsd:anyURI ;
  skos:definition """level landform pattern with extremely low relief and slowly migrating, deep alluvial stream channels, which form non-directional, integrated tributary patterns; it is aggraded by frequently active tides. 
Typical elements: plain (dominant), intertidal flat, supratidal flat, stream channel.
Occasional elements: lagoon, dune, beach ridge, beach."""@en ;
  skos:inScheme asls:landform ;
  skos:notation "TID" ;
  skos:prefLabel "Tidal flat (pattern)"@en ;
  skos:related lf:relief-class-P ;
  skos:topConceptOf asls:landform ;
.
lf:landform-pattern-TID-occasional-elements
  a skos:Collection ;
  dcterms:identifier "http://anzsoil.org/def/au/asls/landform/landform-pattern-TID-occasional-elements"^^xsd:anyURI ;
  skos:member lf:landform-element-BEA ;
  skos:member lf:landform-element-BRI ;
  skos:member lf:landform-element-DUN ;
  skos:member lf:landform-element-LAG ;
  skos:prefLabel "Occasional elements of Tidal flat"@en ;
  skos:related lf:landform-pattern-TID ;
.
lf:landform-pattern-TID-typical-elements
  a skos:Collection ;
  dcterms:identifier "http://anzsoil.org/def/au/asls/landform/landform-pattern-TID-typical-elements"^^xsd:anyURI ;
  skos:member lf:landform-element-ITF ;
  skos:member lf:landform-element-PLA ;
  skos:member lf:landform-element-STC ;
  skos:member lf:landform-element-STF ;
  skos:prefLabel "Typical elements of Tidal flat"@en ;
  skos:related lf:landform-pattern-TID ;
.
lf:landform-pattern-VOL
  a skos:Concept ;
  skos-ext:isMemberOf lf:landform-pattern-glossary ;
  skos-ext:relatedCollection lf:landform-pattern-VOL-common-elements ;
  skos-ext:relatedCollection lf:landform-pattern-VOL-typical-elements ;
  dcterms:identifier "http://anzsoil.org/def/au/asls/landform/landform-pattern-VOL"^^xsd:anyURI ;
  skos:definition """typically very high and very steep landform pattern without stream channels, or with erosional stream channels forming a centrifugal, interrupted tributary pattern. The landform is built up by volcanism, and is modified by erosional agents. 
Typical elements: cone, crater.
Common elements: scarp, hillcrest, hillslope, stream bed, lake, maar.
Occasional element: tumulus."""@en ;
  skos:inScheme asls:landform ;
  skos:notation "VOL" ;
  skos:prefLabel "Volcano"@en ;
  skos:related lf:relief-class-M ;
  skos:related lf:slope-class-VS ;
  skos:topConceptOf asls:landform ;
.
lf:landform-pattern-VOL-common-elements
  a skos:Collection ;
  dcterms:identifier "http://anzsoil.org/def/au/asls/landform/landform-pattern-VOL-common-elements"^^xsd:anyURI ;
  skos:member lf:landform-element-HCR ;
  skos:member lf:landform-element-HSL ;
  skos:member lf:landform-element-LAK ;
  skos:member lf:landform-element-MAA ;
  skos:member lf:landform-element-SCA ;
  skos:member lf:landform-element-STB ;
  skos:prefLabel "Occasional elements of Volcano"@en ;
  skos:related lf:landform-pattern-VOL ;
.
lf:landform-pattern-VOL-occasional-elements
  a skos:Collection ;
  dcterms:identifier "http://anzsoil.org/def/au/asls/landform/landform-pattern-VOL-occasional-elements"^^xsd:anyURI ;
  skos:member lf:landform-element-TUM ;
  skos:prefLabel "Typical elements of Volcano"@en ;
  skos:related lf:landform-pattern-VOL ;
.
lf:landform-pattern-VOL-typical-elements
  a skos:Collection ;
  dcterms:identifier "http://anzsoil.org/def/au/asls/landform/landform-pattern-VOL-typical-elements"^^xsd:anyURI ;
  skos:member lf:landform-element-CON ;
  skos:member lf:landform-element-CRA ;
  skos:prefLabel "Typical elements of Volcano"@en ;
  skos:related lf:landform-pattern-VOL ;
.
lf:landform-pattern-components
  a skos:Collection ;
  skos-ext:topMemberOf asls:landform ;
  dcterms:identifier "http://anzsoil.org/def/au/asls/landform/landform-pattern-components"^^xsd:anyURI ;
  skos:definition "Certain kinds of landform element are typical of a given landform pattern. Some are found commonly and others occasionally in a given type. These landform elements are listed for each type of landform pattern."@en ;
  skos:member lf:landform-pattern-ALF-common-elements ;
  skos:member lf:landform-pattern-ALF-comparewith-patterns ;
  skos:member lf:landform-pattern-ALF-typical-elements ;
  skos:member lf:landform-pattern-ALP-common-elements ;
  skos:member lf:landform-pattern-ALP-included-patterns ;
  skos:member lf:landform-pattern-ALP-occasional-elements ;
  skos:member lf:landform-pattern-ALP-typical-elements ;
  skos:member lf:landform-pattern-ANA-common-elements ;
  skos:member lf:landform-pattern-ANA-comparewith-patterns ;
  skos:member lf:landform-pattern-ANA-typical-elements ;
  skos:member lf:landform-pattern-BAD-comparewith-patterns ;
  skos:member lf:landform-pattern-BAD-occasional-elements ;
  skos:member lf:landform-pattern-BAD-typical-elements ;
  skos:member lf:landform-pattern-BAR-comparewith-patterns ;
  skos:member lf:landform-pattern-BAR-typical-elements ;
  skos:member lf:landform-pattern-BEA-common-elements ;
  skos:member lf:landform-pattern-BEA-comparewith-patterns ;
  skos:member lf:landform-pattern-BEA-typical-elements ;
  skos:member lf:landform-pattern-CAL-occasional-elements ;
  skos:member lf:landform-pattern-CAL-typical-elements ;
  skos:member lf:landform-pattern-CHE-common-elements ;
  skos:member lf:landform-pattern-CHE-comparewith-patterns ;
  skos:member lf:landform-pattern-CHE-typical-elements ;
  skos:member lf:landform-pattern-COR-common-elements ;
  skos:member lf:landform-pattern-COR-typical-elements ;
  skos:member lf:landform-pattern-COV-common-elements ;
  skos:member lf:landform-pattern-COV-comparewith-patterns ;
  skos:member lf:landform-pattern-COV-typical-elements ;
  skos:member lf:landform-pattern-DEL-common-elements ;
  skos:member lf:landform-pattern-DEL-comparewith-patterns ;
  skos:member lf:landform-pattern-DEL-typical-elements ;
  skos:member lf:landform-pattern-DUN-common-elements ;
  skos:member lf:landform-pattern-DUN-included-patterns ;
  skos:member lf:landform-pattern-DUN-typical-elements ;
  skos:member lf:landform-pattern-ESC-common-elements ;
  skos:member lf:landform-pattern-ESC-occasional-elements ;
  skos:member lf:landform-pattern-ESC-typical-elements ;
  skos:member lf:landform-pattern-FLO-common-elements ;
  skos:member lf:landform-pattern-FLO-included-patterns ;
  skos:member lf:landform-pattern-FLO-occasional-elements ;
  skos:member lf:landform-pattern-FLO-related-patterns ;
  skos:member lf:landform-pattern-FLO-typical-elements ;
  skos:member lf:landform-pattern-HIL-common-elements ;
  skos:member lf:landform-pattern-HIL-comparewith-patterns ;
  skos:member lf:landform-pattern-HIL-occasional-elements ;
  skos:member lf:landform-pattern-HIL-typical-elements ;
  skos:member lf:landform-pattern-KAR-common-elements ;
  skos:member lf:landform-pattern-KAR-occasional-elements ;
  skos:member lf:landform-pattern-KAR-typical-elements ;
  skos:member lf:landform-pattern-LAC-common-elements ;
  skos:member lf:landform-pattern-LAC-comparewith-patterns ;
  skos:member lf:landform-pattern-LAC-occasional-elements ;
  skos:member lf:landform-pattern-LAC-typical-elements ;
  skos:member lf:landform-pattern-LAV-common-elements ;
  skos:member lf:landform-pattern-LAV-typical-elements ;
  skos:member lf:landform-pattern-LON-comparewith-patterns ;
  skos:member lf:landform-pattern-LON-typical-elements ;
  skos:member lf:landform-pattern-LOW-common-elements ;
  skos:member lf:landform-pattern-LOW-comparewith-patterns ;
  skos:member lf:landform-pattern-LOW-occasional-elements ;
  skos:member lf:landform-pattern-LOW-typical-elements ;
  skos:member lf:landform-pattern-MAD-common-elements ;
  skos:member lf:landform-pattern-MAD-typical-elements ;
  skos:member lf:landform-pattern-MAR-occasional-elements ;
  skos:member lf:landform-pattern-MAR-typical-elements ;
  skos:member lf:landform-pattern-MEA-common-elements ;
  skos:member lf:landform-pattern-MEA-comparewith-patterns ;
  skos:member lf:landform-pattern-MEA-typical-elements ;
  skos:member lf:landform-pattern-MET-typical-elements ;
  skos:member lf:landform-pattern-MOU-common-elements ;
  skos:member lf:landform-pattern-MOU-comparewith-patterns ;
  skos:member lf:landform-pattern-MOU-occasional-elements ;
  skos:member lf:landform-pattern-MOU-typical-elements ;
  skos:member lf:landform-pattern-PAR-comparewith-patterns ;
  skos:member lf:landform-pattern-PAR-typical-elements ;
  skos:member lf:landform-pattern-PED-comparewith-patterns ;
  skos:member lf:landform-pattern-PED-typical-elements ;
  skos:member lf:landform-pattern-PEP-typical-elements ;
  skos:member lf:landform-pattern-PLA-comparewith-patterns ;
  skos:member lf:landform-pattern-PLT-common-elements ;
  skos:member lf:landform-pattern-PLT-occasional-elements ;
  skos:member lf:landform-pattern-PLT-typical-elements ;
  skos:member lf:landform-pattern-PLY-comparewith-patterns ;
  skos:member lf:landform-pattern-PLY-typical-elements ;
  skos:member lf:landform-pattern-PNP-typical-elements ;
  skos:member lf:landform-pattern-RIS-common-elements ;
  skos:member lf:landform-pattern-RIS-comparewith-patterns ;
  skos:member lf:landform-pattern-RIS-occasional-elements ;
  skos:member lf:landform-pattern-RIS-typical-elements ;
  skos:member lf:landform-pattern-SAN-occasional-elements ;
  skos:member lf:landform-pattern-SAN-typical-elements ;
  skos:member lf:landform-pattern-SHF-comparewith-patterns ;
  skos:member lf:landform-pattern-SHF-typical-elements ;
  skos:member lf:landform-pattern-STA-common-elements ;
  skos:member lf:landform-pattern-STA-comparewith-patterns ;
  skos:member lf:landform-pattern-STA-occasional-elements ;
  skos:member lf:landform-pattern-STA-typical-elements ;
  skos:member lf:landform-pattern-TEL-occasional-elements ;
  skos:member lf:landform-pattern-TEL-typical-elements ;
  skos:member lf:landform-pattern-TER-occasional-elements ;
  skos:member lf:landform-pattern-TER-typical-elements ;
  skos:member lf:landform-pattern-TID-occasional-elements ;
  skos:member lf:landform-pattern-TID-typical-elements ;
  skos:member lf:landform-pattern-VOL-common-elements ;
  skos:member lf:landform-pattern-VOL-occasional-elements ;
  skos:member lf:landform-pattern-VOL-typical-elements ;
  skos:prefLabel "Collections of elements found in specific landform patterns"@en ;
.
lf:landform-pattern-descriptions
  a skos:Collection ;
  skos-ext:topMemberOf asls:landform ;
  dcterms:identifier "http://anzsoil.org/def/au/asls/landform/landform-pattern-descriptions"^^xsd:anyURI ;
  skos:definition """<p>The significant kinds of landform pattern in Australia may be described and differentiated by the following attributes assessed within a circle of about 300 m radius:</p>
<ul>
<li>relief</li>
<li>modal slope</li>
<li>stream channel occurrence</li>
<li>mode of geomorphological activity</li>
<li>geomorphological agent</li>
<li>status of geomorphological activity</li>
<li>component landform elements</li>
</ul>
<p>The landform pattern glossary is based explicitly on these attributes.</p>"""^^rdf:HTML ;
  skos:member lf:geomorphological-agents ;
  skos:member lf:modal-slope ;
  skos:member lf:mode-of-geomorphological-activity ;
  skos:member lf:relief ;
  skos:member lf:simple-erosional-landform-patterns ;
  skos:member lf:stream-channel-occurence ;
  skos:prefLabel "Description of landform pattern"@en ;
.
lf:landform-pattern-glossary
  a skos:Collection ;
  skos-ext:topMemberOf asls:landform ;
  dcterms:identifier "http://anzsoil.org/def/au/asls/landform/landform-pattern-glossary"^^xsd:anyURI ;
  skos:definition "The definitions in this glossary refer explicitly to the attributes of landform patterns that have been set down in the preceding sections."@en ;
  skos:member lf:landform-pattern-ALF ;
  skos:member lf:landform-pattern-ALP ;
  skos:member lf:landform-pattern-ANA ;
  skos:member lf:landform-pattern-BAD ;
  skos:member lf:landform-pattern-BAR ;
  skos:member lf:landform-pattern-BEA ;
  skos:member lf:landform-pattern-CAL ;
  skos:member lf:landform-pattern-CHE ;
  skos:member lf:landform-pattern-COR ;
  skos:member lf:landform-pattern-COV ;
  skos:member lf:landform-pattern-DEL ;
  skos:member lf:landform-pattern-DUN ;
  skos:member lf:landform-pattern-ESC ;
  skos:member lf:landform-pattern-FLO ;
  skos:member lf:landform-pattern-HIL ;
  skos:member lf:landform-pattern-KAR ;
  skos:member lf:landform-pattern-LAC ;
  skos:member lf:landform-pattern-LAV ;
  skos:member lf:landform-pattern-LON ;
  skos:member lf:landform-pattern-LOW ;
  skos:member lf:landform-pattern-MAD ;
  skos:member lf:landform-pattern-MAR ;
  skos:member lf:landform-pattern-MEA ;
  skos:member lf:landform-pattern-MET ;
  skos:member lf:landform-pattern-MOU ;
  skos:member lf:landform-pattern-PAR ;
  skos:member lf:landform-pattern-PED ;
  skos:member lf:landform-pattern-PEP ;
  skos:member lf:landform-pattern-PLA ;
  skos:member lf:landform-pattern-PLT ;
  skos:member lf:landform-pattern-PLY ;
  skos:member lf:landform-pattern-PNP ;
  skos:member lf:landform-pattern-RIS ;
  skos:member lf:landform-pattern-SAN ;
  skos:member lf:landform-pattern-SHF ;
  skos:member lf:landform-pattern-STA ;
  skos:member lf:landform-pattern-TEL ;
  skos:member lf:landform-pattern-TER ;
  skos:member lf:landform-pattern-TID ;
  skos:member lf:landform-pattern-VOL ;
  skos:prefLabel "Glossary of landform patterns"@en ;
.
lf:location-within-the-landform-element
  a skos:Collection ;
  a sosa:ObservableProperty ;
  dcterms:identifier "http://anzsoil.org/def/au/asls/landform/location-within-the-landform-element"^^xsd:anyURI ;
  skos:definition "A site chosen to represent a landform element will often be placed centrally within it. For various reasons, a site may not be centrally placed and this should be recorded. The vertical position of the site within the height of the landform element may be the best measure:"@en ;
  skos:member lf:location-within-the-landform-element-B ;
  skos:member lf:location-within-the-landform-element-M ;
  skos:member lf:location-within-the-landform-element-T ;
  skos:prefLabel "Location within the landform element"@en ;
.
lf:location-within-the-landform-element-B
  a skos:Concept ;
  skos-ext:isMemberOf lf:location-within-the-landform-element ;
  dcterms:identifier "http://anzsoil.org/def/au/asls/landform/location-within-the-landform-element-B"^^xsd:anyURI ;
  skos:definition "Bottom third of the height of the landform element.."@en ;
  skos:inScheme asls:landform ;
  skos:notation "B" ;
  skos:prefLabel "Bottom"@en ;
  skos:topConceptOf asls:landform ;
.
lf:location-within-the-landform-element-M
  a skos:Concept ;
  skos-ext:isMemberOf lf:location-within-the-landform-element ;
  dcterms:identifier "http://anzsoil.org/def/au/asls/landform/location-within-the-landform-element-M"^^xsd:anyURI ;
  skos:definition "Middle third of the height of the landform element.."@en ;
  skos:inScheme asls:landform ;
  skos:notation "M" ;
  skos:prefLabel "Middle"@en ;
  skos:topConceptOf asls:landform ;
.
lf:location-within-the-landform-element-T
  a skos:Concept ;
  skos-ext:isMemberOf lf:location-within-the-landform-element ;
  dcterms:identifier "http://anzsoil.org/def/au/asls/landform/location-within-the-landform-element-T"^^xsd:anyURI ;
  skos:definition "Top third of the height of the landform element.."@en ;
  skos:inScheme asls:landform ;
  skos:notation "T" ;
  skos:prefLabel "Top"@en ;
  skos:topConceptOf asls:landform ;
.
lf:location-within-toposequence
  a skos:Concept ;
  a sosa:ObservableProperty ;
  dcterms:identifier "http://anzsoil.org/def/au/asls/landform/location-within-toposequence"^^xsd:anyURI ;
  skos:definition """For detailed work, the location of the site within the toposequence down a slope line may relate to landform processes. Unfortunately, slope lines, by definition, extend from a summit to the lowest point (Cayley 1859), which may be many kilometres apart. One must arbitrarily determine the effective top and bottom of the toposequence. These effective end points come where the slope line coalesces with other slope lines to form a ridge line or a course line* (Figure 2a). In practice, ridge lines and course lines are to be excluded from the toposequence (see earlier section on landform element height). One arbitrary rule that will exclude the ridge line is to put the top of the toposequence where the contour curvature exceeds 60º in 40 m. The course line may be excluded by the same rule, or by putting the bottom of the toposequence at a stream channel.
Any site can be located by its vertical and horizontal distances from the defined top and bottom of the toposequence. Drainage height (page 88) is one of these measures.
The toposequence concept leads to definition of the attributes specific catchment area and specific dispersal area (Speight 1974, 1980) that predict hillslope hydrology and erosion (see, for example, Moore et al. 1988)."""@en ;
  skos:inScheme asls:landform ;
  skos:prefLabel "Location within toposequence"@en ;
  skos:topConceptOf asls:landform ;
.
lf:modal-slope
  a skos:Collection ;
  a sosa:ObservableProperty ;
  dcterms:identifier "http://anzsoil.org/def/au/asls/landform/modal-slope"^^xsd:anyURI ;
  skos:definition """Modal slope is defined as the most common class of slope occurring in a landform pattern. Where slope classes have been obtained by systematic sampling, define the classes using equal increments on a scale of the logarithm of the slope tangent, a procedure intended to normalise frequency distributions of observed slope (Speight 1971). Where the most common slope class is estimated by direct observation, it is thought that the estimate will compare with that calculated using the log-normal model.
Modal slope class determines the use of certain adjectives applied to landform patterns that are characterised by alternating crests and depressions. These are: rolling for moderate modal slopes (10–32%); undulating for gentle slopes (3–10%); and gently undulating for very gentle slopes (1–3%) (compare with Soil Survey Staff 1951, pages 161–165). The other slope classes, precipitous, very steep, steep and level, are to be applied as they stand. The terminology for simple erosional landform patterns based on relief and modal slope is given in Table 5.
Table 5 defines the category badlands by various combinations of high slope values and low relief values. These combinations imply extremely close spacing of streams or valleys. Specifically, if one assumes a sawtooth terrain profile, the valley spacing implied is less than 100 m in areas with 50 m relief and less than 30 m in areas with 5 m relief; these values appear to accord with usage.
Table 7 lists types of landform pattern in order of their typical class of modal slope. This table should not be regarded as definitive, for slope within each type of landform pattern may vary widely."""@en ;
  skos:member lf:relief-class-H ;
  skos:member lf:relief-class-L ;
  skos:member lf:relief-class-M ;
  skos:member lf:relief-class-P ;
  skos:member lf:relief-class-R ;
  skos:prefLabel "Modal slope"@en ;
.
lf:mode-of-geomorphological-activity
  a skos:Collection ;
  a sosa:ObservableProperty ;
  dcterms:identifier "http://anzsoil.org/def/au/asls/landform/mode-of-geomorphological-activity"^^xsd:anyURI ;
  rdfs:comment """Gradational activities are those that tend to reduce the land to a common elevation by removing material from higher places and depositing it in lower places (Chamberlin and Salisbury 1904, page 2), without necessarily reducing the angle of slope at every point. The work of streams and landslides is almost entirely in the gradational modes. However, this tendency is opposed by many processes that commonly act in an anti-gradational mode. These modes are characteristic of volcanism, diastrophism and various kinds of human and biological activity.
However, many engineering works involve erosion and aggradation because these gradational modes use less energy than anti-gradational modes. For the same reason, erosion and aggradation may easily be induced unintentionally by land use (pages 92–96).
To judge the mode of geomorphological activity responsible for a given landform element, the observer must visualise a former surface that has suffered distortion, burial or removal of material, and seek evidence that such activity has taken place. (Information on soil and substrate materials relevant to this investigation should be recorded as specified in other sections.)
Allow for the recording of more than one mode of activity, together with options concerning geomorphological agents."""@en ;
  skos:definition "Various modes of geomorphological activity may be distinguished (Figure 3)."@en ;
  skos:member lf:mode-of-geomorphological-activity-AG ;
  skos:member lf:mode-of-geomorphological-activity-BU ;
  skos:member lf:mode-of-geomorphological-activity-EA ;
  skos:member lf:mode-of-geomorphological-activity-ER ;
  skos:member lf:mode-of-geomorphological-activity-EX ;
  skos:member lf:mode-of-geomorphological-activity-HU ;
  skos:member lf:mode-of-geomorphological-activity-SU ;
  skos:prefLabel "Mode of geomorphological activity"@en ;
.
lf:mode-of-geomorphological-activity-AG
  a skos:Concept ;
  skos-ext:isMemberOf lf:mode-of-geomorphological-activity ;
  dcterms:identifier "http://anzsoil.org/def/au/asls/landform/mode-of-geomorphological-activity-AG"^^xsd:anyURI ;
  skos:definition "Aggraded (Gradational activity)."@en ;
  skos:inScheme asls:landform ;
  skos:notation "AG" ;
  skos:prefLabel "Aggraded"@en ;
  skos:topConceptOf asls:landform ;
.
lf:mode-of-geomorphological-activity-BU
  a skos:Concept ;
  skos-ext:isMemberOf lf:mode-of-geomorphological-activity ;
  dcterms:identifier "http://anzsoil.org/def/au/asls/landform/mode-of-geomorphological-activity-BU"^^xsd:anyURI ;
  skos:definition "Built up (Anti-gradational activity)."@en ;
  skos:inScheme asls:landform ;
  skos:notation "BU" ;
  skos:prefLabel "Built up"@en ;
  skos:topConceptOf asls:landform ;
.
lf:mode-of-geomorphological-activity-EA
  a skos:Concept ;
  skos-ext:isMemberOf lf:mode-of-geomorphological-activity ;
  dcterms:identifier "http://anzsoil.org/def/au/asls/landform/mode-of-geomorphological-activity-EA"^^xsd:anyURI ;
  skos:definition "Eroded or aggraded (Gradational activity)."@en ;
  skos:inScheme asls:landform ;
  skos:notation "EA" ;
  skos:prefLabel "Eroded or aggraded"@en ;
  skos:topConceptOf asls:landform ;
.
lf:mode-of-geomorphological-activity-ER
  a skos:Concept ;
  skos-ext:isMemberOf lf:mode-of-geomorphological-activity ;
  dcterms:identifier "http://anzsoil.org/def/au/asls/landform/mode-of-geomorphological-activity-ER"^^xsd:anyURI ;
  skos:definition "Eroded (Gradational activity)."@en ;
  skos:inScheme asls:landform ;
  skos:notation "ER" ;
  skos:prefLabel "Eroded"@en ;
  skos:topConceptOf asls:landform ;
.
lf:mode-of-geomorphological-activity-EX
  a skos:Concept ;
  skos-ext:isMemberOf lf:mode-of-geomorphological-activity ;
  dcterms:identifier "http://anzsoil.org/def/au/asls/landform/mode-of-geomorphological-activity-EX"^^xsd:anyURI ;
  skos:definition "Excavated or dug out (Anti-gradational activity)."@en ;
  skos:inScheme asls:landform ;
  skos:notation "EX" ;
  skos:prefLabel "Excavated or dug out"@en ;
  skos:topConceptOf asls:landform ;
.
lf:mode-of-geomorphological-activity-HU
  a skos:Concept ;
  skos-ext:isMemberOf lf:mode-of-geomorphological-activity ;
  dcterms:identifier "http://anzsoil.org/def/au/asls/landform/mode-of-geomorphological-activity-HU"^^xsd:anyURI ;
  skos:definition "Heaved up or elevated (Anti-gradational activity)."@en ;
  skos:inScheme asls:landform ;
  skos:notation "HU" ;
  skos:prefLabel "Heaved up or elevated"@en ;
  skos:topConceptOf asls:landform ;
.
lf:mode-of-geomorphological-activity-SU
  a skos:Concept ;
  skos-ext:isMemberOf lf:mode-of-geomorphological-activity ;
  dcterms:identifier "http://anzsoil.org/def/au/asls/landform/mode-of-geomorphological-activity-SU"^^xsd:anyURI ;
  skos:definition "Subsided or depressed (Anti-gradational activity)."@en ;
  skos:inScheme asls:landform ;
  skos:notation "SU" ;
  skos:prefLabel "Subsided or depressed"@en ;
  skos:topConceptOf asls:landform ;
.
lf:morphological-type
  a skos:Collection ;
  a sosa:ObservableProperty ;
  dcterms:identifier "http://anzsoil.org/def/au/asls/landform/morphological-types"^^xsd:anyURI ;
  skos:definition "Landform elements fall into morphological types as sketched in Figure 1. Ten types are distinguished."@en ;
  skos:member lf:compound-morphological-types ;
  skos:member lf:morphological-type-C ;
  skos:member lf:morphological-type-D ;
  skos:member lf:morphological-type-F ;
  skos:member lf:morphological-type-H ;
  skos:member lf:morphological-type-L ;
  skos:member lf:morphological-type-LA ;
  skos:member lf:morphological-type-LI ;
  skos:member lf:morphological-type-LN ;
  skos:member lf:morphological-type-LX ;
  skos:member lf:morphological-type-M ;
  skos:member lf:morphological-type-MA ;
  skos:member lf:morphological-type-MI ;
  skos:member lf:morphological-type-MN ;
  skos:member lf:morphological-type-MX ;
  skos:member lf:morphological-type-R ;
  skos:member lf:morphological-type-S ;
  skos:member lf:morphological-type-U ;
  skos:member lf:morphological-type-UA ;
  skos:member lf:morphological-type-UI ;
  skos:member lf:morphological-type-UN ;
  skos:member lf:morphological-type-UX ;
  skos:member lf:morphological-type-V ;
  skos:member lf:relative-inclination-of-slope-elements ;
  skos:prefLabel "Morphological type"@en ;
.
lf:morphological-type-C
  a skos:Concept ;
  skos-ext:isMemberOf lf:morphological-type ;
  dcterms:identifier "http://anzsoil.org/def/au/asls/landform/morphological-type-C"^^xsd:anyURI ;
  skos:definition "Landform element that stands above all, or almost all, points in the adjacent terrain. It is characteristically smoothly convex upwards in downslope profile or in contour, or both. The margin of a crest element should be drawn at the limit of observed curvature."@en ;
  skos:inScheme asls:landform ;
  skos:notation "C" ;
  skos:prefLabel "Crest"@en ;
  skos:topConceptOf asls:landform ;
.
lf:morphological-type-D
  a skos:Concept ;
  skos-ext:isMemberOf lf:morphological-type ;
  dcterms:identifier "http://anzsoil.org/def/au/asls/landform/morphological-type-D"^^xsd:anyURI ;
  rdfs:comment "Many depressions are concave upwards and their margins should be drawn at the limit of observed curvature."@en ;
  skos:definition "Landform element that stands below all, or almost all, points in the adjacent terrain. A closed depression stands below all such points."@en ;
  skos:inScheme asls:landform ;
  skos:notation "D" ;
  skos:prefLabel "Closed depression"@en ;
  skos:topConceptOf asls:landform ;
.
lf:morphological-type-F
  a skos:Concept ;
  skos-ext:isMemberOf lf:morphological-type ;
  dcterms:identifier "http://anzsoil.org/def/au/asls/landform/morphological-type-F"^^xsd:anyURI ;
  skos:definition "planar landform element that is neither a crest nor a depression and is level or very gently inclined (less than 3% tangent approximately)."@en ;
  skos:inScheme asls:landform ;
  skos:notation "F" ;
  skos:prefLabel "Flat"@en ;
  skos:topConceptOf asls:landform ;
.
lf:morphological-type-H
  a skos:Concept ;
  skos-ext:isMemberOf lf:morphological-type ;
  dcterms:identifier "http://anzsoil.org/def/au/asls/landform/morphological-type-H"^^xsd:anyURI ;
  skos:definition "compound landform element comprising a narrow crest and short adjoining slopes, the crest length being less than the width of the landform element."@en ;
  skos:inScheme asls:landform ;
  skos:notation "H" ;
  skos:prefLabel "Hillock"@en ;
  skos:topConceptOf asls:landform ;
.
lf:morphological-type-L
  a skos:Concept ;
  skos-ext:isMemberOf lf:morphological-type ;
  dcterms:identifier "http://anzsoil.org/def/au/asls/landform/morphological-type-L"^^xsd:anyURI ;
  rdfs:comment """This morphological type is distinguished on its position in the toposequence relative to crests, flats and depressions.
This morphological type requires a relative inclination of slope element modifier."""@en ;
  skos:definition "slope element not adjacent below a crest or flat but adjacent above a flat or depression."@en ;
  skos:inScheme asls:landform ;
  skos:notation "L" ;
  skos:prefLabel "Lower slope (requires inclination modifier)"@en ;
  skos:topConceptOf asls:landform ;
.
lf:morphological-type-LA
  a skos:Concept ;
  skos-ext:isMemberOf lf:morphological-type ;
  dcterms:identifier "http://anzsoil.org/def/au/asls/landform/morphological-type-LA"^^xsd:anyURI ;
  rdfs:comment """This morphological type is distinguished on its position in the toposequence relative to crests, flats and depressions.
This morphological type has a relative inclination of slope element modifier."""@en ;
  skos:definition "slope element not adjacent below a crest or flat but adjacent above a flat or depression and is maximal."@en ;
  skos:inScheme asls:landform ;
  skos:notation "LA" ;
  skos:prefLabel "Lower slope Maximal"@en ;
  skos:topConceptOf asls:landform ;
.
lf:morphological-type-LI
  a skos:Concept ;
  skos-ext:isMemberOf lf:morphological-type ;
  dcterms:identifier "http://anzsoil.org/def/au/asls/landform/morphological-type-LI"^^xsd:anyURI ;
  rdfs:comment """This morphological type is distinguished on its position in the toposequence relative to crests, flats and depressions.
This morphological type has a relative inclination of slope element modifier."""@en ;
  skos:definition "slope element not adjacent below a crest or flat but adjacent above a flat or depression and is minimal."@en ;
  skos:inScheme asls:landform ;
  skos:notation "LI" ;
  skos:prefLabel "Lower slope Minimal"@en ;
  skos:topConceptOf asls:landform ;
.
lf:morphological-type-LN
  a skos:Concept ;
  skos-ext:isMemberOf lf:morphological-type ;
  dcterms:identifier "http://anzsoil.org/def/au/asls/landform/morphological-type-LN"^^xsd:anyURI ;
  rdfs:comment """This morphological type is distinguished on its position in the toposequence relative to crests, flats and depressions.
This morphological type has a relative inclination of slope element modifier."""@en ;
  skos:definition "slope element not adjacent below a crest or flat but adjacent above a flat or depression and is waning."@en ;
  skos:inScheme asls:landform ;
  skos:notation "LN" ;
  skos:prefLabel "Lower slope Waning"@en ;
  skos:topConceptOf asls:landform ;
.
lf:morphological-type-LX
  a skos:Concept ;
  skos-ext:isMemberOf lf:morphological-type ;
  dcterms:identifier "http://anzsoil.org/def/au/asls/landform/morphological-type-LX"^^xsd:anyURI ;
  rdfs:comment """This morphological type is distinguished on its position in the toposequence relative to crests, flats and depressions.
This morphological type has a relative inclination of slope element modifier."""@en ;
  skos:definition "slope element not adjacent below a crest or flat but adjacent above a flat or depression and is waxing."@en ;
  skos:inScheme asls:landform ;
  skos:notation "LX" ;
  skos:prefLabel "Lower slope Waxing"@en ;
  skos:topConceptOf asls:landform ;
.
lf:morphological-type-M
  a skos:Concept ;
  skos-ext:isMemberOf lf:morphological-type ;
  dcterms:identifier "http://anzsoil.org/def/au/asls/landform/morphological-type-M"^^xsd:anyURI ;
  rdfs:comment """This morphological type is distinguished on its position in the toposequence relative to crests, flats and depressions.
This morphological type requires a relative inclination of slope element modifier."""@en ;
  skos:definition "slope element not adjacent below a crest or flat and not adjacent above a flat or depression."@en ;
  skos:inScheme asls:landform ;
  skos:notation "M" ;
  skos:prefLabel "Mid-slope (requires inclination modifier)"@en ;
  skos:topConceptOf asls:landform ;
.
lf:morphological-type-MA
  a skos:Concept ;
  skos-ext:isMemberOf lf:morphological-type ;
  dcterms:identifier "http://anzsoil.org/def/au/asls/landform/morphological-type-MA"^^xsd:anyURI ;
  rdfs:comment """This morphological type is distinguished on its position in the toposequence relative to crests, flats and depressions.
This morphological type has a relative inclination of slope element modifier."""@en ;
  skos:definition "slope element not adjacent below a crest or flat and not adjacent above a flat or depression and is maximal."@en ;
  skos:inScheme asls:landform ;
  skos:notation "MA" ;
  skos:prefLabel "Mid-slope Maximal"@en ;
  skos:topConceptOf asls:landform ;
.
lf:morphological-type-MI
  a skos:Concept ;
  skos-ext:isMemberOf lf:morphological-type ;
  dcterms:identifier "http://anzsoil.org/def/au/asls/landform/morphological-type-MI"^^xsd:anyURI ;
  rdfs:comment """This morphological type is distinguished on its position in the toposequence relative to crests, flats and depressions.
This morphological type has a relative inclination of slope element modifier."""@en ;
  skos:definition "slope element not adjacent below a crest or flat and not adjacent above a flat or depression and is minimal."@en ;
  skos:inScheme asls:landform ;
  skos:notation "MI" ;
  skos:prefLabel "Mid-slope Minimal"@en ;
  skos:topConceptOf asls:landform ;
.
lf:morphological-type-MN
  a skos:Concept ;
  skos-ext:isMemberOf lf:morphological-type ;
  dcterms:identifier "http://anzsoil.org/def/au/asls/landform/morphological-type-MN"^^xsd:anyURI ;
  rdfs:comment """This morphological type is distinguished on its position in the toposequence relative to crests, flats and depressions.
This morphological type has a relative inclination of slope element modifier."""@en ;
  skos:definition "slope element not adjacent below a crest or flat and not adjacent above a flat or depression and is waning."@en ;
  skos:inScheme asls:landform ;
  skos:notation "MN" ;
  skos:prefLabel "Mid-slope Waning"@en ;
  skos:topConceptOf asls:landform ;
.
lf:morphological-type-MX
  a skos:Concept ;
  skos-ext:isMemberOf lf:morphological-type ;
  dcterms:identifier "http://anzsoil.org/def/au/asls/landform/morphological-type-MX"^^xsd:anyURI ;
  rdfs:comment """This morphological type is distinguished on its position in the toposequence relative to crests, flats and depressions.
This morphological type has a relative inclination of slope element modifier."""@en ;
  skos:definition "slope element not adjacent below a crest or flat and not adjacent above a flat or depression and is waxing."@en ;
  skos:inScheme asls:landform ;
  skos:notation "MX" ;
  skos:prefLabel "Mid-slope Waxing"@en ;
  skos:topConceptOf asls:landform ;
.
lf:morphological-type-R
  a skos:Concept ;
  skos-ext:isMemberOf lf:morphological-type ;
  dcterms:identifier "http://anzsoil.org/def/au/asls/landform/morphological-type-R"^^xsd:anyURI ;
  skos:definition "compound landform element comprising a narrow crest and short adjoining slopes, the crest length being greater than the width of the landform element."@en ;
  skos:inScheme asls:landform ;
  skos:notation "R" ;
  skos:prefLabel "Ridge"@en ;
  skos:topConceptOf asls:landform ;
.
lf:morphological-type-S
  a skos:Concept ;
  skos-ext:isMemberOf lf:morphological-type ;
  dcterms:identifier "http://anzsoil.org/def/au/asls/landform/morphological-type-S"^^xsd:anyURI ;
  rdfs:comment "This morphological type is distinguished on its position in the toposequence relative to crests, flats and depressions."@en ;
  skos:definition "slope element adjacent below a crest or flat and adjacent above a flat or depression."@en ;
  skos:inScheme asls:landform ;
  skos:notation "S" ;
  skos:prefLabel "Simple slope"@en ;
  skos:topConceptOf asls:landform ;
.
lf:morphological-type-U
  a skos:Concept ;
  skos-ext:isMemberOf lf:morphological-type ;
  dcterms:identifier "http://anzsoil.org/def/au/asls/landform/morphological-type-U"^^xsd:anyURI ;
  rdfs:comment """This morphological type is distinguished on its position in the toposequence relative to crests, flats and depressions.
This morphological type requires a relative inclination of slope element modifier."""@en ;
  skos:definition "slope element adjacent below a crest or flat but not adjacent above a flat or depression."@en ;
  skos:inScheme asls:landform ;
  skos:notation "U" ;
  skos:prefLabel "Upper slope (requires inclination modifier)"@en ;
  skos:topConceptOf asls:landform ;
.
lf:morphological-type-UA
  a skos:Concept ;
  skos-ext:isMemberOf lf:morphological-type ;
  dcterms:identifier "http://anzsoil.org/def/au/asls/landform/morphological-type-UA"^^xsd:anyURI ;
  rdfs:comment """This morphological type is distinguished on its position in the toposequence relative to crests, flats and depressions.
This morphological type has a relative inclination of slope element modifier."""@en ;
  skos:definition "slope element adjacent below a crest or flat but not adjacent above a flat or depression and is maximal."@en ;
  skos:inScheme asls:landform ;
  skos:notation "UA" ;
  skos:prefLabel "Upper slope Maximal"@en ;
  skos:topConceptOf asls:landform ;
.
lf:morphological-type-UI
  a skos:Concept ;
  skos-ext:isMemberOf lf:morphological-type ;
  dcterms:identifier "http://anzsoil.org/def/au/asls/landform/morphological-type-UI"^^xsd:anyURI ;
  rdfs:comment """This morphological type is distinguished on its position in the toposequence relative to crests, flats and depressions.
This morphological type has a relative inclination of slope element modifier."""@en ;
  skos:definition "slope element adjacent below a crest or flat but not adjacent above a flat or depression and is minimal."@en ;
  skos:inScheme asls:landform ;
  skos:notation "UI" ;
  skos:prefLabel "Upper slope Minimal"@en ;
  skos:topConceptOf asls:landform ;
.
lf:morphological-type-UN
  a skos:Concept ;
  skos-ext:isMemberOf lf:morphological-type ;
  dcterms:identifier "http://anzsoil.org/def/au/asls/landform/morphological-type-UN"^^xsd:anyURI ;
  rdfs:comment """This morphological type is distinguished on its position in the toposequence relative to crests, flats and depressions.
This morphological type has a relative inclination of slope element modifier."""@en ;
  skos:definition "slope element adjacent below a crest or flat but not adjacent above a flat or depression and is waning."@en ;
  skos:inScheme asls:landform ;
  skos:notation "UN" ;
  skos:prefLabel "Upper slope Waning"@en ;
  skos:topConceptOf asls:landform ;
.
lf:morphological-type-UX
  a skos:Concept ;
  skos-ext:isMemberOf lf:morphological-type ;
  dcterms:identifier "http://anzsoil.org/def/au/asls/landform/morphological-type-UX"^^xsd:anyURI ;
  rdfs:comment """This morphological type is distinguished on its position in the toposequence relative to crests, flats and depressions.
This morphological type has a relative inclination of slope element modifier."""@en ;
  skos:definition "slope element adjacent below a crest or flat but not adjacent above a flat or depression and is waxing."@en ;
  skos:inScheme asls:landform ;
  skos:notation "UX" ;
  skos:prefLabel "Upper slope Waxing"@en ;
  skos:topConceptOf asls:landform ;
.
lf:morphological-type-V
  a skos:Concept ;
  skos-ext:isMemberOf lf:morphological-type ;
  dcterms:identifier "http://anzsoil.org/def/au/asls/landform/morphological-type-V"^^xsd:anyURI ;
  rdfs:comment "Many depressions are concave upwards and their margins should be drawn at the limit of observed curvature."@en ;
  skos:definition "Landform element that stands below all, or almost all, points in the adjacent terrain. An open depression extends at the same elevation, or lower."@en ;
  skos:inScheme asls:landform ;
  skos:notation "V" ;
  skos:prefLabel "Open depression (vale)"@en ;
  skos:topConceptOf asls:landform ;
.
lf:observable-properties
  a skos:Collection ;
  skos:member lf:element-dimension-height ;
  skos:member lf:element-dimension-length ;
  skos:member lf:element-dimension-width ;
  skos:member lf:geomorphological-agents ;
  skos:member lf:location-within-the-landform-element ;
  skos:member lf:location-within-toposequence ;
  skos:member lf:modal-slope ;
  skos:member lf:mode-of-geomorphological-activity ;
  skos:member lf:morphological-type ;
  skos:member lf:relative-inclination-of-slope-elements ;
  skos:member lf:relief ;
  skos:member lf:slope-class ;
  skos:member lf:slope-value ;
  skos:member lf:stream-channel-development ;
  skos:member lf:stream-channel-migration ;
  skos:member lf:stream-channel-network-directionality ;
  skos:member lf:stream-channel-network-integration ;
  skos:member lf:stream-channel-occurence ;
  skos:member lf:stream-channel-relative-depth-width ;
  skos:member lf:stream-channel-spacing ;
  skos:member lf:streamwise-channel-pattern ;
  skos:prefLabel "Observable properties of landforms" ;
.
lf:relative-inclination-of-slope-elements
  a skos:Collection ;
  a sosa:ObservableProperty ;
  dcterms:identifier "http://anzsoil.org/def/au/asls/landform/relative-inclination-of-slope-elements"^^xsd:anyURI ;
  skos:definition "Although lower slopes are often gentler than upper slopes, they need not be so (Figure 1i). A separate morphological attribute expresses the relative inclination of adjacent landform elements in a toposequence."@en ;
  skos:member lf:relative-inclination-of-slope-elements-A ;
  skos:member lf:relative-inclination-of-slope-elements-I ;
  skos:member lf:relative-inclination-of-slope-elements-N ;
  skos:member lf:relative-inclination-of-slope-elements-X ;
  skos:prefLabel "Relative inclination of slope elements"@en ;
.
lf:relative-inclination-of-slope-elements-A
  a skos:Concept ;
  skos-ext:isMemberOf lf:relative-inclination-of-slope-elements ;
  dcterms:identifier "http://anzsoil.org/def/au/asls/landform/relative-inclination-of-slope-elements-A"^^xsd:anyURI ;
  skos:definition "element upslope is gentler, element downslope is gentler."@en ;
  skos:inScheme asls:landform ;
  skos:notation "A" ;
  skos:prefLabel "Maximal"@en ;
  skos:topConceptOf asls:landform ;
.
lf:relative-inclination-of-slope-elements-I
  a skos:Concept ;
  skos-ext:isMemberOf lf:relative-inclination-of-slope-elements ;
  dcterms:identifier "http://anzsoil.org/def/au/asls/landform/relative-inclination-of-slope-elements-I"^^xsd:anyURI ;
  skos:definition "element upslope is steeper, element downslope is steeper."@en ;
  skos:inScheme asls:landform ;
  skos:notation "I" ;
  skos:prefLabel "Minimal"@en ;
  skos:topConceptOf asls:landform ;
.
lf:relative-inclination-of-slope-elements-N
  a skos:Concept ;
  skos-ext:isMemberOf lf:relative-inclination-of-slope-elements ;
  dcterms:identifier "http://anzsoil.org/def/au/asls/landform/relative-inclination-of-slope-elements-N"^^xsd:anyURI ;
  skos:definition "element upslope is steeper, element downslope is gentler."@en ;
  skos:inScheme asls:landform ;
  skos:notation "N" ;
  skos:prefLabel "Waning"@en ;
  skos:topConceptOf asls:landform ;
.
lf:relative-inclination-of-slope-elements-X
  a skos:Concept ;
  skos-ext:isMemberOf lf:relative-inclination-of-slope-elements ;
  dcterms:identifier "http://anzsoil.org/def/au/asls/landform/relative-inclination-of-slope-elements-X"^^xsd:anyURI ;
  skos:definition "element upslope is gentler, element downslope is steeper."@en ;
  skos:inScheme asls:landform ;
  skos:notation "X" ;
  skos:prefLabel "Waxing"@en ;
  skos:topConceptOf asls:landform ;
.
lf:relief
  a skos:Collection ;
  a sosa:ObservableProperty ;
  dcterms:identifier "http://anzsoil.org/def/au/asls/landform/relief"^^xsd:anyURI ;
  skos:definition """Relief is defined as the difference in elevation between the high and low points of a land surface. Its estimation will be made easier by visualising two surfaces of accordance that are planar or gently curved, one touching the major crests of a landform pattern, and the other passing through the major depressions. The average vertical separation of the two surfaces is a measure of the relief. Make this estimation at a field site, either visually or by using a map, and express it in metres.
Relief is the definitive characteristic for the terms mountains, hills, low hills, rises and plains when used as types of erosional landform pattern (Table 5). The class boundaries, shown in Tables 5 and 6, are set at 300 m, 90 m, 30 m and 9 m. These class limits and the class names are similar to those used by Löffler (1974), and are broadly compatible with those of Löffler and Ruxton (1969).
Table 6 lists types of landform pattern defined in the glossary according to their typical relief class. Those types for which the relief class is definitive are in italics."""@en ;
  skos:member lf:relief-class-H ;
  skos:member lf:relief-class-L ;
  skos:member lf:relief-class-M ;
  skos:member lf:relief-class-P ;
  skos:member lf:relief-class-R ;
  skos:prefLabel "Relief"@en ;
.
lf:relief-class-H
  a skos:Concept ;
  skos-ext:isMemberOf lf:relief ;
  dcterms:identifier "http://anzsoil.org/def/au/asls/landform/relief-class-H"^^xsd:anyURI ;
  skos:definition "High relief, 90-300 m, (~150 m)"@en ;
  skos:inScheme asls:landform ;
  skos:notation "H" ;
  skos:prefLabel "High"@en ;
  skos:topConceptOf asls:landform ;
.
lf:relief-class-L
  a skos:Concept ;
  skos-ext:isMemberOf lf:relief ;
  dcterms:identifier "http://anzsoil.org/def/au/asls/landform/relief-class-L"^^xsd:anyURI ;
  skos:definition "Low relief, 30-90 m, (~50 m)"@en ;
  skos:inScheme asls:landform ;
  skos:notation "L" ;
  skos:prefLabel "Low"@en ;
  skos:topConceptOf asls:landform ;
.
lf:relief-class-M
  a skos:Concept ;
  skos-ext:isMemberOf lf:relief ;
  dcterms:identifier "http://anzsoil.org/def/au/asls/landform/relief-class-M"^^xsd:anyURI ;
  skos:definition "Very high relief, >300 m, (~500 m)"@en ;
  skos:inScheme asls:landform ;
  skos:notation "M" ;
  skos:prefLabel "Very high"@en ;
  skos:topConceptOf asls:landform ;
.
lf:relief-class-P
  a skos:Concept ;
  skos-ext:isMemberOf lf:relief ;
  dcterms:identifier "http://anzsoil.org/def/au/asls/landform/relief-class-P"^^xsd:anyURI ;
  skos:definition "Extremely low relief, <9 m, (~5 m)"@en ;
  skos:inScheme asls:landform ;
  skos:notation "P" ;
  skos:prefLabel "Extremely low"@en ;
  skos:topConceptOf asls:landform ;
.
lf:relief-class-R
  a skos:Concept ;
  skos-ext:isMemberOf lf:relief ;
  dcterms:identifier "http://anzsoil.org/def/au/asls/landform/relief-class-R"^^xsd:anyURI ;
  skos:definition "Very low relief, 9-30 m, (~15 m)"@en ;
  skos:inScheme asls:landform ;
  skos:notation "R" ;
  skos:prefLabel "Very low"@en ;
  skos:topConceptOf asls:landform ;
.
lf:simple-erosional-landform-pattern-B
  a skos:Concept ;
  skos-ext:isMemberOf lf:simple-erosional-landform-patterns ;
  dcterms:identifier "http://anzsoil.org/def/au/asls/landform/simple-erosional-landform-pattern-B"^^xsd:anyURI ;
  skos:definition "The Badlands simple erosional landform pattern is defined by various combinations of high slope values and low relief values. These combinations imply extremely close spacing of streams or valleys. Specifically, if one assumes a sawtooth terrain profile, the valley spacing implied is less than 100 m in areas with 50 m relief and less than 30 m in areas with 5 m relief; these values appear to accord with usage."@en ;
  skos:inScheme asls:landform ;
  skos:notation "B" ;
  skos:prefLabel "Badlands (simple erosional pattern)"@en ;
  skos:related lf:landform-pattern-BAD ;
  skos:topConceptOf asls:landform ;
.
lf:simple-erosional-landform-pattern-GP
  a skos:Concept ;
  skos-ext:isMemberOf lf:simple-erosional-landform-patterns ;
  dcterms:identifier "http://anzsoil.org/def/au/asls/landform/simple-erosional-landform-pattern-GP"^^xsd:anyURI ;
  skos:definition """<p>Gently undulating plain is a simple type of erosional landform pattern characterised by Extremely low relief and Very gently inclined modal slope.</p>
<p>Relief is Extremely low < 9m (~5m)</p>
<p>Modal terrain slope is Very gently inclined 1-3% (~2%)</p>""" ;
  skos:inScheme asls:landform ;
  skos:notation "GP" ;
  skos:prefLabel "Gently undulating plain"@en ;
  skos:related lf:relief-class-P ;
  skos:related lf:slope-class-VG ;
  skos:topConceptOf asls:landform ;
.
lf:simple-erosional-landform-pattern-GR
  a skos:Concept ;
  skos-ext:isMemberOf lf:simple-erosional-landform-patterns ;
  dcterms:identifier "http://anzsoil.org/def/au/asls/landform/simple-erosional-landform-pattern-GR"^^xsd:anyURI ;
  skos:definition """<p>Gently undulating rises is a simple type of erosional landform pattern characterised by Very low relief and Very gently inclined modal slope.</p>
<p>Relief is Very low < 9-30m (~15m)</p>
<p>Modal terrain slope is Very gently inclined 1-3% (~2%)</p>""" ;
  skos:inScheme asls:landform ;
  skos:notation "GR" ;
  skos:prefLabel "Gently undulating rises"@en ;
  skos:related lf:relief-class-R ;
  skos:related lf:slope-class-VG ;
  skos:topConceptOf asls:landform ;
.
lf:simple-erosional-landform-pattern-LP
  a skos:Concept ;
  skos-ext:isMemberOf lf:simple-erosional-landform-patterns ;
  dcterms:identifier "http://anzsoil.org/def/au/asls/landform/simple-erosional-landform-pattern-LP"^^xsd:anyURI ;
  skos:definition """<p>Level plain is a simple type of erosional landform pattern characterised by Extremely low relief and Level modal slope.</p>
<p>Relief is Extremely low < 9m (~5m)</p>
<p>Modal terrain slope is Level < 1% (~1:300)</p>""" ;
  skos:inScheme asls:landform ;
  skos:notation "LP" ;
  skos:prefLabel "Level plain"@en ;
  skos:related lf:relief-class-P ;
  skos:related lf:slope-class-LE ;
  skos:topConceptOf asls:landform ;
.
lf:simple-erosional-landform-pattern-PH
  a skos:Concept ;
  skos-ext:isMemberOf lf:simple-erosional-landform-patterns ;
  dcterms:identifier "http://anzsoil.org/def/au/asls/landform/simple-erosional-landform-pattern-PH"^^xsd:anyURI ;
  skos:definition """<p>Precipitous hills is a simple type of erosional landform pattern characterised by High relief and Precipitous modal slope.</p>
<p>Relief is High 90-300m (~150m)</p>
<p>Modal terrain slope is Precipitous >100% (~150%)</p>""" ;
  skos:inScheme asls:landform ;
  skos:notation "PH" ;
  skos:prefLabel "Precipitous hills"@en ;
  skos:related lf:relief-class-H ;
  skos:related lf:slope-class-PR ;
  skos:topConceptOf asls:landform ;
.
lf:simple-erosional-landform-pattern-PM
  a skos:Concept ;
  skos-ext:isMemberOf lf:simple-erosional-landform-patterns ;
  dcterms:identifier "http://anzsoil.org/def/au/asls/landform/simple-erosional-landform-pattern-PM"^^xsd:anyURI ;
  skos:definition """<p>Precipitous mountains is a simple type of erosional landform pattern characterised by Very high relief and Precipitous modal slope.</p>
<p>Relief is Very high >300m (~500m)</p>
<p>Modal terrain slope is Precipitous >100% (~150%)</p>""" ;
  skos:inScheme asls:landform ;
  skos:notation "PM" ;
  skos:prefLabel "Precipitous mountains"@en ;
  skos:related lf:relief-class-M ;
  skos:related lf:slope-class-PR ;
  skos:topConceptOf asls:landform ;
.
lf:simple-erosional-landform-pattern-RH
  a skos:Concept ;
  skos-ext:isMemberOf lf:simple-erosional-landform-patterns ;
  dcterms:identifier "http://anzsoil.org/def/au/asls/landform/simple-erosional-landform-pattern-RH"^^xsd:anyURI ;
  skos:definition """<p>Rolling hills is a simple type of erosional landform pattern characterised by High relief and Moderately inclined modal slope.</p>
<p>Relief is High 90-300m (~150m)</p>
<p>Modal terrain slope is Moderately inclined 10-32% (~20%)</p>""" ;
  skos:inScheme asls:landform ;
  skos:notation "RH" ;
  skos:prefLabel "Rolling hills"@en ;
  skos:related lf:relief-class-H ;
  skos:related lf:slope-class-MO ;
  skos:topConceptOf asls:landform ;
.
lf:simple-erosional-landform-pattern-RL
  a skos:Concept ;
  skos-ext:isMemberOf lf:simple-erosional-landform-patterns ;
  dcterms:identifier "http://anzsoil.org/def/au/asls/landform/simple-erosional-landform-pattern-RL"^^xsd:anyURI ;
  skos:definition """<p>Rolling low hills is a simple type of erosional landform pattern characterised by Low relief and Moderately inclined modal slope.</p>
<p>Relief is Low 30-90m (~50m)</p>
<p>Modal terrain slope is Moderately inclined 10-32% (~20%)</p>""" ;
  skos:inScheme asls:landform ;
  skos:notation "RL" ;
  skos:prefLabel "Rolling low hills"@en ;
  skos:related lf:relief-class-L ;
  skos:related lf:slope-class-MO ;
  skos:topConceptOf asls:landform ;
.
lf:simple-erosional-landform-pattern-RM
  a skos:Concept ;
  skos-ext:isMemberOf lf:simple-erosional-landform-patterns ;
  dcterms:identifier "http://anzsoil.org/def/au/asls/landform/simple-erosional-landform-pattern-RM"^^xsd:anyURI ;
  skos:definition """<p>Rolling mountains is a simple type of erosional landform pattern characterised by Very high relief and Moderately inclined modal slope.</p>
<p>Relief is Very high >300m (~500m)</p>
<p>Modal terrain slope is Moderately inclined 10-32% (~20%)</p>""" ;
  skos:inScheme asls:landform ;
  skos:notation "RM" ;
  skos:prefLabel "Rolling mountains"@en ;
  skos:related lf:relief-class-M ;
  skos:related lf:slope-class-MO ;
  skos:topConceptOf asls:landform ;
.
lf:simple-erosional-landform-pattern-RP
  a skos:Concept ;
  skos-ext:isMemberOf lf:simple-erosional-landform-patterns ;
  dcterms:identifier "http://anzsoil.org/def/au/asls/landform/simple-erosional-landform-pattern-RP"^^xsd:anyURI ;
  skos:definition """<p>Rolling plain is a simple type of erosional landform pattern characterised by Extremely low relief and Moderately inclined modal slope.</p>
<p>Relief is Extremely low < 9m (~5m)</p>
<p>Modal terrain slope is Moderately inclined 10-32% (~20%)</p>""" ;
  skos:inScheme asls:landform ;
  skos:notation "RP" ;
  skos:prefLabel "Rolling plain"@en ;
  skos:related lf:relief-class-P ;
  skos:related lf:slope-class-MO ;
  skos:topConceptOf asls:landform ;
.
lf:simple-erosional-landform-pattern-RR
  a skos:Concept ;
  skos-ext:isMemberOf lf:simple-erosional-landform-patterns ;
  dcterms:identifier "http://anzsoil.org/def/au/asls/landform/simple-erosional-landform-pattern-RR"^^xsd:anyURI ;
  skos:definition """<p>Rolling rises is a simple type of erosional landform pattern characterised by Very low relief and Moderately inclined modal slope.</p>
<p>Relief is Very low 9-30m (~15m)</p>
<p>Modal terrain slope is Moderately inclined 10-32% (~20%)</p>""" ;
  skos:inScheme asls:landform ;
  skos:notation "RR" ;
  skos:prefLabel "Rolling rises"@en ;
  skos:related lf:relief-class-R ;
  skos:related lf:slope-class-MO ;
  skos:topConceptOf asls:landform ;
.
lf:simple-erosional-landform-pattern-SH
  a skos:Concept ;
  skos-ext:isMemberOf lf:simple-erosional-landform-patterns ;
  dcterms:identifier "http://anzsoil.org/def/au/asls/landform/simple-erosional-landform-pattern-SH"^^xsd:anyURI ;
  skos:definition """<p>Steep hills is a simple type of erosional landform pattern characterised by High relief and Steep modal slope.</p>
<p>Relief is High 90-300m (~150m)</p>
<p>Modal terrain slope is Steep 32-56% (~40%)</p>""" ;
  skos:inScheme asls:landform ;
  skos:notation "SH" ;
  skos:prefLabel "Steep hills"@en ;
  skos:related lf:relief-class-H ;
  skos:related lf:slope-class-ST ;
  skos:topConceptOf asls:landform ;
.
lf:simple-erosional-landform-pattern-SL
  a skos:Concept ;
  skos-ext:isMemberOf lf:simple-erosional-landform-patterns ;
  dcterms:identifier "http://anzsoil.org/def/au/asls/landform/simple-erosional-landform-pattern-SL"^^xsd:anyURI ;
  skos:definition """<p>Steep low hills is a simple type of erosional landform pattern characterised by Low relief and Steep modal slope.</p>
<p>Relief is Low 30-90m (~50m)</p>
<p>Modal terrain slope is Steep 32-56% (~40%)</p>""" ;
  skos:inScheme asls:landform ;
  skos:notation "SL" ;
  skos:prefLabel "Steep low hills"@en ;
  skos:related lf:relief-class-L ;
  skos:related lf:slope-class-ST ;
  skos:topConceptOf asls:landform ;
.
lf:simple-erosional-landform-pattern-SM
  a skos:Concept ;
  skos-ext:isMemberOf lf:simple-erosional-landform-patterns ;
  dcterms:identifier "http://anzsoil.org/def/au/asls/landform/simple-erosional-landform-pattern-SM"^^xsd:anyURI ;
  skos:definition """<p>Steep mountains is a simple type of erosional landform pattern characterised by Very high relief and Steep modal slope.</p>
<p>Relief is Very high > 300m (~500m)</p>
<p>Modal terrain slope is Steep 32-56% (~40%)</p>""" ;
  skos:inScheme asls:landform ;
  skos:notation "SM" ;
  skos:prefLabel "Steep mountains"@en ;
  skos:related lf:relief-class-M ;
  skos:related lf:slope-class-ST ;
  skos:topConceptOf asls:landform ;
.
lf:simple-erosional-landform-pattern-SR
  a skos:Concept ;
  skos-ext:isMemberOf lf:simple-erosional-landform-patterns ;
  dcterms:identifier "http://anzsoil.org/def/au/asls/landform/simple-erosional-landform-pattern-SR"^^xsd:anyURI ;
  skos:definition """<p>Steep rises is a simple type of erosional landform pattern characterised by Very low relief and Steep modal slope.</p>
<p>Relief is Very low 9-30m (~15m)</p>
<p>Modal terrain slope is Steep 32-56% (~40%)</p>""" ;
  skos:inScheme asls:landform ;
  skos:notation "SR" ;
  skos:prefLabel "Steep rises"@en ;
  skos:related lf:relief-class-R ;
  skos:related lf:slope-class-ST ;
  skos:topConceptOf asls:landform ;
.
lf:simple-erosional-landform-pattern-UH
  a skos:Concept ;
  skos-ext:isMemberOf lf:simple-erosional-landform-patterns ;
  dcterms:identifier "http://anzsoil.org/def/au/asls/landform/simple-erosional-landform-pattern-UH"^^xsd:anyURI ;
  skos:definition """<p>Undulating hills is a simple type of erosional landform pattern characterised by High relief and Gently inclined modal slope.</p>
<p>Relief is High 90-300m (~150m)</p>
<p>Modal terrain slope is Gently inclined 3-10% (~6%)</p>""" ;
  skos:inScheme asls:landform ;
  skos:notation "UH" ;
  skos:prefLabel "Undulating hills"@en ;
  skos:related lf:relief-class-H ;
  skos:related lf:slope-class-GE ;
  skos:topConceptOf asls:landform ;
.
lf:simple-erosional-landform-pattern-UL
  a skos:Concept ;
  skos-ext:isMemberOf lf:simple-erosional-landform-patterns ;
  dcterms:identifier "http://anzsoil.org/def/au/asls/landform/simple-erosional-landform-pattern-UL"^^xsd:anyURI ;
  skos:definition """<p>Undulating low hills is a simple type of erosional landform pattern characterised by Low relief and Gently inclined modal slope.</p>
<p>Relief is Low 30-90m (~50m)</p>
<p>Modal terrain slope is Gently inclined < 3-10% (~6%)</p>""" ;
  skos:inScheme asls:landform ;
  skos:notation "UL" ;
  skos:prefLabel "Undulating low hills"@en ;
  skos:related lf:relief-class-L ;
  skos:related lf:slope-class-GE ;
  skos:topConceptOf asls:landform ;
.
lf:simple-erosional-landform-pattern-UP
  a skos:Concept ;
  skos-ext:isMemberOf lf:simple-erosional-landform-patterns ;
  dcterms:identifier "http://anzsoil.org/def/au/asls/landform/simple-erosional-landform-pattern-UP"^^xsd:anyURI ;
  skos:definition """<p>Undulating plain is a simple type of erosional landform pattern characterised by Extremely low relief and Gently inclined modal slope.</p>
<p>Relief is Extremely low < 9m (~5m)</p>
<p>Modal terrain slope is Gently inclined 3-10% (~6%)</p>""" ;
  skos:inScheme asls:landform ;
  skos:notation "UP" ;
  skos:prefLabel "Undulating plain"@en ;
  skos:related lf:relief-class-P ;
  skos:related lf:slope-class-GE ;
  skos:topConceptOf asls:landform ;
.
lf:simple-erosional-landform-pattern-UR
  a skos:Concept ;
  skos-ext:isMemberOf lf:simple-erosional-landform-patterns ;
  dcterms:identifier "http://anzsoil.org/def/au/asls/landform/simple-erosional-landform-pattern-UR"^^xsd:anyURI ;
  skos:definition """<p>Undulating rises is a simple type of erosional landform pattern characterised by Very low relief and Gently inclined modal slope.</p>
<p>Relief is Very low 9-30m (~15m)</p>
<p>Modal terrain slope is Gently inclined 3-10% (~6%)</p>""" ;
  skos:inScheme asls:landform ;
  skos:notation "UR" ;
  skos:prefLabel "Undulating rises"@en ;
  skos:related lf:relief-class-R ;
  skos:related lf:slope-class-GE ;
  skos:topConceptOf asls:landform ;
.
lf:simple-erosional-landform-pattern-VH
  a skos:Concept ;
  skos-ext:isMemberOf lf:simple-erosional-landform-patterns ;
  dcterms:identifier "http://anzsoil.org/def/au/asls/landform/simple-erosional-landform-pattern-VH"^^xsd:anyURI ;
  skos:definition """<p>Very steep hills is a simple type of erosional landform pattern characterised by High relief and Very steep modal slope.</p>
<p>Relief is High 90-300m (~150m)</p>
<p>Modal terrain slope is Very steep 56-100% (~70%)</p>""" ;
  skos:inScheme asls:landform ;
  skos:notation "VH" ;
  skos:prefLabel "Very steep hills"@en ;
  skos:related lf:relief-class-H ;
  skos:related lf:slope-class-VS ;
  skos:topConceptOf asls:landform ;
.
lf:simple-erosional-landform-pattern-VL
  a skos:Concept ;
  skos-ext:isMemberOf lf:simple-erosional-landform-patterns ;
  dcterms:identifier "http://anzsoil.org/def/au/asls/landform/simple-erosional-landform-pattern-VL"^^xsd:anyURI ;
  skos:definition """<p>Very steep low hills is a simple type of erosional landform pattern characterised by Low relief and Very steep modal slope.</p>
<p>Relief is Low 30-90m (~50m)</p>
<p>Modal terrain slope is Very steep 56-100% (~70%)</p>""" ;
  skos:inScheme asls:landform ;
  skos:notation "VL" ;
  skos:prefLabel "Very steep low hills"@en ;
  skos:related lf:relief-class-L ;
  skos:related lf:slope-class-VS ;
  skos:topConceptOf asls:landform ;
.
lf:simple-erosional-landform-pattern-VM
  a skos:Concept ;
  skos-ext:isMemberOf lf:simple-erosional-landform-patterns ;
  dcterms:identifier "http://anzsoil.org/def/au/asls/landform/simple-erosional-landform-pattern-VM"^^xsd:anyURI ;
  skos:definition """<p>Very steep mountains is a simple type of erosional landform pattern characterised by Very high relief and Very steep modal slope.</p>
<p>Relief is Very high > 300m (~500m)</p>
<p>Modal terrain slope is Very steep 56-100% (~70%)</p>""" ;
  skos:inScheme asls:landform ;
  skos:notation "VM" ;
  skos:prefLabel "Very steep mountains"@en ;
  skos:related lf:relief-class-M ;
  skos:related lf:slope-class-VS ;
  skos:topConceptOf asls:landform ;
.
lf:simple-erosional-landform-patterns
  a skos:Collection ;
  dcterms:identifier "http://anzsoil.org/def/au/asls/landform/simple-erosional-landform-patterns"^^xsd:anyURI ;
  skos:definition "Simple erosional landform patterns are based on relief and modal slope."@en ;
  skos:member lf:simple-erosional-landform-pattern-B ;
  skos:member lf:simple-erosional-landform-pattern-GP ;
  skos:member lf:simple-erosional-landform-pattern-GR ;
  skos:member lf:simple-erosional-landform-pattern-LP ;
  skos:member lf:simple-erosional-landform-pattern-PH ;
  skos:member lf:simple-erosional-landform-pattern-PM ;
  skos:member lf:simple-erosional-landform-pattern-RH ;
  skos:member lf:simple-erosional-landform-pattern-RL ;
  skos:member lf:simple-erosional-landform-pattern-RM ;
  skos:member lf:simple-erosional-landform-pattern-RP ;
  skos:member lf:simple-erosional-landform-pattern-RR ;
  skos:member lf:simple-erosional-landform-pattern-SH ;
  skos:member lf:simple-erosional-landform-pattern-SL ;
  skos:member lf:simple-erosional-landform-pattern-SM ;
  skos:member lf:simple-erosional-landform-pattern-SR ;
  skos:member lf:simple-erosional-landform-pattern-UH ;
  skos:member lf:simple-erosional-landform-pattern-UL ;
  skos:member lf:simple-erosional-landform-pattern-UP ;
  skos:member lf:simple-erosional-landform-pattern-UR ;
  skos:member lf:simple-erosional-landform-pattern-VH ;
  skos:member lf:simple-erosional-landform-pattern-VL ;
  skos:member lf:simple-erosional-landform-pattern-VM ;
  skos:prefLabel "Simple erosional landform patterns"@en ;
.
lf:slope
  a skos:Collection ;
  dcterms:identifier "http://anzsoil.org/def/au/asls/landform/slope"^^xsd:anyURI ;
  skos:definition "Always observe and record the slope as precisely as the chosen survey method permits. The observation should span no less than 20 m so as not to be influenced too much by features of the microrelief that occurs within the landform element."@en ;
  skos:member lf:slope-class ;
  skos:member lf:slope-evaluations ;
  skos:member lf:slope-value ;
  skos:prefLabel "Slope of landform element"@en ;
.
lf:slope-class
  a skos:Collection ;
  a sosa:ObservableProperty ;
  skos-ext:isMemberOf lf:slope ;
  dcterms:identifier "http://anzsoil.org/def/au/asls/landform/slope-classes"^^xsd:anyURI ;
  skos:definition """Slope classes are defined in Table 2. The optional word ‘inclined’ is used to distinguish slope from other attributes, for example ‘gently inclined footslope’ from ‘gently undulating rises’, and ‘moderately inclined hillslope’ from ‘moderately spaced streams’.
The class boundaries given in Table 2, and repeated in Table 4, are simply boundaries separating slope terms in common use, adjusted to regular logarithmic intervals. They do not refer to observed natural clustering of slope values, since such clustering has not been shown to occur; nor do they relate precisely to boundary criteria for land use, which vary arbitrarily between organisations and which may change with advancing technology.
It may sometimes be advantageous to split each of the classes ‘very gently inclined’, ‘gently inclined’ and ‘moderately inclined’ into two levels, the appropriate boundary values being 1.8%, 5.6% and 18%.
There may also be compelling reasons for using other schemes of slope classes. However, schemes that do not have constant class widths from low to high slope values can lead to problems in subsequent statistical work."""@en ;
  skos:member lf:slope-class-CL ;
  skos:member lf:slope-class-GE ;
  skos:member lf:slope-class-LE ;
  skos:member lf:slope-class-MO ;
  skos:member lf:slope-class-PR ;
  skos:member lf:slope-class-ST ;
  skos:member lf:slope-class-VG ;
  skos:member lf:slope-class-VS ;
  skos:prefLabel "Class of slope"@en ;
.
lf:slope-class-CL
  a skos:Concept ;
  skos-ext:isMemberOf lf:slope-class ;
  dcterms:identifier "http://anzsoil.org/def/au/asls/landform/slope-class-CL"^^xsd:anyURI ;
  skos:definition "A slope tangent boundary of > 300% (72°) with average slope 500% (80°)"@en ;
  skos:inScheme asls:landform ;
  skos:notation "CL" ;
  skos:prefLabel "Cliffed"@en ;
  skos:topConceptOf asls:landform ;
.
lf:slope-class-GE
  a skos:Concept ;
  skos-ext:isMemberOf lf:slope-class ;
  dcterms:identifier "http://anzsoil.org/def/au/asls/landform/slope-class-GE"^^xsd:anyURI ;
  skos:definition "A slope tangent boundary of 3-10% (5°45') with average slope 6% (3°)"@en ;
  skos:inScheme asls:landform ;
  skos:notation "GE" ;
  skos:prefLabel "Gently inclined"@en ;
  skos:topConceptOf asls:landform ;
.
lf:slope-class-LE
  a skos:Concept ;
  skos-ext:isMemberOf lf:slope-class ;
  dcterms:identifier "http://anzsoil.org/def/au/asls/landform/slope-class-LE"^^xsd:anyURI ;
  skos:definition "A slope tangent boundary of 0-1% (0°35') with average slope 0.6% (0°20')"@en ;
  skos:inScheme asls:landform ;
  skos:notation "LE" ;
  skos:prefLabel "level"@en ;
  skos:topConceptOf asls:landform ;
.
lf:slope-class-MO
  a skos:Concept ;
  skos-ext:isMemberOf lf:slope-class ;
  dcterms:identifier "http://anzsoil.org/def/au/asls/landform/slope-class-MO"^^xsd:anyURI ;
  skos:definition "A slope tangent boundary of 10-32% (18°) with average slope 20% (10°)"@en ;
  skos:inScheme asls:landform ;
  skos:notation "MO" ;
  skos:prefLabel "Moderately inclined"@en ;
  skos:topConceptOf asls:landform ;
.
lf:slope-class-PR
  a skos:Concept ;
  skos-ext:isMemberOf lf:slope-class ;
  dcterms:identifier "http://anzsoil.org/def/au/asls/landform/slope-class-PR"^^xsd:anyURI ;
  skos:definition "A slope tangent boundary of 100-300% (72°) with average slope 170% (60°)"@en ;
  skos:inScheme asls:landform ;
  skos:notation "PR" ;
  skos:prefLabel "Precipitous"@en ;
  skos:topConceptOf asls:landform ;
.
lf:slope-class-ST
  a skos:Concept ;
  skos-ext:isMemberOf lf:slope-class ;
  dcterms:identifier "http://anzsoil.org/def/au/asls/landform/slope-class-ST"^^xsd:anyURI ;
  skos:definition "A slope tangent boundary of 32-56% (30°) with average slope 40% (23°)"@en ;
  skos:inScheme asls:landform ;
  skos:notation "ST" ;
  skos:prefLabel "Steep"@en ;
  skos:topConceptOf asls:landform ;
.
lf:slope-class-VG
  a skos:Concept ;
  skos-ext:isMemberOf lf:slope-class ;
  dcterms:identifier "http://anzsoil.org/def/au/asls/landform/slope-class-VG"^^xsd:anyURI ;
  skos:definition "A slope tangent boundary of 1-3 % (1°45') with average slope 1% (1°)"@en ;
  skos:inScheme asls:landform ;
  skos:notation "VG" ;
  skos:prefLabel "Very gently inclined"@en ;
  skos:topConceptOf asls:landform ;
.
lf:slope-class-VS
  a skos:Concept ;
  skos-ext:isMemberOf lf:slope-class ;
  dcterms:identifier "http://anzsoil.org/def/au/asls/landform/slope-class-VS"^^xsd:anyURI ;
  skos:definition "A slope tangent boundary of 56-100% (45°) with average slope 70% (37°)"@en ;
  skos:inScheme asls:landform ;
  skos:notation "VS" ;
  skos:prefLabel "Very steep"@en ;
  skos:topConceptOf asls:landform ;
.
lf:slope-evaluation-A
  a skos:Concept ;
  skos-ext:isMemberOf lf:slope-evaluations ;
  dcterms:identifier "http://anzsoil.org/def/au/asls/landform/slope-evaluation-A"^^xsd:anyURI ;
  skos:definition "Abney level or clinometer and tape"@en ;
  skos:inScheme asls:landform ;
  skos:notation "A" ;
  skos:prefLabel "Abney level or clinometer and tape"@en ;
  skos:topConceptOf asls:landform ;
.
lf:slope-evaluation-E
  a skos:Concept ;
  skos-ext:isMemberOf lf:slope-evaluations ;
  dcterms:identifier "http://anzsoil.org/def/au/asls/landform/slope-evaluation-E"^^xsd:anyURI ;
  skos:definition "Estimate"@en ;
  skos:inScheme asls:landform ;
  skos:notation "E" ;
  skos:prefLabel "Estimate"@en ;
  skos:topConceptOf asls:landform ;
.
lf:slope-evaluation-P
  a skos:Concept ;
  skos-ext:isMemberOf lf:slope-evaluations ;
  dcterms:identifier "http://anzsoil.org/def/au/asls/landform/slope-evaluation-P"^^xsd:anyURI ;
  skos:definition "Contour plan at 1:10 000 or larger scale"@en ;
  skos:inScheme asls:landform ;
  skos:notation "P" ;
  skos:prefLabel "Contour plan at 1:10 000 or larger scale"@en ;
  skos:topConceptOf asls:landform ;
.
lf:slope-evaluation-T
  a skos:Concept ;
  skos-ext:isMemberOf lf:slope-evaluations ;
  dcterms:identifier "http://anzsoil.org/def/au/asls/landform/slope-evaluation-T"^^xsd:anyURI ;
  skos:definition "Tripod-mounted instrument and staff"@en ;
  skos:inScheme asls:landform ;
  skos:notation "T" ;
  skos:prefLabel "Tripod-mounted instrument and staff"@en ;
  skos:topConceptOf asls:landform ;
.
lf:slope-evaluations
  a skos:Collection ;
  a sosa:Procedure ;
  skos-ext:isMemberOf lf:slope ;
  dcterms:identifier "http://anzsoil.org/def/au/asls/landform/slope-evaluations"^^xsd:anyURI ;
  skos:definition "Means of evaluation of slope"@en ;
  skos:member lf:slope-evaluation-A ;
  skos:member lf:slope-evaluation-E ;
  skos:member lf:slope-evaluation-P ;
  skos:member lf:slope-evaluation-T ;
  skos:prefLabel "Means of evaluation of slope"@en ;
.
lf:slope-value
  a skos:Concept ;
  a sosa:ObservableProperty ;
  skos-ext:isMemberOf lf:slope ;
  dcterms:identifier "http://anzsoil.org/def/au/asls/landform/slope-value"^^xsd:anyURI ;
  skos:definition "Express slope tangent as a percentage using up to three significant figures (e.g. 1%, 2.45%, 9%, 12.5%, 115%). Evaluate the slope over an interval of 20 m, straddling the point of soil observation. Always observe and record the slope as precisely as the chosen survey method permits. The observation should span no less than 20 m so as not to be influenced too much by features of the microrelief that occurs within the landform element."@en ;
  skos:inScheme asls:landform ;
  skos:prefLabel "Slope %"@en ;
  skos:topConceptOf asls:landform ;
.
lf:stream-channel-development
  a skos:Collection ;
  a sosa:ObservableProperty ;
  skos-ext:isMemberOf lf:stream-channel-occurence ;
  dcterms:identifier "http://anzsoil.org/def/au/asls/landform/stream-channel-development"^^xsd:anyURI ;
  skos:definition "The degree of development of stream channels."@en ;
  skos:member lf:stream-channel-development-A ;
  skos:member lf:stream-channel-development-E ;
  skos:member lf:stream-channel-development-I ;
  skos:member lf:stream-channel-development-O ;
  skos:prefLabel "Stream channel development"@en ;
.
lf:stream-channel-development-A
  a skos:Concept ;
  skos-ext:isMemberOf lf:stream-channel-development ;
  dcterms:identifier "http://anzsoil.org/def/au/asls/landform/stream-channel-development-A"^^xsd:anyURI ;
  skos:definition "continuous linear channels occur, with rather large width and depth; they are essentially constant with downstream distance and are suited to the available flow. Flood plains of vertical or lateral accretion are formed."@en ;
  skos:inScheme asls:landform ;
  skos:notation "A" ;
  skos:prefLabel "Alluvial"@en ;
  skos:topConceptOf asls:landform ;
.
lf:stream-channel-development-E
  a skos:Concept ;
  skos-ext:isMemberOf lf:stream-channel-development ;
  dcterms:identifier "http://anzsoil.org/def/au/asls/landform/stream-channel-development-E"^^xsd:anyURI ;
  skos:definition "continuous linear channels occur; their width and depth are considerable and display somewhat constant values suited to the available flow. Flood plains are not formed."@en ;
  skos:inScheme asls:landform ;
  skos:notation "E" ;
  skos:prefLabel "Erosional"@en ;
  skos:topConceptOf asls:landform ;
.
lf:stream-channel-development-I
  a skos:Concept ;
  skos-ext:isMemberOf lf:stream-channel-development ;
  dcterms:identifier "http://anzsoil.org/def/au/asls/landform/stream-channel-development-I"^^xsd:anyURI ;
  skos:definition "traces of channelled flow are very shallow, narrow and discontinuous."@en ;
  skos:inScheme asls:landform ;
  skos:notation "I" ;
  skos:prefLabel "Incipient"@en ;
  skos:topConceptOf asls:landform ;
.
lf:stream-channel-development-O
  a skos:Concept ;
  skos-ext:isMemberOf lf:stream-channel-development ;
  dcterms:identifier "http://anzsoil.org/def/au/asls/landform/stream-channel-development-O"^^xsd:anyURI ;
  skos:definition "no traces of channelled flow can be detected."@en ;
  skos:inScheme asls:landform ;
  skos:notation "O" ;
  skos:prefLabel "Absent"@en ;
  skos:topConceptOf asls:landform ;
.
lf:stream-channel-migration
  a skos:Collection ;
  a sosa:ObservableProperty ;
  skos-ext:isMemberOf lf:stream-channel-occurence ;
  dcterms:identifier "http://anzsoil.org/def/au/asls/landform/stream-channel-migration"^^xsd:anyURI ;
  skos:definition "The presence of relict channel landforms or unvegetated, newly formed channel margins or immovable channel margins may permit an assessment of channel migration."@en ;
  skos:member lf:stream-channel-migration-F ;
  skos:member lf:stream-channel-migration-R ;
  skos:member lf:stream-channel-migration-S ;
  skos:prefLabel "Stream channel migration"@en ;
.
lf:stream-channel-migration-F
  a skos:Concept ;
  skos-ext:isMemberOf lf:stream-channel-migration ;
  dcterms:identifier "http://anzsoil.org/def/au/asls/landform/stream-channel-migration-F"^^xsd:anyURI ;
  skos:definition "Fixed."@en ;
  skos:inScheme asls:landform ;
  skos:notation "F" ;
  skos:prefLabel "Fixed"@en ;
  skos:topConceptOf asls:landform ;
.
lf:stream-channel-migration-R
  a skos:Concept ;
  skos-ext:isMemberOf lf:stream-channel-migration ;
  dcterms:identifier "http://anzsoil.org/def/au/asls/landform/stream-channel-migration-R"^^xsd:anyURI ;
  skos:definition "Rapidly migrating."@en ;
  skos:inScheme asls:landform ;
  skos:notation "R" ;
  skos:prefLabel "Rapidly migrating"@en ;
  skos:topConceptOf asls:landform ;
.
lf:stream-channel-migration-S
  a skos:Concept ;
  skos-ext:isMemberOf lf:stream-channel-migration ;
  dcterms:identifier "http://anzsoil.org/def/au/asls/landform/stream-channel-migration-S"^^xsd:anyURI ;
  skos:definition "Slowly migrating."@en ;
  skos:inScheme asls:landform ;
  skos:notation "S" ;
  skos:prefLabel "Slowly migrating"@en ;
  skos:topConceptOf asls:landform ;
.
lf:stream-channel-network-directionality
  a skos:Collection ;
  a sosa:ObservableProperty ;
  skos-ext:isMemberOf lf:stream-channel-occurence ;
  dcterms:identifier "http://anzsoil.org/def/au/asls/landform/stream-channel-network-directionality"^^xsd:anyURI ;
  skos:definition "This attribute combines two simpler attributes: the degree of lineation, that is, the degree to which the channels tend to align in an organised way; and the degree of convergence or divergence of channels in the downstream direction. The latter is distinct from tributary/distributary behaviour, which refers to the combining and splitting of stream channels, rather than their directionality."@en ;
  skos:member lf:stream-channel-network-directionality-B ;
  skos:member lf:stream-channel-network-directionality-C ;
  skos:member lf:stream-channel-network-directionality-D ;
  skos:member lf:stream-channel-network-directionality-F ;
  skos:member lf:stream-channel-network-directionality-N ;
  skos:member lf:stream-channel-network-directionality-P ;
  skos:member lf:stream-channel-network-directionality-U ;
  skos:prefLabel "Stream channel network directionality"@en ;
.
lf:stream-channel-network-directionality-B
  a skos:Concept ;
  skos-ext:isMemberOf lf:stream-channel-network-directionality ;
  dcterms:identifier "http://anzsoil.org/def/au/asls/landform/stream-channel-network-directionality-B"^^xsd:anyURI ;
  skos:definition "two lineations (for example ‘trellis’)"@en ;
  skos:inScheme asls:landform ;
  skos:notation "B" ;
  skos:prefLabel "Bidirectional"@en ;
  skos:topConceptOf asls:landform ;
.
lf:stream-channel-network-directionality-C
  a skos:Concept ;
  skos-ext:isMemberOf lf:stream-channel-network-directionality ;
  dcterms:identifier "http://anzsoil.org/def/au/asls/landform/stream-channel-network-directionality-C"^^xsd:anyURI ;
  skos:definition "maximum convergence between 10º and 90º"@en ;
  skos:inScheme asls:landform ;
  skos:notation "C" ;
  skos:prefLabel "Convergent"@en ;
  skos:topConceptOf asls:landform ;
.
lf:stream-channel-network-directionality-D
  a skos:Concept ;
  skos-ext:isMemberOf lf:stream-channel-network-directionality ;
  dcterms:identifier "http://anzsoil.org/def/au/asls/landform/stream-channel-network-directionality-D"^^xsd:anyURI ;
  skos:definition "maximum divergence between 10º and 90º"@en ;
  skos:inScheme asls:landform ;
  skos:notation "D" ;
  skos:prefLabel "Divergent"@en ;
  skos:topConceptOf asls:landform ;
.
lf:stream-channel-network-directionality-F
  a skos:Concept ;
  skos-ext:isMemberOf lf:stream-channel-network-directionality ;
  dcterms:identifier "http://anzsoil.org/def/au/asls/landform/stream-channel-network-directionality-F"^^xsd:anyURI ;
  skos:definition "maximum divergence >90º"@en ;
  skos:inScheme asls:landform ;
  skos:notation "F" ;
  skos:prefLabel "Centrifugal"@en ;
  skos:topConceptOf asls:landform ;
.
lf:stream-channel-network-directionality-N
  a skos:Concept ;
  skos-ext:isMemberOf lf:stream-channel-network-directionality ;
  dcterms:identifier "http://anzsoil.org/def/au/asls/landform/stream-channel-network-directionality-N"^^xsd:anyURI ;
  skos:definition "no significant orientation, convergence or divergence"@en ;
  skos:inScheme asls:landform ;
  skos:notation "N" ;
  skos:prefLabel "Non-directional"@en ;
  skos:topConceptOf asls:landform ;
.
lf:stream-channel-network-directionality-P
  a skos:Concept ;
  skos-ext:isMemberOf lf:stream-channel-network-directionality ;
  dcterms:identifier "http://anzsoil.org/def/au/asls/landform/stream-channel-network-directionality-P"^^xsd:anyURI ;
  skos:definition "maximum convergence >90º"@en ;
  skos:inScheme asls:landform ;
  skos:notation "P" ;
  skos:prefLabel "Centripetal"@en ;
  skos:topConceptOf asls:landform ;
.
lf:stream-channel-network-directionality-U
  a skos:Concept ;
  skos-ext:isMemberOf lf:stream-channel-network-directionality ;
  dcterms:identifier "http://anzsoil.org/def/au/asls/landform/stream-channel-network-directionality-U"^^xsd:anyURI ;
  skos:definition "convergence or divergence <10º"@en ;
  skos:inScheme asls:landform ;
  skos:notation "U" ;
  skos:prefLabel "Unidirectional"@en ;
  skos:topConceptOf asls:landform ;
.
lf:stream-channel-network-integration
  a skos:Collection ;
  a sosa:ObservableProperty ;
  skos-ext:isMemberOf lf:stream-channel-occurence ;
  dcterms:identifier "http://anzsoil.org/def/au/asls/landform/stream-channel-network-integration"^^xsd:anyURI ;
  skos:definition "In an integrated channel network, one can traverse from any point on a stream channel to any other point on a stream channel without passing through any landform elements other than stream channels. The channel network may be interrupted at points where water loss into the ground or the atmosphere is sufficiently large, and in the extreme case, typical of karst terrain, the surface stream network is disintegrated. Classes of channel network integration are:"@en ;
  skos:member lf:stream-channel-network-integration-D ;
  skos:member lf:stream-channel-network-integration-I ;
  skos:member lf:stream-channel-network-integration-P ;
  skos:prefLabel "Stream channel network integration"@en ;
.
lf:stream-channel-network-integration-D
  a skos:Concept ;
  skos-ext:isMemberOf lf:stream-channel-network-integration ;
  dcterms:identifier "http://anzsoil.org/def/au/asls/landform/stream-channel-network-integration-D"^^xsd:anyURI ;
  skos:definition "Disintegrated"@en ;
  skos:inScheme asls:landform ;
  skos:notation "D" ;
  skos:prefLabel "Disintegrated"@en ;
  skos:topConceptOf asls:landform ;
.
lf:stream-channel-network-integration-I
  a skos:Concept ;
  skos-ext:isMemberOf lf:stream-channel-network-integration ;
  dcterms:identifier "http://anzsoil.org/def/au/asls/landform/stream-channel-network-integration-I"^^xsd:anyURI ;
  skos:definition "Integrated"@en ;
  skos:inScheme asls:landform ;
  skos:notation "I" ;
  skos:prefLabel "Integrated"@en ;
  skos:topConceptOf asls:landform ;
.
lf:stream-channel-network-integration-P
  a skos:Concept ;
  skos-ext:isMemberOf lf:stream-channel-network-integration ;
  dcterms:identifier "http://anzsoil.org/def/au/asls/landform/stream-channel-network-integration-P"^^xsd:anyURI ;
  skos:definition "Interrupted (partial integration)"@en ;
  skos:inScheme asls:landform ;
  skos:notation "P" ;
  skos:prefLabel "Interrupted (partial integration)"@en ;
  skos:topConceptOf asls:landform ;
.
lf:stream-channel-occurence
  a skos:Collection ;
  a sosa:ObservableProperty ;
  dcterms:identifier "http://anzsoil.org/def/au/asls/landform/stream-channel-occurence"^^xsd:anyURI ;
  skos:definition """A number of attributes describing the occurrence and pattern of surface stream channels have diagnostic value. Use of the following attributes may clarify the observable differences between landform patterns, particularly in plains where mapping criteria are elusive.
When assessing attributes of stream channel occurrence, it is easy to make errors by not setting limits to the area to be described. Tentative landform pattern boundaries must be drawn to clarify these limits. Major stream channels are best mapped as wholly within one landform pattern or another, rather than marking a boundary."""@en ;
  skos:member lf:stream-channel-development ;
  skos:member lf:stream-channel-migration ;
  skos:member lf:stream-channel-network-directionality ;
  skos:member lf:stream-channel-network-integration ;
  skos:member lf:stream-channel-relative-depth-width ;
  skos:member lf:stream-channel-spacing ;
  skos:member lf:streamwise-channel-pattern ;
  skos:prefLabel "Stream channel occurence"@en ;
.
lf:stream-channel-relative-depth-width
  a skos:Collection ;
  a sosa:ObservableProperty ;
  skos-ext:isMemberOf lf:stream-channel-occurence ;
  dcterms:identifier "http://anzsoil.org/def/au/asls/landform/stream-channel-relative-depth-width"^^xsd:anyURI ;
  skos:definition """Channel depth and width refer to the dimensions of a landform that is dominated by channelled stream flow. The limit of channelled stream flow dominance must be identified before width or depth can be estimated. Depth is taken from the top of the stream bank down to the average height of the line following the deepest part of the channel.
The distinction between stream bank and hillslope or scarp according to dominant process requires particular care where streams are incised, especially if they are cut into terraces that could be mistaken for flood plains.
 
For detailed studies, keep records of width and depth measurements. In other surveys, use the following classes of relative depth."""@en ;
  skos:member lf:stream-channel-relative-depth-width-D ;
  skos:member lf:stream-channel-relative-depth-width-M ;
  skos:member lf:stream-channel-relative-depth-width-S ;
  skos:member lf:stream-channel-relative-depth-width-V ;
  skos:prefLabel "Stream channel depth relative to width"@en ;
.
lf:stream-channel-relative-depth-width-D
  a skos:Concept ;
  skos-ext:isMemberOf lf:stream-channel-relative-depth-width ;
  dcterms:identifier "http://anzsoil.org/def/au/asls/landform/stream-channel-relative-depth-width-D"^^xsd:anyURI ;
  skos:definition "width/depth ratio <20:1"@en ;
  skos:inScheme asls:landform ;
  skos:notation "D" ;
  skos:prefLabel "Deep"@en ;
  skos:topConceptOf asls:landform ;
.
lf:stream-channel-relative-depth-width-M
  a skos:Concept ;
  skos-ext:isMemberOf lf:stream-channel-relative-depth-width ;
  dcterms:identifier "http://anzsoil.org/def/au/asls/landform/stream-channel-relative-depth-width-M"^^xsd:anyURI ;
  skos:definition "width/depth ratio 20:1 to 50:1"@en ;
  skos:inScheme asls:landform ;
  skos:notation "M" ;
  skos:prefLabel "Moderately deep"@en ;
  skos:topConceptOf asls:landform ;
.
lf:stream-channel-relative-depth-width-S
  a skos:Concept ;
  skos-ext:isMemberOf lf:stream-channel-relative-depth-width ;
  dcterms:identifier "http://anzsoil.org/def/au/asls/landform/stream-channel-relative-depth-width-S"^^xsd:anyURI ;
  skos:definition "width/depth ratio 50:1 to 150:1"@en ;
  skos:inScheme asls:landform ;
  skos:notation "S" ;
  skos:prefLabel "Shallow"@en ;
  skos:topConceptOf asls:landform ;
.
lf:stream-channel-relative-depth-width-V
  a skos:Concept ;
  skos-ext:isMemberOf lf:stream-channel-relative-depth-width ;
  dcterms:identifier "http://anzsoil.org/def/au/asls/landform/stream-channel-relative-depth-width-V"^^xsd:anyURI ;
  skos:definition "width/depth ratio >150:1"@en ;
  skos:inScheme asls:landform ;
  skos:notation "V" ;
  skos:prefLabel "Very shallow"@en ;
  skos:topConceptOf asls:landform ;
.
lf:stream-channel-spacing
  a skos:Collection ;
  a sosa:ObservableProperty ;
  skos-ext:isMemberOf lf:stream-channel-occurence ;
  dcterms:identifier "http://anzsoil.org/def/au/asls/landform/stream-channel-spacing"^^xsd:anyURI ;
  skos:definition """The average spacing of stream channels, L/N, is determined by counting the number, N, of their intersections with an arbitrary line of length L.*
A convenient tool for estimating channel spacing is a circle, with a circumference of 2 km at map or photo scale, drawn on transparent material."""@en ;
  skos:member lf:stream-channel-spacing-AB ;
  skos:member lf:stream-channel-spacing-CS ;
  skos:member lf:stream-channel-spacing-MS ;
  skos:member lf:stream-channel-spacing-NU ;
  skos:member lf:stream-channel-spacing-SP ;
  skos:member lf:stream-channel-spacing-VC ;
  skos:member lf:stream-channel-spacing-VW ;
  skos:member lf:stream-channel-spacing-WS ;
  skos:prefLabel "Stream channel spacing"@en ;
.
lf:stream-channel-spacing-AB
  a skos:Concept ;
  skos-ext:isMemberOf lf:stream-channel-spacing ;
  dcterms:identifier "http://anzsoil.org/def/au/asls/landform/stream-channel-spacing-AB"^^xsd:anyURI ;
  skos:definition ">2500 m"@en ;
  skos:inScheme asls:landform ;
  skos:notation "AB" ;
  skos:prefLabel "Absent or very rare"@en ;
  skos:topConceptOf asls:landform ;
.
lf:stream-channel-spacing-CS
  a skos:Concept ;
  skos-ext:isMemberOf lf:stream-channel-spacing ;
  dcterms:identifier "http://anzsoil.org/def/au/asls/landform/stream-channel-spacing-CS"^^xsd:anyURI ;
  skos:definition "250-400 m"@en ;
  skos:inScheme asls:landform ;
  skos:notation "CS" ;
  skos:prefLabel "Closely spaced"@en ;
  skos:topConceptOf asls:landform ;
.
lf:stream-channel-spacing-MS
  a skos:Concept ;
  skos-ext:isMemberOf lf:stream-channel-spacing ;
  dcterms:identifier "http://anzsoil.org/def/au/asls/landform/stream-channel-spacing-MS"^^xsd:anyURI ;
  skos:definition "400-625 m"@en ;
  skos:inScheme asls:landform ;
  skos:notation "MS" ;
  skos:prefLabel "Moderately spaced"@en ;
  skos:topConceptOf asls:landform ;
.
lf:stream-channel-spacing-NU
  a skos:Concept ;
  skos-ext:isMemberOf lf:stream-channel-spacing ;
  dcterms:identifier "http://anzsoil.org/def/au/asls/landform/stream-channel-spacing-NU"^^xsd:anyURI ;
  skos:definition "<158 m"@en ;
  skos:inScheme asls:landform ;
  skos:notation "NU" ;
  skos:prefLabel "Numerous"@en ;
  skos:topConceptOf asls:landform ;
.
lf:stream-channel-spacing-SP
  a skos:Concept ;
  skos-ext:isMemberOf lf:stream-channel-spacing ;
  dcterms:identifier "http://anzsoil.org/def/au/asls/landform/stream-channel-spacing-SP"^^xsd:anyURI ;
  skos:definition "1585-2500 m"@en ;
  skos:inScheme asls:landform ;
  skos:notation "SP" ;
  skos:prefLabel "Sparse"@en ;
  skos:topConceptOf asls:landform ;
.
lf:stream-channel-spacing-VC
  a skos:Concept ;
  skos-ext:isMemberOf lf:stream-channel-spacing ;
  dcterms:identifier "http://anzsoil.org/def/au/asls/landform/stream-channel-spacing-VC"^^xsd:anyURI ;
  skos:definition "158-250 m"@en ;
  skos:inScheme asls:landform ;
  skos:notation "VC" ;
  skos:prefLabel "Very closely spaced"@en ;
  skos:topConceptOf asls:landform ;
.
lf:stream-channel-spacing-VW
  a skos:Concept ;
  skos-ext:isMemberOf lf:stream-channel-spacing ;
  dcterms:identifier "http://anzsoil.org/def/au/asls/landform/stream-channel-spacing-VW"^^xsd:anyURI ;
  skos:definition "1000 - 1585 m"@en ;
  skos:inScheme asls:landform ;
  skos:notation "VW" ;
  skos:prefLabel "Very widely spaced"@en ;
  skos:topConceptOf asls:landform ;
.
lf:stream-channel-spacing-WS
  a skos:Concept ;
  skos-ext:isMemberOf lf:stream-channel-spacing ;
  dcterms:identifier "http://anzsoil.org/def/au/asls/landform/stream-channel-spacing-WS"^^xsd:anyURI ;
  skos:definition "625-1000 m"@en ;
  skos:inScheme asls:landform ;
  skos:notation "WS" ;
  skos:prefLabel "Widely spaced"@en ;
  skos:topConceptOf asls:landform ;
.
lf:streamwise-channel-pattern
  a skos:Collection ;
  a sosa:ObservableProperty ;
  skos-ext:isMemberOf lf:stream-channel-occurence ;
  dcterms:identifier "http://anzsoil.org/def/au/asls/landform/streamwise-channel-pattern"^^xsd:anyURI ;
  skos:definition "In a traverse downstream, it may happen that tributaries enter the stream at frequent intervals, or that the stream splits into distributaries, or that these tendencies are absent (the non-tributary case) or are in balance with each other (the braided or anastomotic case called here reticulated) giving four classes of stream-wise channel pattern."@en ;
  skos:member lf:streamwise-channel-pattern-D ;
  skos:member lf:streamwise-channel-pattern-N ;
  skos:member lf:streamwise-channel-pattern-R ;
  skos:member lf:streamwise-channel-pattern-T ;
  skos:prefLabel "Stream-wise channel pattern"@en ;
.
lf:streamwise-channel-pattern-D
  a skos:Concept ;
  skos-ext:isMemberOf lf:streamwise-channel-pattern ;
  dcterms:identifier "http://anzsoil.org/def/au/asls/landform/streamwise-channel-pattern-D"^^xsd:anyURI ;
  skos:definition "Distributary"@en ;
  skos:inScheme asls:landform ;
  skos:notation "D" ;
  skos:prefLabel "Distributary"@en ;
  skos:topConceptOf asls:landform ;
.
lf:streamwise-channel-pattern-N
  a skos:Concept ;
  skos-ext:isMemberOf lf:streamwise-channel-pattern ;
  dcterms:identifier "http://anzsoil.org/def/au/asls/landform/streamwise-channel-pattern-N"^^xsd:anyURI ;
  skos:definition "Non-tributary"@en ;
  skos:inScheme asls:landform ;
  skos:notation "N" ;
  skos:prefLabel "Non-tributary"@en ;
  skos:topConceptOf asls:landform ;
.
lf:streamwise-channel-pattern-R
  a skos:Concept ;
  skos-ext:isMemberOf lf:streamwise-channel-pattern ;
  dcterms:identifier "http://anzsoil.org/def/au/asls/landform/streamwise-channel-pattern-R"^^xsd:anyURI ;
  skos:definition "Reticulated"@en ;
  skos:inScheme asls:landform ;
  skos:notation "R" ;
  skos:prefLabel "Reticulated"@en ;
  skos:topConceptOf asls:landform ;
.
lf:streamwise-channel-pattern-T
  a skos:Concept ;
  skos-ext:isMemberOf lf:streamwise-channel-pattern ;
  dcterms:identifier "http://anzsoil.org/def/au/asls/landform/streamwise-channel-pattern-T"^^xsd:anyURI ;
  skos:definition "Tributary"@en ;
  skos:inScheme asls:landform ;
  skos:notation "T" ;
  skos:prefLabel "Tributary"@en ;
  skos:topConceptOf asls:landform ;
.
skos-ext:isMemberOf
  a owl:ObjectProperty ;
  rdfs:domain [
      a owl:Class ;
      owl:unionOf (
          skos:Collection
          skos:Concept
        ) ;
    ] ;
  rdfs:label "is member of collection" ;
  rdfs:range skos:Collection ;
  rdfs:subPropertyOf skos-ext:relatedCollection ;
.
skos-ext:relatedCollection
  a owl:ObjectProperty ;
  rdfs:domain [
      a owl:Class ;
      owl:unionOf (
          skos:Concept
          skos:Collection
        ) ;
    ] ;
  rdfs:label "is related to collection" ;
  rdfs:range skos:Collection ;
  rdfs:subPropertyOf dcterms:relation ;
.
skos-ext:topMemberOf
  a owl:ObjectProperty ;
  rdfs:domain [
      a owl:Class ;
      owl:unionOf (
          skos:Collection
          skos:Concept
        ) ;
    ] ;
  rdfs:label "is top member of collection" ;
  rdfs:range skos:Collection ;
  rdfs:subPropertyOf skos-ext:isMemberOf ;
.
reg:statusAccepted
  dcterms:identifier "http://purl.org/linked-data/registry#statusAccepted"^^xsd:anyURI ;
.
reg:statusDeprecated
  dcterms:identifier "http://purl.org/linked-data/registry#statusDeprecated"^^xsd:anyURI ;
.
reg:statusExperimental
  dcterms:identifier "http://purl.org/linked-data/registry#statusExperimental"^^xsd:anyURI ;
.
reg:statusInvalid
  dcterms:identifier "http://purl.org/linked-data/registry#statusInvalid"^^xsd:anyURI ;
.
reg:statusNotAccepted
  dcterms:identifier "http://purl.org/linked-data/registry#statusNotAccepted"^^xsd:anyURI ;
.
reg:statusReserved
  dcterms:identifier "http://purl.org/linked-data/registry#statusReserved"^^xsd:anyURI ;
.
reg:statusRetired
  dcterms:identifier "http://purl.org/linked-data/registry#statusRetired"^^xsd:anyURI ;
.
reg:statusStable
  dcterms:identifier "http://purl.org/linked-data/registry#statusStable"^^xsd:anyURI ;
.
reg:statusSubmitted
  dcterms:identifier "http://purl.org/linked-data/registry#statusSubmitted"^^xsd:anyURI ;
.
reg:statusSuperseded
  dcterms:identifier "http://purl.org/linked-data/registry#statusSuperseded"^^xsd:anyURI ;
.
reg:statusValid
  dcterms:identifier "http://purl.org/linked-data/registry#statusValid"^^xsd:anyURI ;
.
skos:member
  owl:inverseOf skos-ext:isMemberOf ;
.
skos:semanticRelation
  rdfs:subPropertyOf dcterms:relation ;
.
