@prefix dct: <http://purl.org/dc/terms/> .
@prefix owl: <http://www.w3.org/2002/07/owl#> .
@prefix rdf: <http://www.w3.org/1999/02/22-rdf-syntax-ns#> .
@prefix rdfs: <http://www.w3.org/2000/01/rdf-schema#> .
@prefix skos: <http://www.w3.org/2004/02/skos/core#> .
@prefix ui: <http://purl.org/linked-data/registry-ui#> .
@prefix xml: <http://www.w3.org/XML/1998/namespace> .
@prefix xsd: <http://www.w3.org/2001/XMLSchema#> .

<landform-element-ALC> a skos:Concept ;
    rdfs:label "Alcove"@en ;
    dct:description "Moderately inclined to very steep, short open depression with concave cross-section, eroded by collapse, landslides, creep or surface wash."@en ;
    dct:identifier "http://anzsoil.org/def/au/asls/landform/landform-element-ALC"^^xsd:anyURI ;
    ui:isMemberOf <landform-element> ;
    owl:sameAs <http://anzsoil.org/def/au/asls/landform/landform-element-ALC> ;
    skos:definition "Moderately inclined to very steep, short open depression with concave cross-section, eroded by collapse, landslides, creep or surface wash."@en ;
    skos:notation "ALC"@en ;
    skos:prefLabel "Alcove"@en .

<landform-element-BAN> a skos:Concept ;
    rdfs:label "Bank (stream bank)"@en ;
    dct:description "Very short, very wide slope, moderately inclined to precipitous, forming the marginal upper parts of a stream channel and resulting from erosion or aggradation by channelled stream flow."@en ;
    dct:identifier "http://anzsoil.org/def/au/asls/landform/landform-element-BAN"^^xsd:anyURI ;
    ui:isMemberOf <landform-element> ;
    owl:sameAs <http://anzsoil.org/def/au/asls/landform/landform-element-BAN> ;
    skos:definition "Very short, very wide slope, moderately inclined to precipitous, forming the marginal upper parts of a stream channel and resulting from erosion or aggradation by channelled stream flow."@en ;
    skos:notation "BAN"@en ;
    skos:prefLabel "Bank (stream bank)"@en .

<landform-element-BAR> a skos:Concept ;
    rdfs:label "Bar (stream bar)"@en ;
    dct:description "Elongated, gently to moderately inclined, low ridge built up by channelled stream flow, part of a stream bed."@en ;
    dct:identifier "http://anzsoil.org/def/au/asls/landform/landform-element-BAR"^^xsd:anyURI ;
    ui:isMemberOf <landform-element> ;
    owl:sameAs <http://anzsoil.org/def/au/asls/landform/landform-element-BAR> ;
    skos:definition "Elongated, gently to moderately inclined, low ridge built up by channelled stream flow, part of a stream bed."@en ;
    skos:notation "BAR"@en ;
    skos:prefLabel "Bar (stream bar)"@en .

<landform-element-BEA> a skos:Concept ;
    rdfs:label "Beach"@en ;
    dct:description "Short, low, very wide slope, gently or moderately inclined, built up or eroded by waves, forming the shore of a lake or sea."@en ;
    dct:identifier "http://anzsoil.org/def/au/asls/landform/landform-element-BEA"^^xsd:anyURI ;
    ui:isMemberOf <landform-element> ;
    owl:sameAs <http://anzsoil.org/def/au/asls/landform/landform-element-BEA> ;
    skos:definition "Short, low, very wide slope, gently or moderately inclined, built up or eroded by waves, forming the shore of a lake or sea."@en ;
    skos:notation "BEA"@en ;
    skos:prefLabel "Beach"@en .

<landform-element-BEN> a skos:Concept ;
    rdfs:label "Bench"@en ;
    dct:description "Short, gently or very gently inclined minimal mid-slope element eroded or aggraded by any agent."@en ;
    dct:identifier "http://anzsoil.org/def/au/asls/landform/landform-element-BEN"^^xsd:anyURI ;
    ui:isMemberOf <landform-element> ;
    owl:sameAs <http://anzsoil.org/def/au/asls/landform/landform-element-BEN> ;
    skos:definition "Short, gently or very gently inclined minimal mid-slope element eroded or aggraded by any agent."@en ;
    skos:notation "BEN"@en ;
    skos:prefLabel "Bench"@en .

<landform-element-BER> a skos:Concept ;
    rdfs:label "Berm"@en ;
    dct:description "(i) Short, very gently inclined to level minimal mid-slope in an embankment or cut face, eroded or aggraded by human activity. (ii) Flat built up by waves above a beach."@en ;
    dct:identifier "http://anzsoil.org/def/au/asls/landform/landform-element-BER"^^xsd:anyURI ;
    ui:isMemberOf <landform-element> ;
    owl:sameAs <http://anzsoil.org/def/au/asls/landform/landform-element-BER> ;
    skos:definition "(i) Short, very gently inclined to level minimal mid-slope in an embankment or cut face, eroded or aggraded by human activity. (ii) Flat built up by waves above a beach."@en ;
    skos:notation "BER"@en ;
    skos:prefLabel "Berm"@en .

<landform-element-BKP> a skos:Concept ;
    rdfs:label "Backplain"@en ;
    dct:description "Large flat resulting from aggradation by overbank stream flow at some distance from the stream channel and in some cases biological (peat) accumulation, often characterised by a high watertable and the presence of swamps or lakes, part of a covered plain landform pattern."@en ;
    dct:identifier "http://anzsoil.org/def/au/asls/landform/landform-element-BKP"^^xsd:anyURI ;
    ui:isMemberOf <landform-element> ;
    owl:sameAs <http://anzsoil.org/def/au/asls/landform/landform-element-BKP> ;
    skos:definition "Large flat resulting from aggradation by overbank stream flow at some distance from the stream channel and in some cases biological (peat) accumulation, often characterised by a high watertable and the presence of swamps or lakes, part of a covered plain landform pattern."@en ;
    skos:notation "BKP"@en ;
    skos:prefLabel "Backplain"@en .

<landform-element-BOU> a skos:Concept ;
    rdfs:label "Blow-out"@en ;
    dct:description "Usually small, open or closed depression excavated by the wind."@en ;
    dct:identifier "http://anzsoil.org/def/au/asls/landform/landform-element-BOU"^^xsd:anyURI ;
    ui:isMemberOf <landform-element> ;
    owl:sameAs <http://anzsoil.org/def/au/asls/landform/landform-element-BOU> ;
    skos:definition "Usually small, open or closed depression excavated by the wind."@en ;
    skos:notation "BOU"@en ;
    skos:prefLabel "Blow-out"@en .

<landform-element-BRI> a skos:Concept ;
    rdfs:label "Beach ridge"@en ;
    dct:description "Very long, nearly straight, low ridge, built up by waves and usually modified by wind. A beach ridge is often a relict feature remote from the beach."@en ;
    dct:identifier "http://anzsoil.org/def/au/asls/landform/landform-element-BRI"^^xsd:anyURI ;
    ui:isMemberOf <landform-element> ;
    owl:sameAs <http://anzsoil.org/def/au/asls/landform/landform-element-BRI> ;
    skos:definition "Very long, nearly straight, low ridge, built up by waves and usually modified by wind. A beach ridge is often a relict feature remote from the beach."@en ;
    skos:notation "BRI"@en ;
    skos:prefLabel "Beach ridge"@en .

<landform-element-BRK> a skos:Concept ;
    rdfs:label "Breakaway"@en ;
    dct:description "Steep maximal mid-slope or upper slope, generally comprising both a very short scarp (free face) that is often bare rockland, and a stony scarp-footslope (debris slope), often standing above a pediment."@en ;
    dct:identifier "http://anzsoil.org/def/au/asls/landform/landform-element-BRK"^^xsd:anyURI ;
    ui:isMemberOf <landform-element> ;
    owl:sameAs <http://anzsoil.org/def/au/asls/landform/landform-element-BRK> ;
    skos:definition "Steep maximal mid-slope or upper slope, generally comprising both a very short scarp (free face) that is often bare rockland, and a stony scarp-footslope (debris slope), often standing above a pediment."@en ;
    skos:notation "BRK"@en ;
    skos:prefLabel "Breakaway"@en .

<landform-element-CBE> a skos:Concept ;
    rdfs:label "Channel bench"@en ;
    dct:description "Flat at the margin of a stream channel aggraded and partly eroded by overbank and channelled stream flow, an incipient flood plain. Channel benches have been referred to as 'low terraces', but the term 'terrace' should be restricted to landform patterns above the influence of active stream flow."@en ;
    dct:identifier "http://anzsoil.org/def/au/asls/landform/landform-element-CBE"^^xsd:anyURI ;
    ui:isMemberOf <landform-element> ;
    owl:sameAs <http://anzsoil.org/def/au/asls/landform/landform-element-CBE> ;
    skos:definition "Flat at the margin of a stream channel aggraded and partly eroded by overbank and channelled stream flow, an incipient flood plain. Channel benches have been referred to as 'low terraces', but the term 'terrace' should be restricted to landform patterns above the influence of active stream flow."@en ;
    skos:notation "CBE"@en ;
    skos:prefLabel "Channel bench"@en .

<landform-element-CFS> a skos:Concept ;
    rdfs:label "Cliff-footslope"@en ;
    dct:description "Slope situated below a cliff, with its contours generally parallel to the line of the cliff eroded by sheet wash or water-aided mass movement, and aggraded locally by collapsed material from above."@en ;
    dct:identifier "http://anzsoil.org/def/au/asls/landform/landform-element-CFS"^^xsd:anyURI ;
    ui:isMemberOf <landform-element> ;
    owl:sameAs <http://anzsoil.org/def/au/asls/landform/landform-element-CFS> ;
    skos:definition "Slope situated below a cliff, with its contours generally parallel to the line of the cliff eroded by sheet wash or water-aided mass movement, and aggraded locally by collapsed material from above."@en ;
    skos:notation "CFS"@en ;
    skos:prefLabel "Cliff-footslope"@en .

<landform-element-CIR> a skos:Concept ;
    rdfs:label "Cirque"@en ;
    dct:description "Precipitous to gently inclined, typically closed depression of concave contour and profile excavated by ice. The closed part of the depression may be shallow, the larger part being an open depression like an alcove."@en ;
    dct:identifier "http://anzsoil.org/def/au/asls/landform/landform-element-CIR"^^xsd:anyURI ;
    ui:isMemberOf <landform-element> ;
    owl:sameAs <http://anzsoil.org/def/au/asls/landform/landform-element-CIR> ;
    skos:definition "Precipitous to gently inclined, typically closed depression of concave contour and profile excavated by ice. The closed part of the depression may be shallow, the larger part being an open depression like an alcove."@en ;
    skos:notation "CIR"@en ;
    skos:prefLabel "Cirque"@en .

<landform-element-CLI> a skos:Concept ;
    rdfs:label "Cliff"@en ;
    dct:description "Very wide, cliffed (greater than 72 degrees) maximal slope usually eroded by gravitational fall as a result of erosion of the base by various agencies, sometimes built up by marine organisms."@en ;
    dct:identifier "http://anzsoil.org/def/au/asls/landform/landform-element-CLI"^^xsd:anyURI ;
    ui:isMemberOf <landform-element> ;
    owl:sameAs <http://anzsoil.org/def/au/asls/landform/landform-element-CLI> ;
    skos:definition "Very wide, cliffed (greater than 72 degrees) maximal slope usually eroded by gravitational fall as a result of erosion of the base by various agencies, sometimes built up by marine organisms."@en ;
    skos:notation "CLI"@en ;
    skos:prefLabel "Cliff"@en .

<landform-element-CON> a skos:Concept ;
    rdfs:label "Cone (volcanic)"@en ;
    dct:description "Hillock with a circular symmetry built up by volcanism. The crest may form a ring around a crater."@en ;
    dct:identifier "http://anzsoil.org/def/au/asls/landform/landform-element-CON"^^xsd:anyURI ;
    ui:isMemberOf <landform-element> ;
    owl:sameAs <http://anzsoil.org/def/au/asls/landform/landform-element-CON> ;
    skos:definition "Hillock with a circular symmetry built up by volcanism. The crest may form a ring around a crater."@en ;
    skos:notation "CON"@en ;
    skos:prefLabel "Cone (volcanic)"@en .

<landform-element-COS> a skos:Concept ;
    rdfs:label "Cut-over surface"@en ;
    dct:description "Flat eroded by human activity."@en ;
    dct:identifier "http://anzsoil.org/def/au/asls/landform/landform-element-COS"^^xsd:anyURI ;
    ui:isMemberOf <landform-element> ;
    owl:sameAs <http://anzsoil.org/def/au/asls/landform/landform-element-COS> ;
    skos:definition "Flat eroded by human activity."@en ;
    skos:notation "COS"@en ;
    skos:prefLabel "Cut-over surface"@en .

<landform-element-CRA> a skos:Concept ;
    rdfs:label "Crater"@en ;
    dct:description "Steep to precipitous closed depression excavated by explosions due to volcanism, human action, or impact of an extraterrestrial object."@en ;
    dct:identifier "http://anzsoil.org/def/au/asls/landform/landform-element-CRA"^^xsd:anyURI ;
    ui:isMemberOf <landform-element> ;
    owl:sameAs <http://anzsoil.org/def/au/asls/landform/landform-element-CRA> ;
    skos:definition "Steep to precipitous closed depression excavated by explosions due to volcanism, human action, or impact of an extraterrestrial object."@en ;
    skos:notation "CRA"@en ;
    skos:prefLabel "Crater"@en .

<landform-element-CUT> a skos:Concept ;
    rdfs:label "Cut face"@en ;
    dct:description "Slope eroded by human activity."@en ;
    dct:identifier "http://anzsoil.org/def/au/asls/landform/landform-element-CUT"^^xsd:anyURI ;
    ui:isMemberOf <landform-element> ;
    owl:sameAs <http://anzsoil.org/def/au/asls/landform/landform-element-CUT> ;
    skos:definition "Slope eroded by human activity."@en ;
    skos:notation "CUT"@en ;
    skos:prefLabel "Cut face"@en .

<landform-element-DAM> a skos:Concept ;
    rdfs:label "Dam"@en ;
    dct:description "Ridge built up by human activity so as to close a depression."@en ;
    dct:identifier "http://anzsoil.org/def/au/asls/landform/landform-element-DAM"^^xsd:anyURI ;
    ui:isMemberOf <landform-element> ;
    owl:sameAs <http://anzsoil.org/def/au/asls/landform/landform-element-DAM> ;
    skos:definition "Ridge built up by human activity so as to close a depression."@en ;
    skos:notation "DAM"@en ;
    skos:prefLabel "Dam"@en .

<landform-element-DBA> a skos:Concept ;
    rdfs:label "Deflation basin"@en ;
    dct:description "Basin excavated by wind erosion which removes loose material, commonly above a resistant or wet layer."@en ;
    dct:identifier "http://anzsoil.org/def/au/asls/landform/landform-element-DBA"^^xsd:anyURI ;
    ui:isMemberOf <landform-element> ;
    owl:sameAs <http://anzsoil.org/def/au/asls/landform/landform-element-DBA> ;
    skos:definition "Basin excavated by wind erosion which removes loose material, commonly above a resistant or wet layer."@en ;
    skos:notation "DBA"@en ;
    skos:prefLabel "Deflation basin"@en .

<landform-element-DDE> a skos:Concept ;
    rdfs:label "Drainage depression"@en ;
    dct:description "Level to gently inclined, long, narrow shallow open depression with smoothly concave cross-section rising to moderately inclined side slopes, eroded or aggraded by sheet wash."@en ;
    dct:identifier "http://anzsoil.org/def/au/asls/landform/landform-element-DDE"^^xsd:anyURI ;
    ui:isMemberOf <landform-element> ;
    owl:sameAs <http://anzsoil.org/def/au/asls/landform/landform-element-DDE> ;
    skos:definition "Level to gently inclined, long, narrow shallow open depression with smoothly concave cross-section rising to moderately inclined side slopes, eroded or aggraded by sheet wash."@en ;
    skos:notation "DDE"@en ;
    skos:prefLabel "Drainage depression"@en .

<landform-element-DOC> a skos:Concept ;
    rdfs:label "Collapse doline"@en ;
    dct:description "Steep-sided, circular or elliptical closed depression, commonly funnel-shaped, characterised by subsurface drainage and formed by collapse of underlying caves within bedrock."@en ;
    dct:identifier "http://anzsoil.org/def/au/asls/landform/landform-element-DOC"^^xsd:anyURI ;
    ui:isMemberOf <landform-element> ;
    owl:sameAs <http://anzsoil.org/def/au/asls/landform/landform-element-DOC> ;
    skos:definition "Steep-sided, circular or elliptical closed depression, commonly funnel-shaped, characterised by subsurface drainage and formed by collapse of underlying caves within bedrock."@en ;
    skos:notation "DOC"@en ;
    skos:prefLabel "Collapse doline"@en .

<landform-element-DOL> a skos:Concept ;
    rdfs:label "Solution doline"@en ;
    dct:description "Steep-sided, circular or elliptical closed depression, commonly funnel-shaped, characterised by subsurface drainage and formed by dissolution of the surface or underlying within bedrock."@en ;
    dct:identifier "http://anzsoil.org/def/au/asls/landform/landform-element-DOL"^^xsd:anyURI ;
    ui:isMemberOf <landform-element> ;
    owl:sameAs <http://anzsoil.org/def/au/asls/landform/landform-element-DOL> ;
    skos:definition "Steep-sided, circular or elliptical closed depression, commonly funnel-shaped, characterised by subsurface drainage and formed by dissolution of the surface or underlying within bedrock."@en ;
    skos:notation "DOL"@en ;
    skos:prefLabel "Solution doline"@en .

<landform-element-DUB> a skos:Concept ;
    rdfs:label "Barchan dune"@en ;
    dct:description "Crescent shaped dune with tips extending leeward (downwind), making this side concave and the windward (upwind) side convex. Barchan dunes tend to be arranged in chains extending in the dominant wind direction."@en ;
    dct:identifier "http://anzsoil.org/def/au/asls/landform/landform-element-DUB"^^xsd:anyURI ;
    ui:isMemberOf <landform-element> ;
    owl:sameAs <http://anzsoil.org/def/au/asls/landform/landform-element-DUB> ;
    skos:definition "Crescent shaped dune with tips extending leeward (downwind), making this side concave and the windward (upwind) side convex. Barchan dunes tend to be arranged in chains extending in the dominant wind direction."@en ;
    skos:notation "DUB"@en ;
    skos:prefLabel "Barchan dune"@en .

<landform-element-DUC> a skos:Concept ;
    rdfs:label "Dune crest"@en ;
    dct:description "Crest built up or eroded by the wind (see Dune)."@en ;
    dct:identifier "http://anzsoil.org/def/au/asls/landform/landform-element-DUC"^^xsd:anyURI ;
    ui:isMemberOf <landform-element> ;
    owl:sameAs <http://anzsoil.org/def/au/asls/landform/landform-element-DUC> ;
    skos:definition "Crest built up or eroded by the wind (see Dune)."@en ;
    skos:notation "DUC"@en ;
    skos:prefLabel "Dune crest"@en .

<landform-element-DUF> a skos:Concept ;
    rdfs:label "Linear or longitudinal (seif) dune"@en ;
    dct:description "Large, sharp-crested, elongated, longitudinal (linear) dune or chain of sand dunes, oriented parallel, rather than transverse (perpendicular), to the prevailing wind. Not to be confused with the trailing arms of parabolic dunes."@en ;
    dct:identifier "http://anzsoil.org/def/au/asls/landform/landform-element-DUF"^^xsd:anyURI ;
    ui:isMemberOf <landform-element> ;
    owl:sameAs <http://anzsoil.org/def/au/asls/landform/landform-element-DUF> ;
    skos:definition "Large, sharp-crested, elongated, longitudinal (linear) dune or chain of sand dunes, oriented parallel, rather than transverse (perpendicular), to the prevailing wind. Not to be confused with the trailing arms of parabolic dunes."@en ;
    skos:notation "DUF"@en ;
    skos:prefLabel "Linear or longitudinal (seif) dune"@en .

<landform-element-DUH> a skos:Concept ;
    rdfs:label "Hummocky (weakly oriented dune)"@en ;
    dct:description "Very gently to moderately inclined rises or hillocks built up or eroded by wind and lacking distinct orientation or regular pattern."@en ;
    dct:identifier "http://anzsoil.org/def/au/asls/landform/landform-element-DUH"^^xsd:anyURI ;
    ui:isMemberOf <landform-element> ;
    owl:sameAs <http://anzsoil.org/def/au/asls/landform/landform-element-DUH> ;
    skos:definition "Very gently to moderately inclined rises or hillocks built up or eroded by wind and lacking distinct orientation or regular pattern."@en ;
    skos:notation "DUH"@en ;
    skos:prefLabel "Hummocky (weakly oriented dune)"@en .

<landform-element-DUN> a skos:Concept ;
    rdfs:label "Dune"@en ;
    dct:description "Moderately inclined to very steep ridge or hillock built up by the wind. This element may comprise dunecrest and duneslope."@en ;
    dct:identifier "http://anzsoil.org/def/au/asls/landform/landform-element-DUN"^^xsd:anyURI ;
    ui:isMemberOf <landform-element> ;
    owl:sameAs <http://anzsoil.org/def/au/asls/landform/landform-element-DUN> ;
    skos:definition "Moderately inclined to very steep ridge or hillock built up by the wind. This element may comprise dunecrest and duneslope."@en ;
    skos:notation "DUN"@en ;
    skos:prefLabel "Dune"@en .

<landform-element-DUP> a skos:Concept ;
    rdfs:label "Parabolic dune"@en ;
    dct:description "Sand dune with a long, scoop-shaped form, convex in the downwind direction so that its horns point upwind, whose ground plan approximates the form of a parabola. The dunes left behind can be referred to as trailing arms. Where many such dunes have traversed an area, these can give the appearance of linear dunes."@en ;
    dct:identifier "http://anzsoil.org/def/au/asls/landform/landform-element-DUP"^^xsd:anyURI ;
    ui:isMemberOf <landform-element> ;
    owl:sameAs <http://anzsoil.org/def/au/asls/landform/landform-element-DUP> ;
    skos:definition "Sand dune with a long, scoop-shaped form, convex in the downwind direction so that its horns point upwind, whose ground plan approximates the form of a parabola. The dunes left behind can be referred to as trailing arms. Where many such dunes have traversed an area, these can give the appearance of linear dunes."@en ;
    skos:notation "DUP"@en ;
    skos:prefLabel "Parabolic dune"@en .

<landform-element-DUS> a skos:Concept ;
    rdfs:label "Dune slope"@en ;
    dct:description "Slope built up or eroded by the wind (see Dune)."@en ;
    dct:identifier "http://anzsoil.org/def/au/asls/landform/landform-element-DUS"^^xsd:anyURI ;
    ui:isMemberOf <landform-element> ;
    owl:sameAs <http://anzsoil.org/def/au/asls/landform/landform-element-DUS> ;
    skos:definition "Slope built up or eroded by the wind (see Dune)."@en ;
    skos:notation "DUS"@en ;
    skos:prefLabel "Dune slope"@en .

<landform-element-EMB> a skos:Concept ;
    rdfs:label "Embankment"@en ;
    dct:description "Ridge or slope built up by human activity."@en ;
    dct:identifier "http://anzsoil.org/def/au/asls/landform/landform-element-EMB"^^xsd:anyURI ;
    ui:isMemberOf <landform-element> ;
    owl:sameAs <http://anzsoil.org/def/au/asls/landform/landform-element-EMB> ;
    skos:definition "Ridge or slope built up by human activity."@en ;
    skos:notation "EMB"@en ;
    skos:prefLabel "Embankment"@en .

<landform-element-EST> a skos:Concept ;
    rdfs:label "Estuary"@en ;
    dct:description "Stream channel close to its junction with a sea or lake, where the action of channelled stream flow is modified by tide and waves. The width typically increases downstream."@en ;
    dct:identifier "http://anzsoil.org/def/au/asls/landform/landform-element-EST"^^xsd:anyURI ;
    ui:isMemberOf <landform-element> ;
    owl:sameAs <http://anzsoil.org/def/au/asls/landform/landform-element-EST> ;
    skos:definition "Stream channel close to its junction with a sea or lake, where the action of channelled stream flow is modified by tide and waves. The width typically increases downstream."@en ;
    skos:notation "EST"@en ;
    skos:prefLabel "Estuary"@en .

<landform-element-FAN> a skos:Concept ;
    rdfs:label "Fan"@en ;
    dct:description "Large, gently inclined to level element with radial slope lines inclined away from a point, resulting from aggradation, or occasionally from erosion, by channelled, often braided, stream flow, or possibly by sheet flow."@en ;
    dct:identifier "http://anzsoil.org/def/au/asls/landform/landform-element-FAN"^^xsd:anyURI ;
    ui:isMemberOf <landform-element> ;
    owl:sameAs <http://anzsoil.org/def/au/asls/landform/landform-element-FAN> ;
    skos:definition "Large, gently inclined to level element with radial slope lines inclined away from a point, resulting from aggradation, or occasionally from erosion, by channelled, often braided, stream flow, or possibly by sheet flow."@en ;
    skos:notation "FAN"@en ;
    skos:prefLabel "Fan"@en .

<landform-element-FIL> a skos:Concept ;
    rdfs:label "Fil-top"@en ;
    dct:description "Flat aggraded by human activity."@en ;
    dct:identifier "http://anzsoil.org/def/au/asls/landform/landform-element-FIL"^^xsd:anyURI ;
    ui:isMemberOf <landform-element> ;
    owl:sameAs <http://anzsoil.org/def/au/asls/landform/landform-element-FIL> ;
    skos:definition "Flat aggraded by human activity."@en ;
    skos:notation "FIL"@en ;
    skos:prefLabel "Fil-top"@en .

<landform-element-FLD> a skos:Concept ;
    rdfs:label "Floodout"@en ;
    dct:description "Flat inclined radially away from a point on the margin or at the end of a stream channel, aggraded by overbank stream flow, or by channelled stream flow associated with channels developed within the overbank flow, part of a covered plain landform pattern."@en ;
    dct:identifier "http://anzsoil.org/def/au/asls/landform/landform-element-FLD"^^xsd:anyURI ;
    ui:isMemberOf <landform-element> ;
    owl:sameAs <http://anzsoil.org/def/au/asls/landform/landform-element-FLD> ;
    skos:definition "Flat inclined radially away from a point on the margin or at the end of a stream channel, aggraded by overbank stream flow, or by channelled stream flow associated with channels developed within the overbank flow, part of a covered plain landform pattern."@en ;
    skos:notation "FLD"@en ;
    skos:prefLabel "Floodout"@en .

<landform-element-FOO> a skos:Concept ;
    rdfs:label "Footslope"@en ;
    dct:description "Moderately to very gently inclined waning lower slope resulting from aggradation or erosion by sheet flow, earth flow or creep."@en ;
    dct:identifier "http://anzsoil.org/def/au/asls/landform/landform-element-FOO"^^xsd:anyURI ;
    ui:isMemberOf <landform-element> ;
    owl:sameAs <http://anzsoil.org/def/au/asls/landform/landform-element-FOO> ;
    skos:definition "Moderately to very gently inclined waning lower slope resulting from aggradation or erosion by sheet flow, earth flow or creep."@en ;
    skos:notation "FOO"@en ;
    skos:prefLabel "Footslope"@en .

<landform-element-FOR> a skos:Concept ;
    rdfs:label "Foredune"@en ;
    dct:description "Very long, nearly straight moderately inclined to very steep ridge built up by the wind from material from an adjacent beach."@en ;
    dct:identifier "http://anzsoil.org/def/au/asls/landform/landform-element-FOR"^^xsd:anyURI ;
    ui:isMemberOf <landform-element> ;
    owl:sameAs <http://anzsoil.org/def/au/asls/landform/landform-element-FOR> ;
    skos:definition "Very long, nearly straight moderately inclined to very steep ridge built up by the wind from material from an adjacent beach."@en ;
    skos:notation "FOR"@en ;
    skos:prefLabel "Foredune"@en .

<landform-element-GUL> a skos:Concept ;
    rdfs:label "Gully"@en ;
    dct:description "Open depression with short, precipitous walls and moderately inclined to very gently inclined floor or small stream channel, eroded by channelled stream flow and consequent collapse and water-aided mass movement."@en ;
    dct:identifier "http://anzsoil.org/def/au/asls/landform/landform-element-GUL"^^xsd:anyURI ;
    ui:isMemberOf <landform-element> ;
    owl:sameAs <http://anzsoil.org/def/au/asls/landform/landform-element-GUL> ;
    skos:definition "Open depression with short, precipitous walls and moderately inclined to very gently inclined floor or small stream channel, eroded by channelled stream flow and consequent collapse and water-aided mass movement."@en ;
    skos:notation "GUL"@en ;
    skos:prefLabel "Gully"@en .

<landform-element-HCR> a skos:Concept ;
    rdfs:label "Hillcrest"@en ;
    dct:description "Very gently inclined to steep crest, smoothly convex, eroded mainly by creep and sheet wash. A typical element of mountains, hills, low hills and rises."@en ;
    dct:identifier "http://anzsoil.org/def/au/asls/landform/landform-element-HCR"^^xsd:anyURI ;
    ui:isMemberOf <landform-element> ;
    owl:sameAs <http://anzsoil.org/def/au/asls/landform/landform-element-HCR> ;
    skos:definition "Very gently inclined to steep crest, smoothly convex, eroded mainly by creep and sheet wash. A typical element of mountains, hills, low hills and rises."@en ;
    skos:notation "HCR"@en ;
    skos:prefLabel "Hillcrest"@en .

<landform-element-HSL> a skos:Concept ;
    rdfs:label "Hillslope"@en ;
    dct:description "Gently inclined to precipitous slope, commonly simple and maximal, eroded by sheet wash, creep or water-aided mass movement. A typical element of mountains, hills, low hills and rises."@en ;
    dct:identifier "http://anzsoil.org/def/au/asls/landform/landform-element-HSL"^^xsd:anyURI ;
    ui:isMemberOf <landform-element> ;
    owl:sameAs <http://anzsoil.org/def/au/asls/landform/landform-element-HSL> ;
    skos:definition "Gently inclined to precipitous slope, commonly simple and maximal, eroded by sheet wash, creep or water-aided mass movement. A typical element of mountains, hills, low hills and rises."@en ;
    skos:notation "HSL"@en ;
    skos:prefLabel "Hillslope"@en .

<landform-element-ITF> a skos:Concept ;
    rdfs:label "Intertidal flat"@en ;
    dct:description "See Tidal flat."@en ;
    dct:identifier "http://anzsoil.org/def/au/asls/landform/landform-element-ITF"^^xsd:anyURI ;
    ui:isMemberOf <landform-element> ;
    owl:sameAs <http://anzsoil.org/def/au/asls/landform/landform-element-ITF> ;
    skos:definition "See Tidal flat."@en ;
    skos:notation "ITF"@en ;
    skos:prefLabel "Intertidal flat"@en .

<landform-element-LAG> a skos:Concept ;
    rdfs:label "Lagoon"@en ;
    dct:description "Closed depression filled with water that is typically salt or brackish, bounded at least in part by forms aggraded or built up by waves or reef-building organisms."@en ;
    dct:identifier "http://anzsoil.org/def/au/asls/landform/landform-element-LAG"^^xsd:anyURI ;
    ui:isMemberOf <landform-element> ;
    owl:sameAs <http://anzsoil.org/def/au/asls/landform/landform-element-LAG> ;
    skos:definition "Closed depression filled with water that is typically salt or brackish, bounded at least in part by forms aggraded or built up by waves or reef-building organisms."@en ;
    skos:notation "LAG"@en ;
    skos:prefLabel "Lagoon"@en .

<landform-element-LAK> a skos:Concept ;
    rdfs:label "Lake"@en ;
    dct:description "Large, water-filled closed depression."@en ;
    dct:identifier "http://anzsoil.org/def/au/asls/landform/landform-element-LAK"^^xsd:anyURI ;
    ui:isMemberOf <landform-element> ;
    owl:sameAs <http://anzsoil.org/def/au/asls/landform/landform-element-LAK> ;
    skos:definition "Large, water-filled closed depression."@en ;
    skos:notation "LAK"@en ;
    skos:prefLabel "Lake"@en .

<landform-element-LDS> a skos:Concept ;
    rdfs:label "Landslide"@en ;
    dct:description "Moderately inclined to very steep slope, eroded in the upper part and aggraded in the lower part by water-aided mass movement, characterised by irregular hummocks."@en ;
    dct:identifier "http://anzsoil.org/def/au/asls/landform/landform-element-LDS"^^xsd:anyURI ;
    ui:isMemberOf <landform-element> ;
    owl:sameAs <http://anzsoil.org/def/au/asls/landform/landform-element-LDS> ;
    skos:definition "Moderately inclined to very steep slope, eroded in the upper part and aggraded in the lower part by water-aided mass movement, characterised by irregular hummocks."@en ;
    skos:notation "LDS"@en ;
    skos:prefLabel "Landslide"@en .

<landform-element-LEV> a skos:Concept ;
    rdfs:label "Levee"@en ;
    dct:description "Very long, low, narrow, nearly level, sinuous ridge immediately adjacent to a stream channel, built up by overbank flow. Levees are built usually in pairs bounding the two sides of a stream channel, at the level reached by frequent floods. This element is part of a covered plain landform pattern. For an artificial levee, use Embankment. See also Prior stream."@en ;
    dct:identifier "http://anzsoil.org/def/au/asls/landform/landform-element-LEV"^^xsd:anyURI ;
    ui:isMemberOf <landform-element> ;
    owl:sameAs <http://anzsoil.org/def/au/asls/landform/landform-element-LEV> ;
    skos:definition "Very long, low, narrow, nearly level, sinuous ridge immediately adjacent to a stream channel, built up by overbank flow. Levees are built usually in pairs bounding the two sides of a stream channel, at the level reached by frequent floods. This element is part of a covered plain landform pattern. For an artificial levee, use Embankment. See also Prior stream."@en ;
    skos:notation "LEV"@en ;
    skos:prefLabel "Levee"@en .

<landform-element-LUN> a skos:Concept ;
    rdfs:label "Lunette"@en ;
    dct:description "Elongated, gently curved, low ridge built up by wind on the margin of a playa, typically with a moderate, wave-modified slope towards the playa and a gentle outer slope."@en ;
    dct:identifier "http://anzsoil.org/def/au/asls/landform/landform-element-LUN"^^xsd:anyURI ;
    ui:isMemberOf <landform-element> ;
    owl:sameAs <http://anzsoil.org/def/au/asls/landform/landform-element-LUN> ;
    skos:definition "Elongated, gently curved, low ridge built up by wind on the margin of a playa, typically with a moderate, wave-modified slope towards the playa and a gentle outer slope."@en ;
    skos:notation "LUN"@en ;
    skos:prefLabel "Lunette"@en .

<landform-element-MAA> a skos:Concept ;
    rdfs:label "Maar"@en ;
    dct:description "Level-floored, commonly water-filled closed depression with a nearly circular, steep rim, excavated by volcanism."@en ;
    dct:identifier "http://anzsoil.org/def/au/asls/landform/landform-element-MAA"^^xsd:anyURI ;
    ui:isMemberOf <landform-element> ;
    owl:sameAs <http://anzsoil.org/def/au/asls/landform/landform-element-MAA> ;
    skos:definition "Level-floored, commonly water-filled closed depression with a nearly circular, steep rim, excavated by volcanism."@en ;
    skos:notation "MAA"@en ;
    skos:prefLabel "Maar"@en .

<landform-element-MOU> a skos:Concept ;
    rdfs:label "Mound"@en ;
    dct:description "Hillock built up by human activity."@en ;
    dct:identifier "http://anzsoil.org/def/au/asls/landform/landform-element-MOU"^^xsd:anyURI ;
    ui:isMemberOf <landform-element> ;
    owl:sameAs <http://anzsoil.org/def/au/asls/landform/landform-element-MOU> ;
    skos:definition "Hillock built up by human activity."@en ;
    skos:notation "MOU"@en ;
    skos:prefLabel "Mound"@en .

<landform-element-OXB> a skos:Concept ;
    rdfs:label "Ox-bow"@en ;
    dct:description "Long, curved, commonly water-filled closed depression eroded by channelled stream flow but closed as a result of aggradation by channelled or overbank stream flow during the formation of a meander plain landform pattern. The floor of an ox-bow may be more or less aggraded by overbank stream flow, wind, and biological (peat) accumulation."@en ;
    dct:identifier "http://anzsoil.org/def/au/asls/landform/landform-element-OXB"^^xsd:anyURI ;
    ui:isMemberOf <landform-element> ;
    owl:sameAs <http://anzsoil.org/def/au/asls/landform/landform-element-OXB> ;
    skos:definition "Long, curved, commonly water-filled closed depression eroded by channelled stream flow but closed as a result of aggradation by channelled or overbank stream flow during the formation of a meander plain landform pattern. The floor of an ox-bow may be more or less aggraded by overbank stream flow, wind, and biological (peat) accumulation."@en ;
    skos:notation "OXB"@en ;
    skos:prefLabel "Ox-bow"@en .

<landform-element-PED> a skos:Concept ;
    rdfs:label "Pediment"@en ;
    dct:description "Large, gently inclined to level (<1%) waning lower slope, with slope lines inclined in a single direction, or somewhat convergent or divergent, eroded or sometimes slightly aggraded by sheet flow. It is underlain by bedrock."@en ;
    dct:identifier "http://anzsoil.org/def/au/asls/landform/landform-element-PED"^^xsd:anyURI ;
    ui:isMemberOf <landform-element> ;
    owl:sameAs <http://anzsoil.org/def/au/asls/landform/landform-element-PED> ;
    skos:definition "Large, gently inclined to level (<1%) waning lower slope, with slope lines inclined in a single direction, or somewhat convergent or divergent, eroded or sometimes slightly aggraded by sheet flow. It is underlain by bedrock."@en ;
    skos:notation "PED"@en ;
    skos:prefLabel "Pediment"@en .

<landform-element-PIT> a skos:Concept ;
    rdfs:label "Pit"@en ;
    dct:description "Closed depression excavated by human activity."@en ;
    dct:identifier "http://anzsoil.org/def/au/asls/landform/landform-element-PIT"^^xsd:anyURI ;
    ui:isMemberOf <landform-element> ;
    owl:sameAs <http://anzsoil.org/def/au/asls/landform/landform-element-PIT> ;
    skos:definition "Closed depression excavated by human activity."@en ;
    skos:notation "PIT"@en ;
    skos:prefLabel "Pit"@en .

<landform-element-PLA> a skos:Concept ;
    rdfs:label "Plain"@en ;
    dct:description "Large, very gently inclined or level element, of unspecified geomorphological agent or mode of activity."@en ;
    dct:identifier "http://anzsoil.org/def/au/asls/landform/landform-element-PLA"^^xsd:anyURI ;
    ui:isMemberOf <landform-element> ;
    owl:sameAs <http://anzsoil.org/def/au/asls/landform/landform-element-PLA> ;
    skos:definition "Large, very gently inclined or level element, of unspecified geomorphological agent or mode of activity."@en ;
    skos:notation "PLA"@en ;
    skos:prefLabel "Plain"@en .

<landform-element-PLY> a skos:Concept ;
    rdfs:label "Playa/pan"@en ;
    dct:description "Large, shallow, level-floored closed depression, intermittently water-filled, but mainly dry due to evaporation, bounded as a rule by flats aggraded by sheet flow and channelled stream flow."@en ;
    dct:identifier "http://anzsoil.org/def/au/asls/landform/landform-element-PLY"^^xsd:anyURI ;
    ui:isMemberOf <landform-element> ;
    owl:sameAs <http://anzsoil.org/def/au/asls/landform/landform-element-PLY> ;
    skos:definition "Large, shallow, level-floored closed depression, intermittently water-filled, but mainly dry due to evaporation, bounded as a rule by flats aggraded by sheet flow and channelled stream flow."@en ;
    skos:notation "PLY"@en ;
    skos:prefLabel "Playa/pan"@en .

<landform-element-PST> a skos:Concept ;
    rdfs:label "Prior stream"@en ;
    dct:description "Long, generally sinuous, low ridge built up from materials originally deposited by stream flow along the line of a former stream channel. The landform element may include a depression marking the old stream bed, and relict levees."@en ;
    dct:identifier "http://anzsoil.org/def/au/asls/landform/landform-element-PST"^^xsd:anyURI ;
    ui:isMemberOf <landform-element> ;
    owl:sameAs <http://anzsoil.org/def/au/asls/landform/landform-element-PST> ;
    skos:definition "Long, generally sinuous, low ridge built up from materials originally deposited by stream flow along the line of a former stream channel. The landform element may include a depression marking the old stream bed, and relict levees."@en ;
    skos:notation "PST"@en ;
    skos:prefLabel "Prior stream"@en .

<landform-element-REC> a skos:Concept ;
    rdfs:label "Risecrest"@en ;
    dct:description "Crest of hillock of very low to extremely low relief (<30 m) (see Residual rise)."@en ;
    dct:identifier "http://anzsoil.org/def/au/asls/landform/landform-element-REC"^^xsd:anyURI ;
    ui:isMemberOf <landform-element> ;
    owl:sameAs <http://anzsoil.org/def/au/asls/landform/landform-element-REC> ;
    skos:definition "Crest of hillock of very low to extremely low relief (<30 m) (see Residual rise)."@en ;
    skos:notation "REC"@en ;
    skos:prefLabel "Risecrest"@en .

<landform-element-REF> a skos:Concept ;
    rdfs:label "Reef flat"@en ;
    dct:description "Flat built up to sea level by marine organisms."@en ;
    dct:identifier "http://anzsoil.org/def/au/asls/landform/landform-element-REF"^^xsd:anyURI ;
    ui:isMemberOf <landform-element> ;
    owl:sameAs <http://anzsoil.org/def/au/asls/landform/landform-element-REF> ;
    skos:definition "Flat built up to sea level by marine organisms."@en ;
    skos:notation "REF"@en ;
    skos:prefLabel "Reef flat"@en .

<landform-element-RER> a skos:Concept ;
    rdfs:label "Residual rise"@en ;
    dct:description "Hillock of very low to extremely low relief (<30 m) and very gentle to steep slopes. This term is used to refer to an isolated rise surrounded by other landforms."@en ;
    dct:identifier "http://anzsoil.org/def/au/asls/landform/landform-element-RER"^^xsd:anyURI ;
    ui:isMemberOf <landform-element> ;
    owl:sameAs <http://anzsoil.org/def/au/asls/landform/landform-element-RER> ;
    skos:definition "Hillock of very low to extremely low relief (<30 m) and very gentle to steep slopes. This term is used to refer to an isolated rise surrounded by other landforms."@en ;
    skos:notation "RER"@en ;
    skos:prefLabel "Residual rise"@en .

<landform-element-RES> a skos:Concept ;
    rdfs:label "Riseslope"@en ;
    dct:description "Slope of hillock of very low to extremely low relief (<30 m) (see Residual rise)."@en ;
    dct:identifier "http://anzsoil.org/def/au/asls/landform/landform-element-RES"^^xsd:anyURI ;
    ui:isMemberOf <landform-element> ;
    owl:sameAs <http://anzsoil.org/def/au/asls/landform/landform-element-RES> ;
    skos:definition "Slope of hillock of very low to extremely low relief (<30 m) (see Residual rise)."@en ;
    skos:notation "RES"@en ;
    skos:prefLabel "Riseslope"@en .

<landform-element-RFL> a skos:Concept ;
    rdfs:label "Rock flat"@en ;
    dct:description "Flat of bare consolidated rock, usually eroded by sheet wash."@en ;
    dct:identifier "http://anzsoil.org/def/au/asls/landform/landform-element-RFL"^^xsd:anyURI ;
    ui:isMemberOf <landform-element> ;
    owl:sameAs <http://anzsoil.org/def/au/asls/landform/landform-element-RFL> ;
    skos:definition "Flat of bare consolidated rock, usually eroded by sheet wash."@en ;
    skos:notation "RFL"@en ;
    skos:prefLabel "Rock flat"@en .

<landform-element-RPL> a skos:Concept ;
    rdfs:label "Rock platform"@en ;
    dct:description "Flat of consolidated rock eroded by waves."@en ;
    dct:identifier "http://anzsoil.org/def/au/asls/landform/landform-element-RPL"^^xsd:anyURI ;
    ui:isMemberOf <landform-element> ;
    owl:sameAs <http://anzsoil.org/def/au/asls/landform/landform-element-RPL> ;
    skos:definition "Flat of consolidated rock eroded by waves."@en ;
    skos:notation "RPL"@en ;
    skos:prefLabel "Rock platform"@en .

<landform-element-SCA> a skos:Concept ;
    rdfs:label "Scarp"@en ;
    dct:description "Very wide, steep to precipitous maximal slope eroded by gravlty, water-aided mass movement or sheet flow."@en ;
    dct:identifier "http://anzsoil.org/def/au/asls/landform/landform-element-SCA"^^xsd:anyURI ;
    ui:isMemberOf <landform-element> ;
    owl:sameAs <http://anzsoil.org/def/au/asls/landform/landform-element-SCA> ;
    skos:definition "Very wide, steep to precipitous maximal slope eroded by gravlty, water-aided mass movement or sheet flow."@en ;
    skos:notation "SCA"@en ;
    skos:prefLabel "Scarp"@en .

<landform-element-SCD> a skos:Concept ;
    rdfs:label "Scald"@en ;
    dct:description "Flat, bare of vegetatiorn, from which soil has been eroded or excavated by surface wash or wind."@en ;
    dct:identifier "http://anzsoil.org/def/au/asls/landform/landform-element-SCD"^^xsd:anyURI ;
    ui:isMemberOf <landform-element> ;
    owl:sameAs <http://anzsoil.org/def/au/asls/landform/landform-element-SCD> ;
    skos:definition "Flat, bare of vegetatiorn, from which soil has been eroded or excavated by surface wash or wind."@en ;
    skos:notation "SCD"@en ;
    skos:prefLabel "Scald"@en .

<landform-element-SCR> a skos:Concept ;
    rdfs:label "Scroll"@en ;
    dct:description "Long, curved, very low ridge built up by channelled stream flow and left relict by channel migration. Part of a meander plain landform pattern."@en ;
    dct:identifier "http://anzsoil.org/def/au/asls/landform/landform-element-SCR"^^xsd:anyURI ;
    ui:isMemberOf <landform-element> ;
    owl:sameAs <http://anzsoil.org/def/au/asls/landform/landform-element-SCR> ;
    skos:definition "Long, curved, very low ridge built up by channelled stream flow and left relict by channel migration. Part of a meander plain landform pattern."@en ;
    skos:notation "SCR"@en ;
    skos:prefLabel "Scroll"@en .

<landform-element-SFS> a skos:Concept ;
    rdfs:label "Scarp-footslope"@en ;
    dct:description "Waning or minimal slope situated below a scarp, with its contours generally parallel to the line of the scarp."@en ;
    dct:identifier "http://anzsoil.org/def/au/asls/landform/landform-element-SFS"^^xsd:anyURI ;
    ui:isMemberOf <landform-element> ;
    owl:sameAs <http://anzsoil.org/def/au/asls/landform/landform-element-SFS> ;
    skos:definition "Waning or minimal slope situated below a scarp, with its contours generally parallel to the line of the scarp."@en ;
    skos:notation "SFS"@en ;
    skos:prefLabel "Scarp-footslope"@en .

<landform-element-SRP> a skos:Concept ;
    rdfs:label "Scroll plain"@en ;
    dct:description "Large flat resulting from aggradation by channelled stream flow as a stream migrates from side to side, the dominant element of a meander plain landform pattern. This landform element may include occurrences of scroll, swale and ox-bow."@en ;
    dct:identifier "http://anzsoil.org/def/au/asls/landform/landform-element-SRP"^^xsd:anyURI ;
    ui:isMemberOf <landform-element> ;
    owl:sameAs <http://anzsoil.org/def/au/asls/landform/landform-element-SRP> ;
    skos:definition "Large flat resulting from aggradation by channelled stream flow as a stream migrates from side to side, the dominant element of a meander plain landform pattern. This landform element may include occurrences of scroll, swale and ox-bow."@en ;
    skos:notation "SRP"@en ;
    skos:prefLabel "Scroll plain"@en .

<landform-element-STB> a skos:Concept ;
    rdfs:label "Stream bed"@en ;
    dct:description "Linear, generally sinuous open depression forming the bottom of a stream channel, eroded and locally excavated, aggraded or built up by channelled stream flow. Parts that are built up include bars."@en ;
    dct:identifier "http://anzsoil.org/def/au/asls/landform/landform-element-STB"^^xsd:anyURI ;
    ui:isMemberOf <landform-element> ;
    owl:sameAs <http://anzsoil.org/def/au/asls/landform/landform-element-STB> ;
    skos:definition "Linear, generally sinuous open depression forming the bottom of a stream channel, eroded and locally excavated, aggraded or built up by channelled stream flow. Parts that are built up include bars."@en ;
    skos:notation "STB"@en ;
    skos:prefLabel "Stream bed"@en .

<landform-element-STC> a skos:Concept ;
    rdfs:label "Stream channel"@en ;
    dct:description "Linear, generally sinuous open depression, in parts eroded, excavated, built up and aggraded by channelled stream flow. This element comprises stream bed and banks."@en ;
    dct:identifier "http://anzsoil.org/def/au/asls/landform/landform-element-STC"^^xsd:anyURI ;
    ui:isMemberOf <landform-element> ;
    owl:sameAs <http://anzsoil.org/def/au/asls/landform/landform-element-STC> ;
    skos:definition "Linear, generally sinuous open depression, in parts eroded, excavated, built up and aggraded by channelled stream flow. This element comprises stream bed and banks."@en ;
    skos:notation "STC"@en ;
    skos:prefLabel "Stream channel"@en .

<landform-element-STF> a skos:Concept ;
    rdfs:label "Supratidal flat"@en ;
    dct:description "See Tidal flat."@en ;
    dct:identifier "http://anzsoil.org/def/au/asls/landform/landform-element-STF"^^xsd:anyURI ;
    ui:isMemberOf <landform-element> ;
    owl:sameAs <http://anzsoil.org/def/au/asls/landform/landform-element-STF> ;
    skos:definition "See Tidal flat."@en ;
    skos:notation "STF"@en ;
    skos:prefLabel "Supratidal flat"@en .

<landform-element-SUS> a skos:Concept ;
    rdfs:label "Summit surface"@en ;
    dct:description "Very wide, level to gently inclined crest with abrupt margins, commonly eroded by water-aided mass movement or sheet wash."@en ;
    dct:identifier "http://anzsoil.org/def/au/asls/landform/landform-element-SUS"^^xsd:anyURI ;
    ui:isMemberOf <landform-element> ;
    owl:sameAs <http://anzsoil.org/def/au/asls/landform/landform-element-SUS> ;
    skos:definition "Very wide, level to gently inclined crest with abrupt margins, commonly eroded by water-aided mass movement or sheet wash."@en ;
    skos:notation "SUS"@en ;
    skos:prefLabel "Summit surface"@en .

<landform-element-SWL> a skos:Concept ;
    rdfs:label "Swale"@en ;
    dct:description "(i) Linear, level-floored open depression excavated by wind, or left relict between ridges built up by wind or waves, or built up to a lesser height than them. (ii) Long, curved open or closed depression left relict between scrolls built up by channelled stream flow."@en ;
    dct:identifier "http://anzsoil.org/def/au/asls/landform/landform-element-SWL"^^xsd:anyURI ;
    ui:isMemberOf <landform-element> ;
    owl:sameAs <http://anzsoil.org/def/au/asls/landform/landform-element-SWL> ;
    skos:definition "(i) Linear, level-floored open depression excavated by wind, or left relict between ridges built up by wind or waves, or built up to a lesser height than them. (ii) Long, curved open or closed depression left relict between scrolls built up by channelled stream flow."@en ;
    skos:notation "SWL"@en ;
    skos:prefLabel "Swale"@en .

<landform-element-SWP> a skos:Concept ;
    rdfs:label "Swamp"@en ;
    dct:description "Almost level, closed or almost closed depression with a seasonal or permanent watertable at or above the surface, commonly aggraded by overbank stream flow and sometimes biological (peat) accumulation."@en ;
    dct:identifier "http://anzsoil.org/def/au/asls/landform/landform-element-SWP"^^xsd:anyURI ;
    ui:isMemberOf <landform-element> ;
    owl:sameAs <http://anzsoil.org/def/au/asls/landform/landform-element-SWP> ;
    skos:definition "Almost level, closed or almost closed depression with a seasonal or permanent watertable at or above the surface, commonly aggraded by overbank stream flow and sometimes biological (peat) accumulation."@en ;
    skos:notation "SWP"@en ;
    skos:prefLabel "Swamp"@en .

<landform-element-TAL> a skos:Concept ;
    rdfs:label "Talus"@en ;
    dct:description "Moderately inclined or steep waning lower slope, consisting of rock fragments aggraded by gravlty."@en ;
    dct:identifier "http://anzsoil.org/def/au/asls/landform/landform-element-TAL"^^xsd:anyURI ;
    ui:isMemberOf <landform-element> ;
    owl:sameAs <http://anzsoil.org/def/au/asls/landform/landform-element-TAL> ;
    skos:definition "Moderately inclined or steep waning lower slope, consisting of rock fragments aggraded by gravlty."@en ;
    skos:notation "TAL"@en ;
    skos:prefLabel "Talus"@en .

<landform-element-TDC> a skos:Concept ;
    rdfs:label "Tidal creek"@en ;
    dct:description "Intermittently water-filled open depression in parts eroded, excavated, built up and aggraded by channelled tide-water flow, type of stream channel characterised by a rapid increase in width downstream."@en ;
    dct:identifier "http://anzsoil.org/def/au/asls/landform/landform-element-TDC"^^xsd:anyURI ;
    ui:isMemberOf <landform-element> ;
    owl:sameAs <http://anzsoil.org/def/au/asls/landform/landform-element-TDC> ;
    skos:definition "Intermittently water-filled open depression in parts eroded, excavated, built up and aggraded by channelled tide-water flow, type of stream channel characterised by a rapid increase in width downstream."@en ;
    skos:notation "TDC"@en ;
    skos:prefLabel "Tidal creek"@en .

<landform-element-TDF> a skos:Concept ;
    rdfs:label "Tidal flat"@en ;
    dct:description "Large flat subject to inundation by water that is usually salt or brackish, aggradedby tides. An intertidal flat (ITF) is frequently inundated, a supratidal flat (STF) is seldom inundated."@en ;
    dct:identifier "http://anzsoil.org/def/au/asls/landform/landform-element-TDF"^^xsd:anyURI ;
    ui:isMemberOf <landform-element> ;
    owl:sameAs <http://anzsoil.org/def/au/asls/landform/landform-element-TDF> ;
    skos:definition "Large flat subject to inundation by water that is usually salt or brackish, aggradedby tides. An intertidal flat (ITF) is frequently inundated, a supratidal flat (STF) is seldom inundated."@en ;
    skos:notation "TDF"@en ;
    skos:prefLabel "Tidal flat"@en .

<landform-element-TEF> a skos:Concept ;
    rdfs:label "Terrace Flat"@en ;
    dct:description "Small flat aggraded or eroded by channelled or overbank stream flow, standing above a scarp and no longer frequently inundated, a former valley flat or part of a former flood plain."@en ;
    dct:identifier "http://anzsoil.org/def/au/asls/landform/landform-element-TEF"^^xsd:anyURI ;
    ui:isMemberOf <landform-element> ;
    owl:sameAs <http://anzsoil.org/def/au/asls/landform/landform-element-TEF> ;
    skos:definition "Small flat aggraded or eroded by channelled or overbank stream flow, standing above a scarp and no longer frequently inundated, a former valley flat or part of a former flood plain."@en ;
    skos:notation "TEF"@en ;
    skos:prefLabel "Terrace Flat"@en .

<landform-element-TEP> a skos:Concept ;
    rdfs:label "Terrace plain"@en ;
    dct:description "Large or very large flat aggraded by channelled or overbank stream flow, standing above a scarp and no longer frequently inundated, part of a former flood plain."@en ;
    dct:identifier "http://anzsoil.org/def/au/asls/landform/landform-element-TEP"^^xsd:anyURI ;
    ui:isMemberOf <landform-element> ;
    owl:sameAs <http://anzsoil.org/def/au/asls/landform/landform-element-TEP> ;
    skos:definition "Large or very large flat aggraded by channelled or overbank stream flow, standing above a scarp and no longer frequently inundated, part of a former flood plain."@en ;
    skos:notation "TEP"@en ;
    skos:prefLabel "Terrace plain"@en .

<landform-element-TOR> a skos:Concept ;
    rdfs:label "Tor"@en ;
    dct:description "Steep to precipitous hillock, typically convex, with a surface mainly of bare rock, either coherent or comprising subangular to rounded, large boulders (exhumed core-stones, also themselves called tors) separated by open fissures, eroded by sheet wash or water-aided mass movement."@en ;
    dct:identifier "http://anzsoil.org/def/au/asls/landform/landform-element-TOR"^^xsd:anyURI ;
    ui:isMemberOf <landform-element> ;
    owl:sameAs <http://anzsoil.org/def/au/asls/landform/landform-element-TOR> ;
    skos:definition "Steep to precipitous hillock, typically convex, with a surface mainly of bare rock, either coherent or comprising subangular to rounded, large boulders (exhumed core-stones, also themselves called tors) separated by open fissures, eroded by sheet wash or water-aided mass movement."@en ;
    skos:notation "TOR"@en ;
    skos:prefLabel "Tor"@en .

<landform-element-TRE> a skos:Concept ;
    rdfs:label "Trench"@en ;
    dct:description "Open depression excavated by human activity."@en ;
    dct:identifier "http://anzsoil.org/def/au/asls/landform/landform-element-TRE"^^xsd:anyURI ;
    ui:isMemberOf <landform-element> ;
    owl:sameAs <http://anzsoil.org/def/au/asls/landform/landform-element-TRE> ;
    skos:definition "Open depression excavated by human activity."@en ;
    skos:notation "TRE"@en ;
    skos:prefLabel "Trench"@en .

<landform-element-TUM> a skos:Concept ;
    rdfs:label "Tumulus"@en ;
    dct:description "Hillock heaved up by volcanism (or, elsewhere, built up by human activity at a burial site)."@en ;
    dct:identifier "http://anzsoil.org/def/au/asls/landform/landform-element-TUM"^^xsd:anyURI ;
    ui:isMemberOf <landform-element> ;
    owl:sameAs <http://anzsoil.org/def/au/asls/landform/landform-element-TUM> ;
    skos:definition "Hillock heaved up by volcanism (or, elsewhere, built up by human activity at a burial site)."@en ;
    skos:notation "TUM"@en ;
    skos:prefLabel "Tumulus"@en .

<landform-element-VLF> a skos:Concept ;
    rdfs:label "Valley flat"@en ;
    dct:description "Small, gently inclined to level flat, aggraded or sometimes eroded by channelled or overbank stream flow, typically enclosed by hillslopes, a miniature alluvial plain landform pattern."@en ;
    dct:identifier "http://anzsoil.org/def/au/asls/landform/landform-element-VLF"^^xsd:anyURI ;
    ui:isMemberOf <landform-element> ;
    owl:sameAs <http://anzsoil.org/def/au/asls/landform/landform-element-VLF> ;
    skos:definition "Small, gently inclined to level flat, aggraded or sometimes eroded by channelled or overbank stream flow, typically enclosed by hillslopes, a miniature alluvial plain landform pattern."@en ;
    skos:notation "VLF"@en ;
    skos:prefLabel "Valley flat"@en .

<landform-element> a skos:Collection,
        <http://www.w3.org/ns/sosa/ObservableProperty> ;
    dct:source "National Committee on Soil and Terrain (2009), 'Australian soil and land survey field handbook (3rd edn).' (CSIRO Publishing: Melbourne)"@en ;
    ui:topMemberOf <> ;
    skos:member <landform-element-ALC>,
        <landform-element-BAN>,
        <landform-element-BAR>,
        <landform-element-BEA>,
        <landform-element-BEN>,
        <landform-element-BER>,
        <landform-element-BKP>,
        <landform-element-BOU>,
        <landform-element-BRI>,
        <landform-element-BRK>,
        <landform-element-CBE>,
        <landform-element-CFS>,
        <landform-element-CIR>,
        <landform-element-CLI>,
        <landform-element-CON>,
        <landform-element-COS>,
        <landform-element-CRA>,
        <landform-element-CUT>,
        <landform-element-DAM>,
        <landform-element-DBA>,
        <landform-element-DDE>,
        <landform-element-DOC>,
        <landform-element-DOL>,
        <landform-element-DUB>,
        <landform-element-DUC>,
        <landform-element-DUF>,
        <landform-element-DUH>,
        <landform-element-DUN>,
        <landform-element-DUP>,
        <landform-element-DUS>,
        <landform-element-EMB>,
        <landform-element-EST>,
        <landform-element-FAN>,
        <landform-element-FIL>,
        <landform-element-FLD>,
        <landform-element-FOO>,
        <landform-element-FOR>,
        <landform-element-GUL>,
        <landform-element-HCR>,
        <landform-element-HSL>,
        <landform-element-ITF>,
        <landform-element-LAG>,
        <landform-element-LAK>,
        <landform-element-LDS>,
        <landform-element-LEV>,
        <landform-element-LUN>,
        <landform-element-MAA>,
        <landform-element-MOU>,
        <landform-element-OXB>,
        <landform-element-PED>,
        <landform-element-PIT>,
        <landform-element-PLA>,
        <landform-element-PLY>,
        <landform-element-PST>,
        <landform-element-REC>,
        <landform-element-REF>,
        <landform-element-RER>,
        <landform-element-RES>,
        <landform-element-RFL>,
        <landform-element-RPL>,
        <landform-element-SCA>,
        <landform-element-SCD>,
        <landform-element-SCR>,
        <landform-element-SFS>,
        <landform-element-SRP>,
        <landform-element-STB>,
        <landform-element-STC>,
        <landform-element-STF>,
        <landform-element-SUS>,
        <landform-element-SWL>,
        <landform-element-SWP>,
        <landform-element-TAL>,
        <landform-element-TDC>,
        <landform-element-TDF>,
        <landform-element-TEF>,
        <landform-element-TEP>,
        <landform-element-TOR>,
        <landform-element-TRE>,
        <landform-element-TUM>,
        <landform-element-VLF> ;
    skos:prefLabel "Landform Element Key and Glossary"@en .

